<?xml version="1.0"?>
<rdf:RDF xmlns="https://purl.iso.org/idmp/iso-11239#"
     xml:base="https://purl.iso.org/idmp/iso-11239"
     xmlns:g="https://purl.iso.org/idmp/graphs/"
     xmlns:ns1="http://www.novartis.com/data_governance/knowledgefeed#"
     xmlns:nvs="https://data-qa.novartis.net/r1/informationtechnology/architecture/iserver/v1/object/"
     xmlns:owl="http://www.w3.org/2002/07/owl#"
     xmlns:rdf="http://www.w3.org/1999/02/22-rdf-syntax-ns#"
     xmlns:xml="http://www.w3.org/XML/1998/namespace"
     xmlns:xsd="http://www.w3.org/2001/XMLSchema#"
     xmlns:idmp="https://purl.iso.org/idmp/"
     xmlns:rdfs="http://www.w3.org/2000/01/rdf-schema#"
     xmlns:skos="http://www.w3.org/2004/02/skos/core#"
     xmlns:terms="http://purl.org/dc/terms/"
     xmlns:upper="https://data-qa.novartis.net/r1/enterprise/datastrategy/upperontology/v1/"
     xmlns:nvsdoc="https://data-qa.novartis.net/r1/informationtechnology/architecture/iserver/v1/document/"
     xmlns:skos-xl="http://www.w3.org/2008/05/skos-xl#"
     xmlns:authority="http://publications.europa.eu/ontology/authority/">
    <owl:Ontology rdf:about="https://purl.iso.org/idmp/iso-11239">
        <owl:versionIRI rdf:resource="https://purl.iso.org/idmp/iso-11239/0.2"/>
        <owl:imports rdf:resource="https://purl.iso.org/idmp/core"/>
        <terms:date rdf:datatype="http://www.w3.org/2001/XMLSchema#date">2020-11-05</terms:date>
        <terms:modified rdf:datatype="http://www.w3.org/2001/XMLSchema#date">2022-04-02</terms:modified>
        <terms:title>ISO IDMP 11239 Dose Forms.</terms:title>
        <rdfs:comment>This ontology contains entities of the domain of IDMP Dose Forms based on ISO standard ISO_11239_2012(en) Dose Forms</rdfs:comment>
        <rdfs:label>ISO IDMP 11239 Dose Forms.</rdfs:label>
    </owl:Ontology>
    


    <!-- 
    ///////////////////////////////////////////////////////////////////////////////////////
    //
    // Annotation properties
    //
    ///////////////////////////////////////////////////////////////////////////////////////
     -->

    


    <!-- http://purl.org/dc/terms/date -->

    <owl:AnnotationProperty rdf:about="http://purl.org/dc/terms/date"/>
    


    <!-- 
    ///////////////////////////////////////////////////////////////////////////////////////
    //
    // Object Properties
    //
    ///////////////////////////////////////////////////////////////////////////////////////
     -->

    


    <!-- https://purl.iso.org/idmp/currentConcept -->

    <owl:ObjectProperty rdf:about="https://purl.iso.org/idmp/currentConcept"/>
    


    <!-- 
    ///////////////////////////////////////////////////////////////////////////////////////
    //
    // Classes
    //
    ///////////////////////////////////////////////////////////////////////////////////////
     -->

    


    <!-- https://purl.iso.org/datatypes/CodeTermPair -->

    <owl:Class rdf:about="https://purl.iso.org/datatypes/CodeTermPair"/>
    


    <!-- https://purl.iso.org/idmp/AdministrationMethodClass -->

    <owl:Class rdf:about="https://purl.iso.org/idmp/AdministrationMethodClass">
        <rdfs:subClassOf rdf:resource="http://www.w3.org/2004/02/skos/core#Concept"/>
    </owl:Class>
    


    <!-- https://purl.iso.org/idmp/BasicDoseForm -->

    <owl:Class rdf:about="https://purl.iso.org/idmp/BasicDoseForm">
        <rdfs:subClassOf rdf:resource="http://www.w3.org/2004/02/skos/core#Concept"/>
    </owl:Class>
    


    <!-- https://purl.iso.org/idmp/Code -->

    <owl:Class rdf:about="https://purl.iso.org/idmp/Code">
        <rdfs:subClassOf rdf:resource="http://www.w3.org/2004/02/skos/core#Concept"/>
    </owl:Class>
    


    <!-- https://purl.iso.org/idmp/CodeTermPair -->

    <owl:Class rdf:about="https://purl.iso.org/idmp/CodeTermPair">
        <rdfs:subClassOf rdf:resource="http://www.w3.org/2004/02/skos/core#Concept"/>
    </owl:Class>
    


    <!-- https://purl.iso.org/idmp/CodedConcept -->

    <owl:Class rdf:about="https://purl.iso.org/idmp/CodedConcept">
        <rdfs:subClassOf rdf:resource="http://www.w3.org/2004/02/skos/core#Concept"/>
    </owl:Class>
    


    <!-- https://purl.iso.org/idmp/Comment -->

    <owl:Class rdf:about="https://purl.iso.org/idmp/Comment">
        <rdfs:subClassOf rdf:resource="http://www.w3.org/2004/02/skos/core#Concept"/>
    </owl:Class>
    


    <!-- https://purl.iso.org/idmp/ConceptStatus -->

    <owl:Class rdf:about="https://purl.iso.org/idmp/ConceptStatus">
        <rdfs:subClassOf rdf:resource="http://www.w3.org/2004/02/skos/core#Concept"/>
    </owl:Class>
    


    <!-- https://purl.iso.org/idmp/CreatedBy -->

    <owl:Class rdf:about="https://purl.iso.org/idmp/CreatedBy">
        <rdfs:subClassOf rdf:resource="http://www.w3.org/2004/02/skos/core#Concept"/>
    </owl:Class>
    


    <!-- https://purl.iso.org/idmp/CreationDate -->

    <owl:Class rdf:about="https://purl.iso.org/idmp/CreationDate">
        <rdfs:subClassOf rdf:resource="http://www.w3.org/2004/02/skos/core#Concept"/>
    </owl:Class>
    


    <!-- https://purl.iso.org/idmp/Definition -->

    <owl:Class rdf:about="https://purl.iso.org/idmp/Definition">
        <rdfs:subClassOf rdf:resource="http://www.w3.org/2004/02/skos/core#Concept"/>
    </owl:Class>
    


    <!-- https://purl.iso.org/idmp/Domain -->

    <owl:Class rdf:about="https://purl.iso.org/idmp/Domain">
        <rdfs:subClassOf rdf:resource="http://www.w3.org/2004/02/skos/core#Concept"/>
    </owl:Class>
    


    <!-- https://purl.iso.org/idmp/IntendedSiteClass -->

    <owl:Class rdf:about="https://purl.iso.org/idmp/IntendedSiteClass">
        <rdfs:subClassOf rdf:resource="http://www.w3.org/2004/02/skos/core#Concept"/>
    </owl:Class>
    


    <!-- https://purl.iso.org/idmp/LanguageCode -->

    <owl:Class rdf:about="https://purl.iso.org/idmp/LanguageCode">
        <rdfs:subClassOf rdf:resource="http://www.w3.org/2004/02/skos/core#Concept"/>
    </owl:Class>
    


    <!-- https://purl.iso.org/idmp/ModificationBy -->

    <owl:Class rdf:about="https://purl.iso.org/idmp/ModificationBy">
        <rdfs:subClassOf rdf:resource="http://www.w3.org/2004/02/skos/core#Concept"/>
    </owl:Class>
    


    <!-- https://purl.iso.org/idmp/ModificationDate -->

    <owl:Class rdf:about="https://purl.iso.org/idmp/ModificationDate">
        <rdfs:subClassOf rdf:resource="http://www.w3.org/2004/02/skos/core#Concept"/>
    </owl:Class>
    


    <!-- https://purl.iso.org/idmp/ModificationMade -->

    <owl:Class rdf:about="https://purl.iso.org/idmp/ModificationMade">
        <rdfs:subClassOf rdf:resource="http://www.w3.org/2004/02/skos/core#Concept"/>
    </owl:Class>
    


    <!-- https://purl.iso.org/idmp/Packaging -->

    <owl:Class rdf:about="https://purl.iso.org/idmp/Packaging">
        <rdfs:subClassOf rdf:resource="http://www.w3.org/2004/02/skos/core#Concept"/>
    </owl:Class>
    


    <!-- https://purl.iso.org/idmp/PackagingCategoryClass -->

    <owl:Class rdf:about="https://purl.iso.org/idmp/PackagingCategoryClass">
        <rdfs:subClassOf rdf:resource="http://www.w3.org/2004/02/skos/core#Concept"/>
    </owl:Class>
    


    <!-- https://purl.iso.org/idmp/PackagingClass -->

    <owl:Class rdf:about="https://purl.iso.org/idmp/PackagingClass">
        <rdfs:subClassOf rdf:resource="http://www.w3.org/2004/02/skos/core#Concept"/>
    </owl:Class>
    


    <!-- https://purl.iso.org/idmp/PharmaceuticalDoseForm -->

    <owl:Class rdf:about="https://purl.iso.org/idmp/PharmaceuticalDoseForm">
        <rdfs:subClassOf rdf:resource="http://www.w3.org/2004/02/skos/core#Concept"/>
    </owl:Class>
    


    <!-- https://purl.iso.org/idmp/RegionCode -->

    <owl:Class rdf:about="https://purl.iso.org/idmp/RegionCode">
        <rdfs:subClassOf rdf:resource="http://www.w3.org/2004/02/skos/core#Concept"/>
    </owl:Class>
    


    <!-- https://purl.iso.org/idmp/ReleaseCharacteristics -->

    <owl:Class rdf:about="https://purl.iso.org/idmp/ReleaseCharacteristics">
        <rdfs:subClassOf rdf:resource="http://www.w3.org/2004/02/skos/core#Concept"/>
    </owl:Class>
    


    <!-- https://purl.iso.org/idmp/RouteOfAdministration -->

    <owl:Class rdf:about="https://purl.iso.org/idmp/RouteOfAdministration">
        <rdfs:subClassOf rdf:resource="http://www.w3.org/2004/02/skos/core#Concept"/>
    </owl:Class>
    


    <!-- https://purl.iso.org/idmp/StateOfMatter -->

    <owl:Class rdf:about="https://purl.iso.org/idmp/StateOfMatter">
        <rdfs:subClassOf rdf:resource="http://www.w3.org/2004/02/skos/core#Concept"/>
    </owl:Class>
    


    <!-- https://purl.iso.org/idmp/Term -->

    <owl:Class rdf:about="https://purl.iso.org/idmp/Term">
        <rdfs:subClassOf rdf:resource="http://www.w3.org/2004/02/skos/core#Concept"/>
    </owl:Class>
    


    <!-- https://purl.iso.org/idmp/TransformationClass -->

    <owl:Class rdf:about="https://purl.iso.org/idmp/TransformationClass">
        <rdfs:subClassOf rdf:resource="http://www.w3.org/2004/02/skos/core#Concept"/>
    </owl:Class>
    


    <!-- https://purl.iso.org/idmp/Translation -->

    <owl:Class rdf:about="https://purl.iso.org/idmp/Translation">
        <rdfs:subClassOf rdf:resource="http://www.w3.org/2004/02/skos/core#Concept"/>
    </owl:Class>
    


    <!-- https://purl.iso.org/idmp/UnitOfPresentation -->

    <owl:Class rdf:about="https://purl.iso.org/idmp/UnitOfPresentation">
        <rdfs:subClassOf rdf:resource="http://www.w3.org/2004/02/skos/core#Concept"/>
    </owl:Class>
    


    <!-- https://purl.iso.org/idmp/Value -->

    <owl:Class rdf:about="https://purl.iso.org/idmp/Value">
        <rdfs:subClassOf rdf:resource="http://www.w3.org/2004/02/skos/core#Concept"/>
    </owl:Class>
    


    <!-- https://purl.iso.org/idmp/VersionNumber -->

    <owl:Class rdf:about="https://purl.iso.org/idmp/VersionNumber">
        <rdfs:subClassOf rdf:resource="http://www.w3.org/2004/02/skos/core#Concept"/>
    </owl:Class>
    


    <!-- https://purl.iso.org/idmp/Versioning -->

    <owl:Class rdf:about="https://purl.iso.org/idmp/Versioning">
        <rdfs:subClassOf rdf:resource="http://www.w3.org/2004/02/skos/core#Concept"/>
    </owl:Class>
    


    <!-- 
    ///////////////////////////////////////////////////////////////////////////////////////
    //
    // Individuals
    //
    ///////////////////////////////////////////////////////////////////////////////////////
     -->

    


    <!-- https://purl.iso.org/idmp/AdministrationMethodClass -->

    <owl:NamedIndividual rdf:about="https://purl.iso.org/idmp/AdministrationMethodClass">
        <rdf:type rdf:resource="https://purl.iso.org/datatypes/CD"/>
    </owl:NamedIndividual>
    


    <!-- https://purl.iso.org/idmp/BasicDoseForm -->

    <owl:NamedIndividual rdf:about="https://purl.iso.org/idmp/BasicDoseForm">
        <rdf:type rdf:resource="https://purl.iso.org/datatypes/CD"/>
    </owl:NamedIndividual>
    


    <!-- https://purl.iso.org/idmp/Code -->

    <owl:NamedIndividual rdf:about="https://purl.iso.org/idmp/Code">
        <rdf:type rdf:resource="https://purl.iso.org/datatypes/ST"/>
        <idmp:isUMLAttributeOf rdf:resource="https://purl.iso.org/idmp/CodeTermPair"/>
        <idmp:isUMLAttributeOf rdf:resource="https://purl.iso.org/idmp/CodedConcept"/>
        <idmp:isUMLAttributeOf rdf:resource="https://purl.iso.org/idmp/Versioning"/>
    </owl:NamedIndividual>
    


    <!-- https://purl.iso.org/idmp/CodeTermPair -->

    <owl:NamedIndividual rdf:about="https://purl.iso.org/idmp/CodeTermPair">
        <rdf:type rdf:resource="https://purl.iso.org/datatypes/ST"/>
        <skos:narrower rdf:resource="https://purl.iso.org/idmp/Code"/>
        <skos:narrower rdf:resource="https://purl.iso.org/idmp/Comment"/>
        <skos:narrower rdf:resource="https://purl.iso.org/idmp/Definition"/>
        <skos:narrower rdf:resource="https://purl.iso.org/idmp/Domain"/>
        <skos:narrower rdf:resource="https://purl.iso.org/idmp/LanguageCode"/>
        <skos:narrower rdf:resource="https://purl.iso.org/idmp/Term"/>
        <idmp:hasUMLAttribute rdf:resource="https://purl.iso.org/idmp/Code"/>
        <idmp:hasUMLAttribute rdf:resource="https://purl.iso.org/idmp/Comment"/>
        <idmp:hasUMLAttribute rdf:resource="https://purl.iso.org/idmp/Definition"/>
        <idmp:hasUMLAttribute rdf:resource="https://purl.iso.org/idmp/Domain"/>
        <idmp:hasUMLAttribute rdf:resource="https://purl.iso.org/idmp/LanguageCode"/>
        <idmp:hasUMLAttribute rdf:resource="https://purl.iso.org/idmp/RegionCode"/>
        <idmp:hasUMLAttribute rdf:resource="https://purl.iso.org/idmp/Term"/>
    </owl:NamedIndividual>
    


    <!-- https://purl.iso.org/idmp/CodedConcept -->

    <owl:NamedIndividual rdf:about="https://purl.iso.org/idmp/CodedConcept">
        <skos:narrower rdf:resource="https://purl.iso.org/idmp/CodeTermPair"/>
        <skos:narrower rdf:resource="https://purl.iso.org/idmp/Translation"/>
        <skos:narrower rdf:resource="https://purl.iso.org/idmp/code"/>
        <idmp:hasUMLAttribute rdf:resource="https://purl.iso.org/idmp/Code"/>
        <idmp:hasUMLAttribute rdf:resource="https://purl.iso.org/idmp/Translation"/>
        <idmp:hasUMLAttribute rdf:resource="https://purl.iso.org/idmp/Value"/>
    </owl:NamedIndividual>
    


    <!-- https://purl.iso.org/idmp/Comment -->

    <owl:NamedIndividual rdf:about="https://purl.iso.org/idmp/Comment">
        <rdf:type rdf:resource="https://purl.iso.org/datatypes/ST"/>
        <idmp:isUMLAttributeOf rdf:resource="https://purl.iso.org/idmp/CodeTermPair"/>
    </owl:NamedIndividual>
    


    <!-- https://purl.iso.org/idmp/ConceptStatus -->

    <owl:NamedIndividual rdf:about="https://purl.iso.org/idmp/ConceptStatus">
        <rdf:type rdf:resource="https://purl.iso.org/datatypes/CD"/>
    </owl:NamedIndividual>
    


    <!-- https://purl.iso.org/idmp/CreatedBy -->

    <owl:NamedIndividual rdf:about="https://purl.iso.org/idmp/CreatedBy">
        <rdf:type rdf:resource="https://purl.iso.org/datatypes/ST"/>
    </owl:NamedIndividual>
    


    <!-- https://purl.iso.org/idmp/CreationDate -->

    <owl:NamedIndividual rdf:about="https://purl.iso.org/idmp/CreationDate">
        <rdf:type rdf:resource="https://purl.iso.org/datatypes/TS"/>
    </owl:NamedIndividual>
    


    <!-- https://purl.iso.org/idmp/CurrentConcept -->

    <owl:NamedIndividual rdf:about="https://purl.iso.org/idmp/CurrentConcept"/>
    


    <!-- https://purl.iso.org/idmp/Definition -->

    <owl:NamedIndividual rdf:about="https://purl.iso.org/idmp/Definition">
        <rdf:type rdf:resource="https://purl.iso.org/datatypes/ST"/>
        <idmp:isUMLAttributeOf rdf:resource="https://purl.iso.org/idmp/CodeTermPair"/>
    </owl:NamedIndividual>
    


    <!-- https://purl.iso.org/idmp/Domain -->

    <owl:NamedIndividual rdf:about="https://purl.iso.org/idmp/Domain">
        <rdf:type rdf:resource="https://purl.iso.org/datatypes/CD"/>
        <idmp:isUMLAttributeOf rdf:resource="https://purl.iso.org/idmp/CodeTermPair"/>
    </owl:NamedIndividual>
    


    <!-- https://purl.iso.org/idmp/IntendedSiteClass -->

    <owl:NamedIndividual rdf:about="https://purl.iso.org/idmp/IntendedSiteClass">
        <rdf:type rdf:resource="https://purl.iso.org/datatypes/CD"/>
    </owl:NamedIndividual>
    


    <!-- https://purl.iso.org/idmp/LanguageCode -->

    <owl:NamedIndividual rdf:about="https://purl.iso.org/idmp/LanguageCode">
        <rdf:type rdf:resource="https://purl.iso.org/datatypes/CD"/>
        <idmp:isUMLAttributeOf rdf:resource="https://purl.iso.org/idmp/CodeTermPair"/>
    </owl:NamedIndividual>
    


    <!-- https://purl.iso.org/idmp/ModificationBy -->

    <owl:NamedIndividual rdf:about="https://purl.iso.org/idmp/ModificationBy">
        <rdf:type rdf:resource="https://purl.iso.org/datatypes/ST"/>
    </owl:NamedIndividual>
    


    <!-- https://purl.iso.org/idmp/ModificationDate -->

    <owl:NamedIndividual rdf:about="https://purl.iso.org/idmp/ModificationDate">
        <rdf:type rdf:resource="https://purl.iso.org/datatypes/TS"/>
        <idmp:isUMLAttributeOf rdf:resource="https://purl.iso.org/idmp/Versioning"/>
    </owl:NamedIndividual>
    


    <!-- https://purl.iso.org/idmp/ModificationMade -->

    <owl:NamedIndividual rdf:about="https://purl.iso.org/idmp/ModificationMade">
        <rdf:type rdf:resource="https://purl.iso.org/datatypes/ST"/>
    </owl:NamedIndividual>
    


    <!-- https://purl.iso.org/idmp/Packaging -->

    <owl:NamedIndividual rdf:about="https://purl.iso.org/idmp/Packaging">
        <rdf:type rdf:resource="https://purl.iso.org/datatypes/CD"/>
    </owl:NamedIndividual>
    


    <!-- https://purl.iso.org/idmp/PackagingCategoryClass -->

    <owl:NamedIndividual rdf:about="https://purl.iso.org/idmp/PackagingCategoryClass">
        <rdf:type rdf:resource="https://purl.iso.org/datatypes/CD"/>
    </owl:NamedIndividual>
    


    <!-- https://purl.iso.org/idmp/PackagingClass -->

    <owl:NamedIndividual rdf:about="https://purl.iso.org/idmp/PackagingClass">
        <rdf:type rdf:resource="https://purl.iso.org/datatypes/CD"/>
    </owl:NamedIndividual>
    


    <!-- https://purl.iso.org/idmp/PharmaceuticalDoseForm -->

    <owl:NamedIndividual rdf:about="https://purl.iso.org/idmp/PharmaceuticalDoseForm">
        <rdf:type rdf:resource="https://purl.iso.org/datatypes/CD"/>
    </owl:NamedIndividual>
    


    <!-- https://purl.iso.org/idmp/RegionCode -->

    <owl:NamedIndividual rdf:about="https://purl.iso.org/idmp/RegionCode">
        <rdf:type rdf:resource="https://purl.iso.org/datatypes/CD"/>
        <idmp:isUMLAttributeOf rdf:resource="https://purl.iso.org/idmp/CodeTermPair"/>
    </owl:NamedIndividual>
    


    <!-- https://purl.iso.org/idmp/ReleaseCharacteristics -->

    <owl:NamedIndividual rdf:about="https://purl.iso.org/idmp/ReleaseCharacteristics">
        <rdf:type rdf:resource="https://purl.iso.org/datatypes/CD"/>
    </owl:NamedIndividual>
    


    <!-- https://purl.iso.org/idmp/RouteOfAdministration -->

    <owl:NamedIndividual rdf:about="https://purl.iso.org/idmp/RouteOfAdministration">
        <rdf:type rdf:resource="https://purl.iso.org/datatypes/CD"/>
    </owl:NamedIndividual>
    


    <!-- https://purl.iso.org/idmp/StateOfMatter -->

    <owl:NamedIndividual rdf:about="https://purl.iso.org/idmp/StateOfMatter">
        <rdf:type rdf:resource="https://purl.iso.org/datatypes/CD"/>
    </owl:NamedIndividual>
    


    <!-- https://purl.iso.org/idmp/Term -->

    <owl:NamedIndividual rdf:about="https://purl.iso.org/idmp/Term">
        <rdf:type rdf:resource="https://purl.iso.org/datatypes/ST"/>
        <idmp:isUMLAttributeOf rdf:resource="https://purl.iso.org/idmp/CodeTermPair"/>
    </owl:NamedIndividual>
    


    <!-- https://purl.iso.org/idmp/TransformationClass -->

    <owl:NamedIndividual rdf:about="https://purl.iso.org/idmp/TransformationClass">
        <rdf:type rdf:resource="https://purl.iso.org/datatypes/CD"/>
    </owl:NamedIndividual>
    


    <!-- https://purl.iso.org/idmp/Translation -->

    <owl:NamedIndividual rdf:about="https://purl.iso.org/idmp/Translation">
        <rdf:type rdf:resource="https://purl.iso.org/datatypes/CodeTermPair"/>
        <idmp:isUMLAttributeOf rdf:resource="https://purl.iso.org/idmp/CodedConcept"/>
    </owl:NamedIndividual>
    


    <!-- https://purl.iso.org/idmp/UnitOfPresentation -->

    <owl:NamedIndividual rdf:about="https://purl.iso.org/idmp/UnitOfPresentation">
        <rdf:type rdf:resource="https://purl.iso.org/datatypes/CD"/>
    </owl:NamedIndividual>
    


    <!-- https://purl.iso.org/idmp/Value -->

    <owl:NamedIndividual rdf:about="https://purl.iso.org/idmp/Value">
        <rdf:type rdf:resource="https://purl.iso.org/datatypes/CodeTermPair"/>
        <idmp:isUMLAttributeOf rdf:resource="https://purl.iso.org/idmp/CodedConcept"/>
    </owl:NamedIndividual>
    


    <!-- https://purl.iso.org/idmp/VersionNumber -->

    <rdf:Description rdf:about="https://purl.iso.org/idmp/VersionNumber">
        <rdf:type rdf:resource="https://purl.iso.org/datatypes/INT"/>
        <idmp:isUMLAttributeOf rdf:resource="https://purl.iso.org/idmp/Versioning"/>
    </rdf:Description>
    


    <!-- https://purl.iso.org/idmp/Versioning -->

    <owl:NamedIndividual rdf:about="https://purl.iso.org/idmp/Versioning">
        <skos:narrower rdf:resource="https://purl.iso.org/idmp/Code"/>
        <skos:narrower rdf:resource="https://purl.iso.org/idmp/ConceptStatus"/>
        <skos:narrower rdf:resource="https://purl.iso.org/idmp/CreatedBy"/>
        <skos:narrower rdf:resource="https://purl.iso.org/idmp/CreationDate"/>
        <skos:narrower rdf:resource="https://purl.iso.org/idmp/CurrentConcept"/>
        <skos:narrower rdf:resource="https://purl.iso.org/idmp/ModificationBy"/>
        <skos:narrower rdf:resource="https://purl.iso.org/idmp/ModificationDate"/>
        <skos:narrower rdf:resource="https://purl.iso.org/idmp/ModificationMade"/>
        <skos:narrower rdf:resource="https://purl.iso.org/idmp/VersionNumber"/>
        <idmp:hasUMLAttribute rdf:resource="https://purl.iso.org/idmp/Code"/>
        <idmp:hasUMLAttribute rdf:resource="https://purl.iso.org/idmp/ConceptStatus"/>
        <idmp:hasUMLAttribute rdf:resource="https://purl.iso.org/idmp/CreatedBy"/>
        <idmp:hasUMLAttribute rdf:resource="https://purl.iso.org/idmp/CreationDate"/>
        <idmp:hasUMLAttribute rdf:resource="https://purl.iso.org/idmp/ModificationBy"/>
        <idmp:hasUMLAttribute rdf:resource="https://purl.iso.org/idmp/ModificationDate"/>
        <idmp:hasUMLAttribute rdf:resource="https://purl.iso.org/idmp/ModificationMade"/>
        <idmp:hasUMLAttribute rdf:resource="https://purl.iso.org/idmp/VersionNumber"/>
        <idmp:hasUMLAttribute rdf:resource="https://purl.iso.org/idmp/currentConcept"/>
    </owl:NamedIndividual>
    


    <!-- https://purl.iso.org/idmp/code -->

    <owl:NamedIndividual rdf:about="https://purl.iso.org/idmp/code"/>
    


    <!-- https://purl.iso.org/idmp/currentConcept -->

    <owl:NamedIndividual rdf:about="https://purl.iso.org/idmp/currentConcept"/>
    


    <!-- 
    ///////////////////////////////////////////////////////////////////////////////////////
    //
    // Annotations
    //
    ///////////////////////////////////////////////////////////////////////////////////////
     -->

    <rdf:Description rdf:about="https://purl.iso.org/idmp/AdministrationMethodClass">
        <terms:source>ISO/TS 11239:2012(E) page 12</terms:source>
        <terms:source rdf:resource="https://purl.iso.org/idmp/iso-11239/2012E"/>
        <skos:prefLabel>administration method class</skos:prefLabel>
        <skos:definition>The administration method class shall be used to describe the pharmaceutical dose form according to the general intended method by which it is to be administered to the body. It describes a set of high-level general terms expressly for describing the intended administration method for a pharmaceutical dose form, rather than a specialized vocabulary detailing precise methods of administration. Where there is no administration method associated, the class has an appropriate null value. An administration method is associated with zero to many pharmaceutical dose forms.</skos:definition>
        <skos:example>Application, inhalation, injection, none. See also Annex A (Table A.5) for controlled vocabulary examples, and Annex B for medicinal product examples.</skos:example>
    </rdf:Description>
    <rdf:Description rdf:about="https://purl.iso.org/idmp/BasicDoseForm">
        <terms:source>ISO/TS 11239:2012(E) page 11</terms:source>
        <terms:source rdf:resource="https://purl.iso.org/idmp/iso-11239/2012E"/>
        <skos:definition>The basic dose form class shall be used as the high-level grouping category that classes the pharmaceutical dose form according to its general type of pharmaceutical dose form. A basic dose form has zero to many pharmaceutical dose forms.</skos:definition>
        <terms:source>ISO/TS 11239:2012(E) page 2</terms:source>
        <skos:prefLabel>basic dose form</skos:prefLabel>
        <skos:example>Tablet, capsule, powder, solution. See also Annex A (Table A.1) for controlled vocabulary examples, and Annex B for medicinal product examples.</skos:example>
    </rdf:Description>
    <rdf:Description rdf:about="https://purl.iso.org/idmp/Code">
        <skos:prefLabel>code</skos:prefLabel>
        <skos:definition>the unique (machine-processable) identifier for the codedConcept</skos:definition>
        <terms:source rdf:resource="https://purl.iso.org/idmp/iso-11239/2012E"/>
        <skos:definition>the unique (machine-processable) identifier for the concept that is the subject of the versioning</skos:definition>
        <terms:source>ISO/TS 11239:2012(E) page 8</terms:source>
        <skos:definition>a unique (machine-processable) identifier for the codeTermPair (data type: ST)</skos:definition>
        <idmp:conformance rdf:resource="https://purl.iso.org/idmp/MandatoryInformation"/>
        <terms:source>ISO/TS 11239:2012(E) page 9</terms:source>
    </rdf:Description>
    <rdf:Description rdf:about="https://purl.iso.org/idmp/CodeTermPair">
        <terms:source>ISO/TS 11239:2012(E) page 8</terms:source>
        <terms:source rdf:resource="https://purl.iso.org/idmp/iso-11239/2012E"/>
        <skos:prefLabel>code term pair</skos:prefLabel>
        <idmp:conformance rdf:resource="https://purl.iso.org/idmp/MandatoryInformation"/>
        <skos:definition>The codeTermPair shall be used as the underlying class that carries the base code, the associated text string and other elements of definition, and will be used as a data type in the creation of the codedConcept. Data type that groups together the attributes required to describe a single concept in a specified language and for a specified geographical location.</skos:definition>
        <terms:source>ISO/TS 11239:2012(E) page 2</terms:source>
    </rdf:Description>
    <rdf:Description rdf:about="https://purl.iso.org/idmp/CodedConcept">
        <terms:source>ISO/TS 11239:2012(E) page 2</terms:source>
        <skos:definition>The codedConcept associates a concept for a selected language and geographical region (e.g. in English for the UK) with zero to many translations of that same concept for different languages and/or geographical regions (e.g. in French for France, in German for Germany). The codeTermPair code for the concept for the user-selected language and region is used for the “value” element, and zero to many codeTermPair codes for that same concept for different languages and/or regions are used for the “translation” element; together these define the codedConcept data type. Data type that groups together a set of code term pairs that represent a single concept but differ in language and/or geographical region.</skos:definition>
        <skos:note>The coded concept is used to manage translations, and it is the basic data type that is found in all of the high-level conceptual models.</skos:note>
        <skos:prefLabel>coded concept</skos:prefLabel>
        <terms:source rdf:resource="https://purl.iso.org/idmp/iso-11239/2012E"/>
        <terms:source>ISO/TS 11239:2012(E) page 8</terms:source>
    </rdf:Description>
    <rdf:Description rdf:about="https://purl.iso.org/idmp/Comment">
        <skos:prefLabel>comment</skos:prefLabel>
        <skos:definition>An optional textual comment.</skos:definition>
        <idmp:conformance rdf:resource="https://purl.iso.org/idmp/MandatoryInformation"/>
        <terms:source>ISO/TS 11239:2012(E) page 8</terms:source>
        <terms:source rdf:resource="https://purl.iso.org/idmp/iso-11239/2012E"/>
    </rdf:Description>
    <rdf:Description rdf:about="https://purl.iso.org/idmp/ConceptStatus">
        <skos:definition>the status of the concept, i.e. whether it is current, deprecated, etc.</skos:definition>
        <idmp:isUMLAttributeOf rdf:resource="https://purl.iso.org/idmp/Versioning"/>
        <terms:source>ISO/TS 11239:2012(E) page 9</terms:source>
        <terms:source rdf:resource="https://purl.iso.org/idmp/iso-11239/2012E"/>
        <skos:prefLabel>concept status</skos:prefLabel>
    </rdf:Description>
    <rdf:Description rdf:about="https://purl.iso.org/idmp/CreatedBy">
        <skos:prefLabel>created by</skos:prefLabel>
        <idmp:isUMLAttributeOf rdf:resource="https://purl.iso.org/idmp/Versioning"/>
        <terms:source>ISO/TS 11239:2012(E) page 9</terms:source>
        <skos:definition>information to identify the person who created the concept</skos:definition>
        <terms:source rdf:resource="https://purl.iso.org/idmp/iso-11239/2012E"/>
    </rdf:Description>
    <rdf:Description rdf:about="https://purl.iso.org/idmp/CreationDate">
        <skos:prefLabel>creation date</skos:prefLabel>
        <skos:definition>a time stamp indicating the date and time that the concept was created</skos:definition>
        <terms:source>ISO/TS 11239:2012(E) page 9</terms:source>
        <terms:source rdf:resource="https://purl.iso.org/idmp/iso-11239/2012E"/>
        <idmp:isUMLAttributeOf rdf:resource="https://purl.iso.org/idmp/Versioning"/>
    </rdf:Description>
    <rdf:Description rdf:about="https://purl.iso.org/idmp/Definition">
        <skos:definition>A textual definition for the concept.</skos:definition>
        <terms:source rdf:resource="https://purl.iso.org/idmp/iso-11239/2012E"/>
        <terms:source>ISO/TS 11239:2012(E) page 8</terms:source>
        <skos:prefLabel>definition</skos:prefLabel>
        <idmp:conformance rdf:resource="https://purl.iso.org/idmp/MandatoryInformation"/>
    </rdf:Description>
    <rdf:Description rdf:about="https://purl.iso.org/idmp/Domain">
        <skos:prefLabel>domain</skos:prefLabel>
        <terms:source>ISO/TS 11239:2012(E) page 8</terms:source>
        <skos:definition>an optional indicator for use where veterinary-only terms are also provided in the same database, indicates that the concept is for either “human and veterinary” or “veterinary only” use (default value is “human and veterinary”)</skos:definition>
        <terms:source rdf:resource="https://purl.iso.org/idmp/iso-11239/2012E"/>
        <idmp:conformance rdf:resource="https://purl.iso.org/idmp/MandatoryInformation"/>
    </rdf:Description>
    <rdf:Description rdf:about="https://purl.iso.org/idmp/IntendedSiteClass">
        <skos:prefLabel>intended site class</skos:prefLabel>
        <terms:source>ISO/TS 11239:2012(E) page 12</terms:source>
        <skos:definition>The intended site class shall be used to describe the general body site at which the pharmaceutical dose form is intended to be administered. It is a set of high-level general terms expressly for describing the intended site, rather than a specialized vocabulary detailing precise sites of administration. It is not the same concept as route of administration. Where there is no intended site associated, the class has an appropriate null value. An intended site is associated with zero to many pharmaceutical dose forms.</skos:definition>
        <terms:source rdf:resource="https://purl.iso.org/idmp/iso-11239/2012E"/>
        <skos:example>Auricular, ocular, oral, none. See also Annex A (Table A.4) for controlled vocabulary examples, and Annex B for medicinal product examples.</skos:example>
        <idmp:conformance rdf:resource="https://purl.iso.org/idmp/MandatoryInformation"/>
    </rdf:Description>
    <rdf:Description rdf:about="https://purl.iso.org/idmp/LanguageCode">
        <terms:source>ISO/TS 11239:2012(E) page 8</terms:source>
        <skos:definition>The language used to describe term, definition, domain and comment, in accordance with ISO 639.</skos:definition>
        <terms:source rdf:resource="https://purl.iso.org/idmp/iso-11239/2012E"/>
        <skos:prefLabel>language code</skos:prefLabel>
        <idmp:conformance rdf:resource="https://purl.iso.org/idmp/MandatoryInformation"/>
    </rdf:Description>
    <rdf:Description rdf:about="https://purl.iso.org/idmp/ModificationBy">
        <skos:definition>information to identify the person who modified the concept</skos:definition>
        <idmp:isUMLAttributeOf rdf:resource="https://purl.iso.org/idmp/Versioning"/>
        <terms:source>ISO/TS 11239:2012(E) page 9</terms:source>
        <terms:source rdf:resource="https://purl.iso.org/idmp/iso-11239/2012E"/>
        <skos:prefLabel>modification by</skos:prefLabel>
    </rdf:Description>
    <rdf:Description rdf:about="https://purl.iso.org/idmp/ModificationDate">
        <terms:source rdf:resource="https://purl.iso.org/idmp/iso-11239/2012E"/>
        <terms:source>ISO/TS 11239:2012(E) page 9</terms:source>
        <skos:prefLabel>modification date</skos:prefLabel>
        <skos:definition>a time stamp indicating the date and time that the modification was made for the specified version</skos:definition>
    </rdf:Description>
    <rdf:Description rdf:about="https://purl.iso.org/idmp/ModificationMade">
        <skos:prefLabel>modification made</skos:prefLabel>
        <skos:definition>a description in free text of the modification made for the specified version</skos:definition>
        <terms:source rdf:resource="https://purl.iso.org/idmp/iso-11239/2012E"/>
        <terms:source>ISO/TS 11239:2012(E) page 9</terms:source>
        <idmp:isUMLAttributeOf rdf:resource="https://purl.iso.org/idmp/Versioning"/>
    </rdf:Description>
    <rdf:Description rdf:about="https://purl.iso.org/idmp/Packaging">
        <idmp:conformance rdf:resource="https://purl.iso.org/idmp/MandatoryInformation"/>
        <skos:prefLabel>packaging</skos:prefLabel>
        <terms:source>ISO/TS 11239:2012(E) page 15</terms:source>
        <skos:definition>The packaging concept is a group of three concepts that describe particular elements of the medicinal product: container, closure and administration device.</skos:definition>
        <terms:source rdf:resource="https://purl.iso.org/idmp/iso-11239/2012E"/>
    </rdf:Description>
    <rdf:Description rdf:about="https://purl.iso.org/idmp/PackagingCategoryClass">
        <terms:source>ISO/TS 11239:2012(E) page 15</terms:source>
        <skos:definition>The packaging category class shall be used as the high-level grouping category that classes the packaging concept according to the general category of packaging into which it falls, namely: container, closure and administration device. A packaging category has zero to many types of packaging. The packaging category class shall be described using a codedConcept.</skos:definition>
        <skos:prefLabel>packaging category class</skos:prefLabel>
        <idmp:conformance rdf:resource="https://purl.iso.org/idmp/MandatoryInformation"/>
        <terms:source rdf:resource="https://purl.iso.org/idmp/iso-11239/2012E"/>
    </rdf:Description>
    <rdf:Description rdf:about="https://purl.iso.org/idmp/PackagingClass">
        <terms:source>ISO/TS 11239:2012(E) page 8</terms:source>
        <idmp:conformance rdf:resource="https://purl.iso.org/idmp/MandatoryInformation"/>
        <skos:example>EXAMPLE 1 For the container: ampoule, blister, bottle, tube, box, carton. See also Annex A (Table A.10) for controlled vocabulary examples, and Annex B for medicinal product examples. EXAMPLE 2 For the closure: cap, screw-cap, stopper. See also Annex A (Table A.10) for controlled vocabulary examples, and Annex B for medicinal product examples. EXAMPLE 3 For the administration device: needle, oral syringe. See also Annex A (Table A.10) for controlled vocabulary examples, and Annex B for medicinal product examples.</skos:example>
        <skos:definition>The packaging class shall be used to specify the attributes that are needed to define properly the container, closure, or administration device concept. A packaging has one packaging category.</skos:definition>
        <terms:source rdf:resource="https://purl.iso.org/idmp/iso-11239/2012E"/>
        <skos:prefLabel>packaging class</skos:prefLabel>
    </rdf:Description>
    <rdf:Description rdf:about="https://purl.iso.org/idmp/PharmaceuticalDoseForm">
        <skos:prefLabel>pharmaceutical dose form</skos:prefLabel>
        <terms:source rdf:resource="https://purl.iso.org/idmp/iso-11239/2012E"/>
        <terms:source>ISO/TS 11239:2012(E) page 4</terms:source>
        <idmp:conformance rdf:resource="https://purl.iso.org/idmp/MandatoryInformation"/>
        <skos:note>“Pharmaceutical dose form” can refer to the administrable dose form or the manufactured dose form, depending on the product that it is describing.</skos:note>
        <skos:definition>The pharmaceutical dose form is built from a set of basic dose forms, which are in turn grouped according to state of matter. Each pharmaceutical dose form is associated with attributes that describe any release characteristics, any transformation that is required to be carried out before administration, the intended site of administration, and the intended method of administration. The pharmaceutical dose form concept and its attributes are described using the codedConcept datatype, thereby incorporating the translated concepts. Physical manifestation of a product that contains the active ingredient(s) and/or inactive ingredient(s) that are intended to be delivered to the patient.</skos:definition>
        <terms:source>ISO/TS 11239:2012(E) page 11</terms:source>
    </rdf:Description>
    <rdf:Description rdf:about="https://purl.iso.org/idmp/RegionCode">
        <idmp:conformance rdf:resource="https://purl.iso.org/idmp/MandatoryInformation"/>
        <terms:source rdf:resource="https://purl.iso.org/idmp/iso-11239/2012E"/>
        <skos:definition>The country/region that uses this codeTermPair in this language, in accordance with ISO 3166.</skos:definition>
        <skos:prefLabel>region code</skos:prefLabel>
        <terms:source>ISO/TS 11239:2012(E) page 8</terms:source>
    </rdf:Description>
    <rdf:Description rdf:about="https://purl.iso.org/idmp/ReleaseCharacteristics">
        <terms:source rdf:resource="https://purl.iso.org/idmp/iso-11239/2012E"/>
        <terms:source>ISO/TS 11239:2012(E) page 12</terms:source>
        <skos:prefLabel>release characteristics</skos:prefLabel>
        <skos:definition>The release characteristics class shall be used to describe the release characteristics of the pharmaceutical dose form. Where there are no release characteristics to be specified, the class has an appropriate null value. A release characteristic is associated with zero to many pharmaceutical dose forms.</skos:definition>
        <skos:example>Delayed, extended, pulsatile, none. See also Annex A (Table A.2) for controlled vocabulary examples, and Annex B for medicinal product examples.</skos:example>
    </rdf:Description>
    <rdf:Description rdf:about="https://purl.iso.org/idmp/RouteOfAdministration">
        <terms:source>ISO/TS 11239:2012(E) page 15</terms:source>
        <skos:prefLabel>route of administration</skos:prefLabel>
        <skos:definition>The route of administration is a concept that is used to describe the path by which the pharmaceutical product is taken into or makes contact with the body.</skos:definition>
        <terms:source rdf:resource="https://purl.iso.org/idmp/iso-11239/2012E"/>
    </rdf:Description>
    <rdf:Description rdf:about="https://purl.iso.org/idmp/StateOfMatter">
        <terms:source rdf:resource="https://purl.iso.org/idmp/iso-11239/2012E"/>
        <skos:prefLabel>state of matter</skos:prefLabel>
        <terms:source>ISO/TS 11239:2012(E) page 11</terms:source>
        <terms:source>ISO/TS 11239:2012(E) page 5</terms:source>
        <skos:definition>The state of matter class shall be used as the high-level grouping category that classes the pharmaceutical dose form, via the basic dose form, according to its state of matter attribute. A state of matter class has zero to many basic dose forms.</skos:definition>
        <skos:example>Solid, semi-solid, liquid, gas. See also Annex A (Table A.1) for controlled vocabulary examples, and Annex B for medicinal product examples.</skos:example>
        <skos:note>State of matter is used to group basic dose forms according to their physical properties.</skos:note>
    </rdf:Description>
    <rdf:Description rdf:about="https://purl.iso.org/idmp/Term">
        <skos:prefLabel>term</skos:prefLabel>
        <terms:source rdf:resource="https://purl.iso.org/idmp/iso-11239/2012E"/>
        <terms:source>ISO/TS 11239:2012(E) page 8</terms:source>
        <skos:definition>The textual term description for the concept.</skos:definition>
        <idmp:conformance rdf:resource="https://purl.iso.org/idmp/MandatoryInformation"/>
    </rdf:Description>
    <rdf:Description rdf:about="https://purl.iso.org/idmp/TransformationClass">
        <terms:source rdf:resource="https://purl.iso.org/idmp/iso-11239/2012E"/>
        <terms:source>ISO/TS 11239:2012(E) page 12</terms:source>
        <skos:prefLabel>transformation class</skos:prefLabel>
        <skos:definition>The transformation class shall be used to describe the physical operation that is required in order to convert a manufactured dose form into an administrable dose form, where this is necessary. Where there is no transformation, the class has an appropriate null value. A transformation is associated with zero to many pharmaceutical dose forms.</skos:definition>
        <idmp:conformance rdf:resource="https://purl.iso.org/idmp/MandatoryInformation"/>
        <skos:example>Dilution, dissolution, none. See also Annex A (Table A.3) for controlled vocabulary examples, and Annex B for medicinal product examples.</skos:example>
    </rdf:Description>
    <rdf:Description rdf:about="https://purl.iso.org/idmp/Translation">
        <terms:source>ISO/TS 11239:2012(E) page 9</terms:source>
        <terms:source rdf:resource="https://purl.iso.org/idmp/iso-11239/2012E"/>
        <skos:prefLabel>translation</skos:prefLabel>
        <skos:definition>zero to many codeTermPair codes for the same concept with different language and/or region codes (e.g. French and France, German and Germany)</skos:definition>
        <idmp:conformance rdf:resource="https://purl.iso.org/idmp/MandatoryInformation"/>
    </rdf:Description>
    <rdf:Description rdf:about="https://purl.iso.org/idmp/UnitOfPresentation">
        <skos:prefLabel>unit of presentation</skos:prefLabel>
        <idmp:conformance rdf:resource="https://purl.iso.org/idmp/MandatoryInformation"/>
        <terms:source>ISO/TS 11239:2012(E) page 14</terms:source>
        <terms:source rdf:resource="https://purl.iso.org/idmp/iso-11239/2012E"/>
        <skos:definition>The unit of presentation is a concept that is used in describing the qualitative unit in which the strength or quantity of the manufactured item or pharmaceutical product are presented and described, in cases where a quantitative unit of measurement is not applicable. It is used where the strength may be described in terms of “each” in a general manner; in such a case, “each” would be replaced by “per tablet”, “per puff”, “per patch”, etc. It is also used where the strength or total quantity of a manufactured item or pharmaceutical product is described in terms of the packaging, such as “100 ml per bottle”.</skos:definition>
    </rdf:Description>
    <rdf:Description rdf:about="https://purl.iso.org/idmp/Value">
        <terms:source rdf:resource="https://purl.iso.org/idmp/iso-11239/2012E"/>
        <skos:prefLabel>value</skos:prefLabel>
        <skos:definition>the codeTermPair code for the concept that has the user-selected language code (e.g. English) and user-selected region code (e.g. UK)</skos:definition>
        <terms:source>ISO/TS 11239:2012(E) page 8</terms:source>
    </rdf:Description>
    <rdf:Description rdf:about="https://purl.iso.org/idmp/VersionNumber">
        <terms:source>ISO/TS 11239:2012(E) page 9</terms:source>
        <terms:source rdf:resource="https://purl.iso.org/idmp/iso-11239/2012E"/>
        <skos:definition>A number that indicates the version of the concept.</skos:definition>
        <skos:prefLabel>version number</skos:prefLabel>
    </rdf:Description>
    <rdf:Description rdf:about="https://purl.iso.org/idmp/Versioning">
        <terms:source rdf:resource="https://purl.iso.org/idmp/iso-11239/2012E"/>
        <skos:prefLabel>versioning</skos:prefLabel>
        <skos:definition>Versioning provides a traceable history for each concept from the point of creation of the concept, including details of all modifications thereafter.</skos:definition>
        <terms:source>ISO/TS 11239:2012(E) page 9</terms:source>
    </rdf:Description>
    <rdf:Description rdf:about="https://purl.iso.org/idmp/currentConcept">
        <terms:source rdf:resource="https://purl.iso.org/idmp/iso-11239/2012E"/>
        <terms:source>ISO/TS 11239:2012(E) page 9</terms:source>
        <skos:definition>when a concept is deprecated, the code of the concept that replaces it. There may be more than one replacement concept for a single deprecated concept</skos:definition>
        <skos:prefLabel>current concept</skos:prefLabel>
        <idmp:conformance rdf:resource="https://purl.iso.org/idmp/MandatoryInformation"/>
        <idmp:isUMLAttributeOf rdf:resource="https://purl.iso.org/idmp/Versioning"/>
    </rdf:Description>
</rdf:RDF>



<!-- Generated by the OWL API (version 4.5.9.2019-02-01T07:24:44Z) https://github.com/owlcs/owlapi -->

