<?xml version="1.0" encoding="UTF-8"?>
<!DOCTYPE rdf:RDF [
	<!ENTITY dct "http://purl.org/dc/terms/">
	<!ENTITY idmp "https://spec.pistoiaalliance.org/idmp/ontology/ISO/ISO11615-MedicinalProducts/">
	<!ENTITY owl "http://www.w3.org/2002/07/owl#">
	<!ENTITY rdf "http://www.w3.org/1999/02/22-rdf-syntax-ns#">
	<!ENTITY rdfs "http://www.w3.org/2000/01/rdf-schema#">
	<!ENTITY skos "http://www.w3.org/2004/02/skos/core#">
	<!ENTITY upper "https://data-qa.novartis.net/r1/enterprise/datastrategy/upperontology/v1/">
	<!ENTITY xsd "http://www.w3.org/2001/XMLSchema#">
]>
<rdf:RDF xml:base="https://spec.pistoiaalliance.org/idmp/ontology/ISO/ISO11615-MedicinalProducts/iso-11615"
	xmlns="https://spec.pistoiaalliance.org/idmp/ontology/ISO/ISO11615-MedicinalProducts/iso-11615#"
	xmlns:dct="http://purl.org/dc/terms/"
	xmlns:idmp="https://spec.pistoiaalliance.org/idmp/ontology/ISO/ISO11615-MedicinalProducts/"
	xmlns:owl="http://www.w3.org/2002/07/owl#"
	xmlns:rdf="http://www.w3.org/1999/02/22-rdf-syntax-ns#"
	xmlns:rdfs="http://www.w3.org/2000/01/rdf-schema#"
	xmlns:skos="http://www.w3.org/2004/02/skos/core#"
	xmlns:upper="https://data-qa.novartis.net/r1/enterprise/datastrategy/upperontology/v1/"
	xmlns:xsd="http://www.w3.org/2001/XMLSchema#">
	
	<owl:Ontology rdf:about="&idmp;iso-11615">
		<rdfs:comment>Open Source - exact license to be clarified</rdfs:comment>
		<dct:date rdf:datatype="&xsd;date">2020-11-05</dct:date>
		<dct:modified rdf:datatype="&xsd;date">2022-04-11</dct:modified>
		<dct:title>IMDP Ontology - Product module.</dct:title>
		<owl:imports rdf:resource="&idmp;core"/>
		<owl:versionIRI rdf:resource="https://purl.iso.org/idmp/iso-11615/0.1"/>
		<owl:versionInfo>0.1</owl:versionInfo>
	</owl:Ontology>
	
	<owl:AnnotationProperty rdf:about="&dct;date">
	</owl:AnnotationProperty>
	
	<owl:AnnotationProperty rdf:about="&dct;modified">
	</owl:AnnotationProperty>
	
	<owl:AnnotationProperty rdf:about="&dct;source">
	</owl:AnnotationProperty>
	
	<owl:AnnotationProperty rdf:about="&dct;title">
	</owl:AnnotationProperty>
	
	<owl:Class rdf:about="&skos;Concept">
	</owl:Class>
	
	<owl:AnnotationProperty rdf:about="&skos;altLabel">
	</owl:AnnotationProperty>
	
	<owl:AnnotationProperty rdf:about="&skos;definition">
	</owl:AnnotationProperty>
	
	<owl:AnnotationProperty rdf:about="&skos;example">
	</owl:AnnotationProperty>
	
	<owl:AnnotationProperty rdf:about="&skos;prefLabel">
	</owl:AnnotationProperty>
	
	<owl:AnnotationProperty rdf:about="&skos;related">
	</owl:AnnotationProperty>
	
	<owl:Class rdf:about="&upper;DataAttribute">
	</owl:Class>
	
	<owl:Class rdf:about="&upper;DataObject">
	</owl:Class>
	
	<owl:Class rdf:about="&upper;LogicalDataEntity">
	</owl:Class>
	
	<owl:NamedIndividual rdf:about="&idmp;IMPIDAttributeSet">
		<rdf:type rdf:resource="&owl;Class"/>
		<rdf:type rdf:resource="&skos;Concept"/>
		<rdf:type rdf:resource="&upper;DataObject"/>
		<rdf:type rdf:resource="&upper;LogicalDataEntity"/>
		<rdfs:subClassOf rdf:resource="&skos;Concept"/>
		<skos:altLabel>IDMP.IMPIDAttributeSet</skos:altLabel>
		<skos:definition>A set of attributes which when they have a value define a specific MPID concept. Some of the attributes are defining attributes and, if present a change will result in a change in MPID. Other attributes are optional and changes to the values of these will NOT result in a new MPID.</skos:definition>
		<skos:prefLabel>Impid attribute set</skos:prefLabel>
		<idmp:hasUMLAttribute rdf:resource="&idmp;IMPIDAttributeSet.IMPID"/>
		<idmp:hasUMLAttribute rdf:resource="&idmp;IMPIDAttributeSet.productClassification"/>
		<idmp:hasUMLAttribute rdf:resource="&idmp;IMPIDAttributeSet.protocolNumber"/>
	</owl:NamedIndividual>
	
	<owl:NamedIndividual rdf:about="&idmp;IMPIDAttributeSet.IMPID">
		<rdf:type rdf:resource="&skos;Concept"/>
		<rdf:type rdf:resource="&upper;DataAttribute"/>
		<rdf:type rdf:resource="&upper;LogicalDataEntity"/>
		<skos:altLabel>IDMP.IMPIDAttributeSet.IMPID</skos:altLabel>
		<skos:definition>Investigational Medicinal Product Identifier</skos:definition>
		<skos:prefLabel>Impid</skos:prefLabel>
		<idmp:isUMLAttributeOf rdf:resource="&idmp;IMPIDAttributeSet"/>
	</owl:NamedIndividual>
	
	<owl:NamedIndividual rdf:about="&idmp;IMPIDAttributeSet.productClassification">
		<rdf:type rdf:resource="&skos;Concept"/>
		<rdf:type rdf:resource="&upper;DataAttribute"/>
		<rdf:type rdf:resource="&upper;LogicalDataEntity"/>
		<skos:altLabel>IDMP.IMPIDAttributeSet.productClassification</skos:altLabel>
		<skos:definition>If the investigational medicinal product designated in the indication(s) as an orphan drug this shall be set to the value or values of the orphan drug designation reference number(s) within the Product Classification.</skos:definition>
		<skos:prefLabel>Product classification</skos:prefLabel>
		<idmp:isUMLAttributeOf rdf:resource="&idmp;IMPIDAttributeSet"/>
	</owl:NamedIndividual>
	
	<owl:NamedIndividual rdf:about="&idmp;IMPIDAttributeSet.protocolNumber">
		<rdf:type rdf:resource="&skos;Concept"/>
		<rdf:type rdf:resource="&upper;DataAttribute"/>
		<rdf:type rdf:resource="&upper;LogicalDataEntity"/>
		<skos:altLabel>IDMP.IMPIDAttributeSet.protocolNumber</skos:altLabel>
		<skos:definition>The number assigned to the clinical trial protocol shall be specified.</skos:definition>
		<skos:prefLabel>Protocol number</skos:prefLabel>
		<idmp:isUMLAttributeOf rdf:resource="&idmp;IMPIDAttributeSet"/>
	</owl:NamedIndividual>
	
	<owl:NamedIndividual rdf:about="&idmp;IPCIDAttributeSet">
		<rdf:type rdf:resource="&owl;Class"/>
		<rdf:type rdf:resource="&skos;Concept"/>
		<rdf:type rdf:resource="&upper;DataObject"/>
		<rdf:type rdf:resource="&upper;LogicalDataEntity"/>
		<rdfs:subClassOf rdf:resource="&skos;Concept"/>
		<skos:altLabel>IDMP.IPCIDAttributeSet</skos:altLabel>
		<skos:definition>Unique identifier allocated to an investigational medicinal product at package level supplementary to any existing identifier as ascribed by a medicines regulatory authority in a jurisdiction or a sponsor of a clinical trial. This is for indexing purposes and to contribute to improving patient safety by allowing for the unique identification of medicinal products worldwide.</skos:definition>
		<skos:prefLabel>Ipcid attribute set</skos:prefLabel>
		<skos:related rdf:resource="&idmp;IMPIDAttributeSet"/>
		<idmp:hasUMLAttribute rdf:resource="&idmp;IPCIDAttributeSet.IPCID"/>
	</owl:NamedIndividual>
	
	<owl:NamedIndividual rdf:about="&idmp;IPCIDAttributeSet.IPCID">
		<rdf:type rdf:resource="&skos;Concept"/>
		<rdf:type rdf:resource="&upper;DataAttribute"/>
		<rdf:type rdf:resource="&upper;LogicalDataEntity"/>
		<skos:altLabel>IDMP.IPCIDAttributeSet.IPCID</skos:altLabel>
		<skos:definition>Unique identifier allocated to an investigational medicinal product at package level supplementary to any existing identifier as ascribed by a medicines regulatory authority in a jurisdiction or a sponsor of a clinical trialNOTE This is for indexing purposes and to contribute to improving patient safety by allowing for the unique identification of medicinal products worldwide.</skos:definition>
		<skos:prefLabel>Ipcid</skos:prefLabel>
		<idmp:isUMLAttributeOf rdf:resource="&idmp;IPCIDAttributeSet"/>
	</owl:NamedIndividual>
	
	<owl:NamedIndividual rdf:about="&idmp;Ingredient">
		<rdf:type rdf:resource="&owl;Class"/>
		<rdf:type rdf:resource="&skos;Concept"/>
		<rdf:type rdf:resource="&upper;DataObject"/>
		<rdf:type rdf:resource="&upper;LogicalDataEntity"/>
		<rdfs:subClassOf rdf:resource="&skos;Concept"/>
		<dct:source>ISO IDMP 11615:2017</dct:source>
		<skos:altLabel>IDMP.Ingredient</skos:altLabel>
		<skos:definition>IngredientThis subclause specifies information on all the active ingredients, adjuvants and excipients present in the Investigational Medicinal Products.</skos:definition>
		<skos:prefLabel>Ingredient</skos:prefLabel>
		<skos:related rdf:resource="&idmp;manufacturedItem"/>
		<skos:related rdf:resource="&idmp;medicalDevice"/>
		<skos:related rdf:resource="&idmp;pharmaceuticalProduct"/>
	</owl:NamedIndividual>
	
	<owl:NamedIndividual rdf:about="&idmp;InvestigationalMedicinalProductName.code">
		<rdf:type rdf:resource="&skos;Concept"/>
		<rdf:type rdf:resource="&upper;DataAttribute"/>
		<rdf:type rdf:resource="&upper;LogicalDataEntity"/>
		<skos:altLabel>IDMP.InvestigationalMedicinalProductName.code</skos:altLabel>
		<skos:definition>If the sponsor has assigned a code to the IMP for the purpose of the trial the code value shall be specified.</skos:definition>
		<skos:prefLabel>Investigational medicinal product code</skos:prefLabel>
		<idmp:isUMLAttributeOf rdf:resource="&idmp;investigationalMedicinalProductName"/>
	</owl:NamedIndividual>
	
	<owl:NamedIndividual rdf:about="&idmp;InvestigationalMedicinalProductName.containerPart">
		<rdf:type rdf:resource="&skos;Concept"/>
		<rdf:type rdf:resource="&upper;DataAttribute"/>
		<rdf:type rdf:resource="&upper;LogicalDataEntity"/>
		<skos:altLabel>IDMP.InvestigationalMedicinalProductName.containerPart</skos:altLabel>
		<skos:definition>The container, if reflected in the medicinal product name, shall be specified.EXAMPLE For the medicinal product name ‘LXA – 10 mg/ ml - Solution for injection – Subcutaneous use - Vial (glass) - 4 ml - 1 Vial’, the container part is ‘vial (glass)’.</skos:definition>
		<skos:prefLabel>Container part</skos:prefLabel>
		<idmp:isUMLAttributeOf rdf:resource="&idmp;investigationalMedicinalProductName"/>
	</owl:NamedIndividual>
	
	<owl:NamedIndividual rdf:about="&idmp;InvestigationalMedicinalProductName.devicePart">
		<rdf:type rdf:resource="&skos;Concept"/>
		<rdf:type rdf:resource="&upper;DataAttribute"/>
		<rdf:type rdf:resource="&upper;LogicalDataEntity"/>
		<skos:altLabel>IDMP.InvestigationalMedicinalProductName.devicePart</skos:altLabel>
		<skos:definition>The device, if reflected in the medicinal product name, shall be specified.EXAMPLE For the medicinal product name ‘LXA ‘Drug XYZ® Accuhaler 200 mg for adults’, the device part is ‘Accuhaler’.</skos:definition>
		<skos:prefLabel>Device part</skos:prefLabel>
		<idmp:isUMLAttributeOf rdf:resource="&idmp;investigationalMedicinalProductName"/>
	</owl:NamedIndividual>
	
	<owl:NamedIndividual rdf:about="&idmp;InvestigationalMedicinalProductName.intendedUsePart">
		<rdf:type rdf:resource="&skos;Concept"/>
		<rdf:type rdf:resource="&upper;DataAttribute"/>
		<rdf:type rdf:resource="&upper;LogicalDataEntity"/>
		<skos:altLabel>IDMP.InvestigationalMedicinalProductName.intendedUsePart</skos:altLabel>
		<skos:definition>The intended use, if reflected in the medicinal product name, shall be specified. EXAMPLE For the medicinal product name ‘Drug-BI Caplets - Heartburn Relief’, the intended use part is ‘Heartburn Relief’.</skos:definition>
		<skos:prefLabel>Intended use part</skos:prefLabel>
		<idmp:isUMLAttributeOf rdf:resource="&idmp;investigationalMedicinalProductName"/>
	</owl:NamedIndividual>
	
	<owl:NamedIndividual rdf:about="&idmp;InvestigationalMedicinalProductName.inventedNamePart">
		<rdf:type rdf:resource="&skos;Concept"/>
		<rdf:type rdf:resource="&upper;DataAttribute"/>
		<rdf:type rdf:resource="&upper;LogicalDataEntity"/>
		<skos:altLabel>IDMP.InvestigationalMedicinalProductName.inventedNamePart</skos:altLabel>
		<skos:definition>The invented name (i.e. trade name) of the medicinal product without e.g. the trademark or any other descriptors reflected in the product name shall be specified. EXAMPLE For the medicinal product name ‘Drug XYZ® Accuhaler 200 mg for adults’ the invented (trade) name element is ‘Drug XYZ’.</skos:definition>
		<skos:prefLabel>Invented name part</skos:prefLabel>
		<idmp:isUMLAttributeOf rdf:resource="&idmp;investigationalMedicinalProductName"/>
	</owl:NamedIndividual>
	
	<owl:NamedIndividual rdf:about="&idmp;InvestigationalMedicinalProductName.language">
		<rdf:type rdf:resource="&skos;Concept"/>
		<rdf:type rdf:resource="&upper;DataAttribute"/>
		<rdf:type rdf:resource="&upper;LogicalDataEntity"/>
		<skos:altLabel>IDMP.InvestigationalMedicinalProductName.language</skos:altLabel>
		<skos:definition>The ‘Name’ and its elements and ‘Language’ are actually all part of the EN data type as provided by ISO 21090. They are defined in full here for clarity. Implementations shall use the EN data type.</skos:definition>
		<skos:prefLabel>Language</skos:prefLabel>
		<idmp:isUMLAttributeOf rdf:resource="&idmp;investigationalMedicinalProductName"/>
	</owl:NamedIndividual>
	
	<owl:NamedIndividual rdf:about="&idmp;InvestigationalMedicinalProductName.name">
		<rdf:type rdf:resource="&skos;Concept"/>
		<rdf:type rdf:resource="&upper;DataAttribute"/>
		<rdf:type rdf:resource="&upper;LogicalDataEntity"/>
		<skos:altLabel>IDMP.InvestigationalMedicinalProductName.name</skos:altLabel>
		<skos:definition>The ‘Name’ and its elements and ‘Language’ are actually all part of the EN data type as provided by ISO 21090. They are defined in full here for clarity. Implementations shall use the EN data type.</skos:definition>
		<skos:prefLabel>Name of investigational medicinal product</skos:prefLabel>
		<idmp:isUMLAttributeOf rdf:resource="&idmp;investigationalMedicinalProductName"/>
	</owl:NamedIndividual>
	
	<owl:NamedIndividual rdf:about="&idmp;InvestigationalMedicinalProductName.pharmaceuticalDoseFormPart">
		<rdf:type rdf:resource="&skos;Concept"/>
		<rdf:type rdf:resource="&upper;DataAttribute"/>
		<rdf:type rdf:resource="&upper;LogicalDataEntity"/>
		<skos:altLabel>IDMP.InvestigationalMedicinalProductName.pharmaceuticalDoseFormPart</skos:altLabel>
		<skos:definition>The pharmaceutical dose form, if reflected in the medicinal product name, shall be specified. This pharmaceutical dose form name part may differ from the concept of ‘Administrable Dose Form’ and ‘Manufactured Dose Form’ as described in section X. EXAMPLE For the medicinal product name ‘Novo-DrugX EASY-TO-SWALLOW CAPLETS’, the pharmaceutical dose form name element is ‘EASY-TO-SWALLOW CAPLETS’.</skos:definition>
		<skos:prefLabel>Pharmaceutical dose form part</skos:prefLabel>
		<idmp:isUMLAttributeOf rdf:resource="&idmp;investigationalMedicinalProductName"/>
	</owl:NamedIndividual>
	
	<owl:NamedIndividual rdf:about="&idmp;InvestigationalMedicinalProductName.scientificNamePart">
		<rdf:type rdf:resource="&skos;Concept"/>
		<rdf:type rdf:resource="&upper;DataAttribute"/>
		<rdf:type rdf:resource="&upper;LogicalDataEntity"/>
		<skos:altLabel>IDMP.InvestigationalMedicinalProductName.scientificNamePart</skos:altLabel>
		<skos:definition>The scientific or common (i.e. generic) name of the medicinal product without any other descriptors shall be specified. EXAMPLE For the medicinal product name ‘Irbesartan/Hydrochlorothiazide Pharma KK’ the common (generic) name element is ‘Irbesartan/Hydrochlorothiazide’.</skos:definition>
		<skos:prefLabel>Scientific name part</skos:prefLabel>
		<idmp:isUMLAttributeOf rdf:resource="&idmp;investigationalMedicinalProductName"/>
	</owl:NamedIndividual>
	
	<owl:NamedIndividual rdf:about="&idmp;InvestigationalMedicinalProductName.strengthNamePart">
		<rdf:type rdf:resource="&skos;Concept"/>
		<rdf:type rdf:resource="&upper;DataAttribute"/>
		<rdf:type rdf:resource="&upper;LogicalDataEntity"/>
		<skos:altLabel>IDMP.InvestigationalMedicinalProductName.strengthNamePart</skos:altLabel>
		<skos:definition>The strength, if reflected in the medicinal product name, shall be specified. This strength name part may differ from the concept of ‘Strength’ as described in section 5.13.5. The use of decimal points shall be accommodated, if required. EXAMPLE For the medicinal product name ‘Drug K Forte (Paracetamol 500mg, dihydrocodeine tartrate 30mg)’, the strength name part is ‘Forte’.</skos:definition>
		<skos:prefLabel>Strength name part</skos:prefLabel>
		<idmp:isUMLAttributeOf rdf:resource="&idmp;investigationalMedicinalProductName"/>
	</owl:NamedIndividual>
	
	<owl:NamedIndividual rdf:about="&idmp;InvestigationalMedicinalProductName.trademarkOrCompanyPart">
		<rdf:type rdf:resource="&skos;Concept"/>
		<rdf:type rdf:resource="&upper;DataAttribute"/>
		<rdf:type rdf:resource="&upper;LogicalDataEntity"/>
		<skos:altLabel>IDMP.InvestigationalMedicinalProductName.trademarkOrCompanyPart</skos:altLabel>
		<skos:definition>The trademark, if present in the medicinal product name, shall be provided.</skos:definition>
		<skos:prefLabel>Trademark or company part</skos:prefLabel>
		<idmp:isUMLAttributeOf rdf:resource="&idmp;investigationalMedicinalProductName"/>
	</owl:NamedIndividual>
	
	<owl:NamedIndividual rdf:about="&idmp;InvestigationalMedicinalProductName.year">
		<rdf:type rdf:resource="&skos;Concept"/>
		<rdf:type rdf:resource="&upper;DataAttribute"/>
		<rdf:type rdf:resource="&upper;LogicalDataEntity"/>
		<skos:altLabel>IDMP.InvestigationalMedicinalProductName.year</skos:altLabel>
		<skos:definition>The year/period, if present in the medicinal product name, shall be provided.EXAMPLE For an influenza vaccine with the medicinal product name ‘Drug-FLU season 2008/2009’, the year/period is ‘2008/2009’.</skos:definition>
		<skos:prefLabel>Year on investigational medicinal product</skos:prefLabel>
		<idmp:isUMLAttributeOf rdf:resource="&idmp;investigationalMedicinalProductName"/>
	</owl:NamedIndividual>
	
	<owl:NamedIndividual rdf:about="&idmp;MPIDAttreibuteSet.MPID">
		<rdf:type rdf:resource="&skos;Concept"/>
		<rdf:type rdf:resource="&upper;DataAttribute"/>
		<rdf:type rdf:resource="&upper;LogicalDataEntity"/>
		<skos:altLabel>IDMP.MPIDAttreibuteSet.MPID</skos:altLabel>
		<skos:definition>Medicinal product identifier</skos:definition>
		<skos:prefLabel>Mpid</skos:prefLabel>
		<idmp:isUMLAttributeOf rdf:resource="&idmp;MPIDAttributeSet"/>
	</owl:NamedIndividual>
	
	<owl:NamedIndividual rdf:about="&idmp;MPIDAttributeSet">
		<rdf:type rdf:resource="&owl;Class"/>
		<rdf:type rdf:resource="&skos;Concept"/>
		<rdf:type rdf:resource="&upper;DataObject"/>
		<rdf:type rdf:resource="&upper;LogicalDataEntity"/>
		<rdfs:subClassOf rdf:resource="&skos;Concept"/>
		<skos:altLabel>IDMP.MPIDAttributeSet</skos:altLabel>
		<skos:definition>Medicinal Product Identifier and its related attributes</skos:definition>
		<skos:prefLabel>Mpid attribute set</skos:prefLabel>
		<idmp:hasUMLAttribute rdf:resource="&idmp;MPIDAttreibuteSet.MPID"/>
		<idmp:hasUMLAttribute rdf:resource="&idmp;MPIDAttributeSet.MPID"/>
		<idmp:hasUMLAttribute rdf:resource="&idmp;MPIDAttributeSet.country"/>
		<idmp:hasUMLAttribute rdf:resource="&idmp;MPIDAttributeSet.name"/>
	</owl:NamedIndividual>
	
	<owl:NamedIndividual rdf:about="&idmp;MPIDAttributeSet.MPID">
		<rdf:type rdf:resource="&skos;Concept"/>
		<rdf:type rdf:resource="&upper;DataAttribute"/>
		<rdf:type rdf:resource="&upper;LogicalDataEntity"/>
		<skos:altLabel>IDMP.MPIDAttributeSet.MPID</skos:altLabel>
		<skos:definition>The criteria for the unique identification of an authorized medicinal product.</skos:definition>
		<skos:prefLabel>Mpid</skos:prefLabel>
		<idmp:isUMLAttributeOf rdf:resource="&idmp;MPIDAttributeSet"/>
	</owl:NamedIndividual>
	
	<owl:NamedIndividual rdf:about="&idmp;MPIDAttributeSet.country">
		<rdf:type rdf:resource="&skos;Concept"/>
		<rdf:type rdf:resource="&upper;DataAttribute"/>
		<rdf:type rdf:resource="&upper;LogicalDataEntity"/>
		<skos:altLabel>IDMP.MPIDAttributeSet.country</skos:altLabel>
		<skos:definition>Country in which the medicinal product was developed</skos:definition>
		<skos:prefLabel>Mpid attribute set country</skos:prefLabel>
		<idmp:isUMLAttributeOf rdf:resource="&idmp;MPIDAttributeSet"/>
	</owl:NamedIndividual>
	
	<owl:NamedIndividual rdf:about="&idmp;MPIDAttributeSet.name">
		<rdf:type rdf:resource="&skos;Concept"/>
		<rdf:type rdf:resource="&upper;DataAttribute"/>
		<rdf:type rdf:resource="&upper;LogicalDataEntity"/>
		<skos:altLabel>IDMP.MPIDAttributeSet.name</skos:altLabel>
		<skos:definition>Name of the medicinal product</skos:definition>
		<skos:prefLabel>Mpid attribute set name</skos:prefLabel>
		<idmp:isUMLAttributeOf rdf:resource="&idmp;MPIDAttributeSet"/>
	</owl:NamedIndividual>
	
	<owl:NamedIndividual rdf:about="&idmp;Medicinalproductbatchidentifier.batchId">
		<rdf:type rdf:resource="&skos;Concept"/>
		<rdf:type rdf:resource="&upper;DataAttribute"/>
		<rdf:type rdf:resource="&upper;LogicalDataEntity"/>
		<skos:altLabel>IDMP.Medicinalproductbatchidentifier.batchId</skos:altLabel>
		<skos:definition>Manufacturer&apos;s batch identification at product level.</skos:definition>
		<skos:prefLabel>Batch id</skos:prefLabel>
		<idmp:isUMLAttributeOf rdf:resource="&idmp;medicinalProductBatchIdentifier"/>
	</owl:NamedIndividual>
	
	<owl:NamedIndividual rdf:about="&idmp;Organisation">
		<rdf:type rdf:resource="&owl;Class"/>
		<rdf:type rdf:resource="&skos;Concept"/>
		<rdf:type rdf:resource="&upper;DataObject"/>
		<rdf:type rdf:resource="&upper;LogicalDataEntity"/>
		<rdfs:subClassOf rdf:resource="&skos;Concept"/>
		<dct:source>ISO IDMP 11615:2017</dct:source>
		<skos:altLabel>IDMP.Organisation</skos:altLabel>
		<skos:definition>The Medicinal Product is associated with organisation information for one or more manufacturers or establishments which undertake various manufacturing operations in order to produce a Medicinal Product. These may be overseen by an appropriate Medicines Regulatory Agency. Sourcehttp://www.ema.europa.eu/docs/en_GB/document_library/Presentation/2016/08/WC500212059.pdfOrganisations: Data that comprises of organisation name and location address data for organisations such as MAH  sponsors  regulatory authority  manufacturers</skos:definition>
		<skos:prefLabel>Organisation</skos:prefLabel>
		<skos:related rdf:resource="&idmp;manufacturingAuthorisation"/>
		<skos:related rdf:resource="&idmp;medicalDevice"/>
		<idmp:hasUMLAttribute rdf:resource="&idmp;organisation.address"/>
		<idmp:hasUMLAttribute rdf:resource="&idmp;organisation.identifier"/>
		<idmp:hasUMLAttribute rdf:resource="&idmp;organisation.name"/>
	</owl:NamedIndividual>
	
	<owl:NamedIndividual rdf:about="&idmp;PCID.marketingAuthorisation">
		<rdf:type rdf:resource="&skos;Concept"/>
		<rdf:type rdf:resource="&upper;DataAttribute"/>
		<rdf:type rdf:resource="&upper;LogicalDataEntity"/>
		<skos:altLabel>IDMP.PCID.marketingAuthorisation</skos:altLabel>
		<skos:definition>The marketing authorization is issued by the appropriate regulatory medicines authority in a jurisdiction. In line with the laws and regulations applicable in a jurisdiction, an authorization is required before a medicinal product is placed on the market. For some categories of medicinal products (e.g. ‘grandfather’ drugs) exemptions may be applicable. For these type of medicines, the same principles as for authorized medicinal products shall be applied as outlined in this section. Where no formal marketing authorization holder is established, the distributor shall be specified.</skos:definition>
		<skos:prefLabel>Pcid Marketing authorisation</skos:prefLabel>
		<idmp:isUMLAttributeOf rdf:resource="&idmp;PCIDAttributeSet"/>
	</owl:NamedIndividual>
	
	<owl:NamedIndividual rdf:about="&idmp;PCIDAttributeSet">
		<rdf:type rdf:resource="&owl;Class"/>
		<rdf:type rdf:resource="&skos;Concept"/>
		<rdf:type rdf:resource="&upper;DataObject"/>
		<rdf:type rdf:resource="&upper;LogicalDataEntity"/>
		<rdfs:subClassOf rdf:resource="&skos;Concept"/>
		<skos:altLabel>IDMP.PCIDAttributeSet</skos:altLabel>
		<skos:definition>This is the product in its packaging. This class acts as a parent for more detailed descriptive classes.</skos:definition>
		<skos:prefLabel>Pcid attribute set</skos:prefLabel>
		<skos:related rdf:resource="&idmp;MPIDAttributeSet"/>
		<idmp:hasUMLAttribute rdf:resource="&idmp;PCID.marketingAuthorisation"/>
		<idmp:hasUMLAttribute rdf:resource="&idmp;PCIDAttributeSet.PCID"/>
		<idmp:hasUMLAttribute rdf:resource="&idmp;PCIDAttributeSet.otherCharacteristics"/>
	</owl:NamedIndividual>
	
	<owl:NamedIndividual rdf:about="&idmp;PCIDAttributeSet.PCID">
		<rdf:type rdf:resource="&skos;Concept"/>
		<rdf:type rdf:resource="&upper;DataAttribute"/>
		<rdf:type rdf:resource="&upper;LogicalDataEntity"/>
		<skos:altLabel>IDMP.PCIDAttributeSet.PCID</skos:altLabel>
		<skos:definition>Investigational medicinal product package identifier</skos:definition>
		<skos:prefLabel>Pcid</skos:prefLabel>
		<idmp:isUMLAttributeOf rdf:resource="&idmp;PCIDAttributeSet"/>
	</owl:NamedIndividual>
	
	<owl:NamedIndividual rdf:about="&idmp;PCIDAttributeSet.otherCharacteristics">
		<rdf:type rdf:resource="&skos;Concept"/>
		<rdf:type rdf:resource="&upper;DataAttribute"/>
		<rdf:type rdf:resource="&upper;LogicalDataEntity"/>
		<skos:altLabel>IDMP.PCIDAttributeSet.otherCharacteristics</skos:altLabel>
		<skos:definition>Zero or more other observations shall be made about the characteristics of the ‘Packaged Medicinal Product’, where applicable. They are represented by naming the characteristic in the ‘Code’ attribute using a CD data type, and then if required providing a ‘Value’ for the characteristic named using an ANY data type. This facility is useful for capturing unusual details not explicitly catered for in the other attributes.</skos:definition>
		<skos:prefLabel>Other characteristics</skos:prefLabel>
		<idmp:isUMLAttributeOf rdf:resource="&idmp;PCIDAttributeSet"/>
	</owl:NamedIndividual>
	
	<owl:NamedIndividual rdf:about="&idmp;PhPID.administerableDoseForm">
		<rdf:type rdf:resource="&skos;Concept"/>
		<rdf:type rdf:resource="&upper;DataAttribute"/>
		<rdf:type rdf:resource="&upper;LogicalDataEntity"/>
		<skos:altLabel>IDMP.PhPID.administerableDoseForm</skos:altLabel>
		<skos:definition>This shall describe the pharmaceutical dose form as to be administered to the patient in accordance with theterms laid down in the marketing authorization. It is after it has undergone any necessary reconstitution. A term and a term identifier as defined by ISO/DIS 11239 and its resulting controlled vocabulary shall be used. It is to be specified using a cde data type. EXAMPLE Values are: Tablet, Capsule, Oral Solution, Suspension. NOTE A medicinal product may have two manufactured items, one with a ‘Manufactured Dose Form’ of ‘powder for solution for injection’ and the other with a ‘Manufactured Dose Form’ of ‘solvent for solution for injection’. These are then reconstituted to an ‘Administrable Dose Form’ ‘solution for injection’ before administered to a patient.</skos:definition>
		<skos:prefLabel>Phpid administerable dose form</skos:prefLabel>
		<idmp:isUMLAttributeOf rdf:resource="&idmp;PhPIDSub"/>
	</owl:NamedIndividual>
	
	<owl:NamedIndividual rdf:about="&idmp;PhPID.identifier">
		<rdf:type rdf:resource="&skos;Concept"/>
		<rdf:type rdf:resource="&upper;DataAttribute"/>
		<rdf:type rdf:resource="&upper;LogicalDataEntity"/>
		<skos:altLabel>IDMP.PhPID.identifier</skos:altLabel>
		<skos:definition>Unique identifier for a pharmaceutical product</skos:definition>
		<skos:prefLabel>Phpid identifier</skos:prefLabel>
		<idmp:isUMLAttributeOf rdf:resource="&idmp;PhPIDSub"/>
	</owl:NamedIndividual>
	
	<owl:NamedIndividual rdf:about="&idmp;PhPID.name">
		<rdf:type rdf:resource="&skos;Concept"/>
		<rdf:type rdf:resource="&upper;DataAttribute"/>
		<rdf:type rdf:resource="&upper;LogicalDataEntity"/>
		<skos:altLabel>IDMP.PhPID.name</skos:altLabel>
		<skos:definition>Name of the pharmceutical product</skos:definition>
		<skos:prefLabel>Phpid name</skos:prefLabel>
		<idmp:isUMLAttributeOf rdf:resource="&idmp;PhPIDSub"/>
	</owl:NamedIndividual>
	
	<owl:NamedIndividual rdf:about="&idmp;PhPID.strength">
		<rdf:type rdf:resource="&skos;Concept"/>
		<rdf:type rdf:resource="&upper;DataAttribute"/>
		<rdf:type rdf:resource="&upper;LogicalDataEntity"/>
		<skos:altLabel>IDMP.PhPID.strength</skos:altLabel>
		<skos:definition>The strength of the Substance(s) or Specified Substance(s) shall be described as a quantity of the substance present in a given quantity of the Pharmaceutical Product.</skos:definition>
		<skos:prefLabel>Phpid strength</skos:prefLabel>
		<idmp:isUMLAttributeOf rdf:resource="&idmp;PhPIDSub"/>
	</owl:NamedIndividual>
	
	<owl:NamedIndividual rdf:about="&idmp;PhPID.unitOfPresentation">
		<rdf:type rdf:resource="&skos;Concept"/>
		<rdf:type rdf:resource="&upper;DataAttribute"/>
		<rdf:type rdf:resource="&upper;LogicalDataEntity"/>
		<skos:altLabel>IDMP.PhPID.unitOfPresentation</skos:altLabel>
		<skos:definition>Unit of presentation shall refer to the qualitative description of the unit in which the strength(s) of the pharmaceutical product is presented and described, often specifically at the point of delivery to the patient, in cases where a quantitative unit of measurement is not applicable. The unit of presentation standard term (see ISO/DIS 11239) shall be described.</skos:definition>
		<skos:prefLabel>Phpid unit of presentation</skos:prefLabel>
		<idmp:isUMLAttributeOf rdf:resource="&idmp;PhPIDSub"/>
	</owl:NamedIndividual>
	
	<owl:NamedIndividual rdf:about="&idmp;PhPIDSet">
		<rdf:type rdf:resource="&owl;Class"/>
		<rdf:type rdf:resource="&skos;Concept"/>
		<rdf:type rdf:resource="&upper;DataObject"/>
		<rdf:type rdf:resource="&upper;LogicalDataEntity"/>
		<rdfs:subClassOf rdf:resource="&skos;Concept"/>
		<skos:altLabel>IDMP.PhPIDSet</skos:altLabel>
		<skos:definition>Pharmaceutical Product Identifier and its related attributes</skos:definition>
		<skos:prefLabel>Phpid set</skos:prefLabel>
		<skos:related rdf:resource="&idmp;pharmaceuticalProduct"/>
	</owl:NamedIndividual>
	
	<owl:NamedIndividual rdf:about="&idmp;PhPIDSpSub">
		<rdf:type rdf:resource="&owl;Class"/>
		<rdf:type rdf:resource="&skos;Concept"/>
		<rdf:type rdf:resource="&upper;DataObject"/>
		<rdf:type rdf:resource="&upper;LogicalDataEntity"/>
		<rdfs:subClassOf rdf:resource="&skos;Concept"/>
		<skos:altLabel>IDMP.PhPIDSpSub</skos:altLabel>
		<skos:definition>Special Substance, see Special Substance model for definition</skos:definition>
		<skos:prefLabel>Phpid sp sub</skos:prefLabel>
		<skos:related rdf:resource="&idmp;PhPIDSet"/>
		<idmp:hasUMLAttribute rdf:resource="&idmp;PhPIDSpSub.administerableDoseForm"/>
		<idmp:hasUMLAttribute rdf:resource="&idmp;PhPIDSpSub.identifier"/>
		<idmp:hasUMLAttribute rdf:resource="&idmp;PhPIDSpSub.name"/>
		<idmp:hasUMLAttribute rdf:resource="&idmp;PhPIDSpSub.strength"/>
		<idmp:hasUMLAttribute rdf:resource="&idmp;PhPIDSpSub.unitOfPresentation"/>
	</owl:NamedIndividual>
	
	<owl:NamedIndividual rdf:about="&idmp;PhPIDSpSub.administerableDoseForm">
		<rdf:type rdf:resource="&skos;Concept"/>
		<rdf:type rdf:resource="&upper;DataAttribute"/>
		<rdf:type rdf:resource="&upper;LogicalDataEntity"/>
		<skos:altLabel>IDMP.PhPIDSpSub.administerableDoseForm</skos:altLabel>
		<skos:definition>This shall describe the pharmaceutical dose form as to be administered in accordance with the terms as authorised by a regulatory medicines authority. It is after it has undergone any necessary reconstitution. It is a value drawn from a value set specified in ISO 11239. It is to be specified using a CD data type. EXAMPLE Tablet, Capsule, Oral Solution, Suspension.Each pharmaceutical product can have only one pharmaceutical form.</skos:definition>
		<skos:prefLabel>Phpid sp sub administerable dose form</skos:prefLabel>
		<idmp:isUMLAttributeOf rdf:resource="&idmp;PhPIDSpSub"/>
	</owl:NamedIndividual>
	
	<owl:NamedIndividual rdf:about="&idmp;PhPIDSpSub.identifier">
		<rdf:type rdf:resource="&skos;Concept"/>
		<rdf:type rdf:resource="&upper;DataAttribute"/>
		<rdf:type rdf:resource="&upper;LogicalDataEntity"/>
		<skos:altLabel>IDMP.PhPIDSpSub.identifier</skos:altLabel>
		<skos:definition>Idetifier for special substance</skos:definition>
		<skos:prefLabel>Phpid sub identifier</skos:prefLabel>
		<idmp:isUMLAttributeOf rdf:resource="&idmp;PhPIDSpSub"/>
	</owl:NamedIndividual>
	
	<owl:NamedIndividual rdf:about="&idmp;PhPIDSpSub.name">
		<rdf:type rdf:resource="&skos;Concept"/>
		<rdf:type rdf:resource="&upper;DataAttribute"/>
		<rdf:type rdf:resource="&upper;LogicalDataEntity"/>
		<skos:altLabel>IDMP.PhPIDSpSub.name</skos:altLabel>
		<skos:definition>Name of the special substance</skos:definition>
		<skos:prefLabel>Phpid sp sub name</skos:prefLabel>
		<idmp:isUMLAttributeOf rdf:resource="&idmp;PhPIDSpSub"/>
	</owl:NamedIndividual>
	
	<owl:NamedIndividual rdf:about="&idmp;PhPIDSpSub.strength">
		<rdf:type rdf:resource="&skos;Concept"/>
		<rdf:type rdf:resource="&upper;DataAttribute"/>
		<rdf:type rdf:resource="&upper;LogicalDataEntity"/>
		<skos:altLabel>IDMP.PhPIDSpSub.strength</skos:altLabel>
		<skos:definition>Strength of the special substance</skos:definition>
		<skos:prefLabel>Phpid Sp sub strength</skos:prefLabel>
		<idmp:isUMLAttributeOf rdf:resource="&idmp;PhPIDSpSub"/>
	</owl:NamedIndividual>
	
	<owl:NamedIndividual rdf:about="&idmp;PhPIDSpSub.unitOfPresentation">
		<rdf:type rdf:resource="&skos;Concept"/>
		<rdf:type rdf:resource="&upper;DataAttribute"/>
		<rdf:type rdf:resource="&upper;LogicalDataEntity"/>
		<skos:altLabel>IDMP.PhPIDSpSub.unitOfPresentation</skos:altLabel>
		<skos:definition>Qualitative term describing the unit in which the strength(s) of the manufactured item or pharmaceutical product is presented and described. Often used specifically at the point of delivery to the patient in cases where a quantitative unit of measurement is not applicable. A unit of presentation may have the same ‘display name’ as in another controlled vocabulary, such as apharmaceutical dose form, but the two concepts are not equivalent, and each has a unique controlled vocabulary term identifier. EXAMPLE Tablet, spray, puff. Contains 100 mcg per spray (Here unit of presentation is spray)</skos:definition>
		<skos:prefLabel>Phpid sp sub unit of presentation</skos:prefLabel>
		<idmp:isUMLAttributeOf rdf:resource="&idmp;PhPIDSpSub"/>
	</owl:NamedIndividual>
	
	<owl:NamedIndividual rdf:about="&idmp;PhPIDSpSubL1">
		<rdf:type rdf:resource="&owl;Class"/>
		<rdf:type rdf:resource="&skos;Concept"/>
		<rdf:type rdf:resource="&upper;DataObject"/>
		<rdf:type rdf:resource="&upper;LogicalDataEntity"/>
		<rdfs:subClassOf rdf:resource="&skos;Concept"/>
		<skos:altLabel>IDMP.PhPIDSpSubL1</skos:altLabel>
		<skos:definition>Specified substance level1</skos:definition>
		<skos:prefLabel>Phpid sp sub l1</skos:prefLabel>
		<skos:related rdf:resource="&idmp;PhPIDSet"/>
		<idmp:hasUMLAttribute rdf:resource="&idmp;PhPIDSpSubL1.Identifier"/>
		<idmp:hasUMLAttribute rdf:resource="&idmp;PhPIDSpSubL1.name"/>
	</owl:NamedIndividual>
	
	<owl:NamedIndividual rdf:about="&idmp;PhPIDSpSubL1.Identifier">
		<rdf:type rdf:resource="&skos;Concept"/>
		<rdf:type rdf:resource="&upper;DataAttribute"/>
		<rdf:type rdf:resource="&upper;LogicalDataEntity"/>
		<skos:altLabel>IDMP.PhPIDSpSubL1.Identifier</skos:altLabel>
		<skos:definition>Idetifier for special substance</skos:definition>
		<skos:prefLabel>Phpid sp sub l1 identifier</skos:prefLabel>
		<idmp:isUMLAttributeOf rdf:resource="&idmp;PhPIDSpSubL1"/>
	</owl:NamedIndividual>
	
	<owl:NamedIndividual rdf:about="&idmp;PhPIDSpSubL1.name">
		<rdf:type rdf:resource="&skos;Concept"/>
		<rdf:type rdf:resource="&upper;DataAttribute"/>
		<rdf:type rdf:resource="&upper;LogicalDataEntity"/>
		<skos:altLabel>IDMP.PhPIDSpSubL1.name</skos:altLabel>
		<skos:definition>Name of the special substance</skos:definition>
		<skos:prefLabel>Phpid sp sub l1 name</skos:prefLabel>
		<idmp:isUMLAttributeOf rdf:resource="&idmp;PhPIDSpSubL1"/>
	</owl:NamedIndividual>
	
	<owl:NamedIndividual rdf:about="&idmp;PhPIDSpSubL2">
		<rdf:type rdf:resource="&owl;Class"/>
		<rdf:type rdf:resource="&skos;Concept"/>
		<rdf:type rdf:resource="&upper;DataObject"/>
		<rdf:type rdf:resource="&upper;LogicalDataEntity"/>
		<rdfs:subClassOf rdf:resource="&skos;Concept"/>
		<skos:altLabel>IDMP.PhPIDSpSubL2</skos:altLabel>
		<skos:definition>Specified substance level2</skos:definition>
		<skos:prefLabel>Phpid sp sub l2</skos:prefLabel>
		<skos:related rdf:resource="&idmp;PhPIDSet"/>
		<idmp:hasUMLAttribute rdf:resource="&idmp;PhPIDSpSubL2.identifier"/>
		<idmp:hasUMLAttribute rdf:resource="&idmp;PhPIDSpSubL2.name"/>
	</owl:NamedIndividual>
	
	<owl:NamedIndividual rdf:about="&idmp;PhPIDSpSubL2.identifier">
		<rdf:type rdf:resource="&skos;Concept"/>
		<rdf:type rdf:resource="&upper;DataAttribute"/>
		<rdf:type rdf:resource="&upper;LogicalDataEntity"/>
		<skos:altLabel>IDMP.PhPIDSpSubL2.identifier</skos:altLabel>
		<skos:definition>Idetifier for special substance</skos:definition>
		<skos:prefLabel>Phpid sp sub l2 identifier</skos:prefLabel>
		<idmp:isUMLAttributeOf rdf:resource="&idmp;PhPIDSpSubL2"/>
	</owl:NamedIndividual>
	
	<owl:NamedIndividual rdf:about="&idmp;PhPIDSpSubL2.name">
		<rdf:type rdf:resource="&skos;Concept"/>
		<rdf:type rdf:resource="&upper;DataAttribute"/>
		<rdf:type rdf:resource="&upper;LogicalDataEntity"/>
		<skos:altLabel>IDMP.PhPIDSpSubL2.name</skos:altLabel>
		<skos:definition>Name of the special substance</skos:definition>
		<skos:prefLabel>Phpid sp sub l2 name</skos:prefLabel>
		<idmp:isUMLAttributeOf rdf:resource="&idmp;PhPIDSpSubL2"/>
	</owl:NamedIndividual>
	
	<owl:NamedIndividual rdf:about="&idmp;PhPIDSpSubL3">
		<rdf:type rdf:resource="&owl;Class"/>
		<rdf:type rdf:resource="&skos;Concept"/>
		<rdf:type rdf:resource="&upper;DataObject"/>
		<rdf:type rdf:resource="&upper;LogicalDataEntity"/>
		<rdfs:subClassOf rdf:resource="&skos;Concept"/>
		<skos:altLabel>IDMP.PhPIDSpSubL3</skos:altLabel>
		<skos:definition>Specified substance level3</skos:definition>
		<skos:prefLabel>Phpid sp sub l3</skos:prefLabel>
		<skos:related rdf:resource="&idmp;PhPIDSet"/>
		<idmp:hasUMLAttribute rdf:resource="&idmp;PhPIDSpSubL3.identifier"/>
		<idmp:hasUMLAttribute rdf:resource="&idmp;PhPIDSpSubL3.name"/>
	</owl:NamedIndividual>
	
	<owl:NamedIndividual rdf:about="&idmp;PhPIDSpSubL3.identifier">
		<rdf:type rdf:resource="&skos;Concept"/>
		<rdf:type rdf:resource="&upper;DataAttribute"/>
		<rdf:type rdf:resource="&upper;LogicalDataEntity"/>
		<skos:altLabel>IDMP.PhPIDSpSubL3.identifier</skos:altLabel>
		<skos:definition>Idetifier for special substance</skos:definition>
		<skos:prefLabel>Phpid sp sub l3 identifier</skos:prefLabel>
		<idmp:isUMLAttributeOf rdf:resource="&idmp;PhPIDSpSubL3"/>
	</owl:NamedIndividual>
	
	<owl:NamedIndividual rdf:about="&idmp;PhPIDSpSubL3.name">
		<rdf:type rdf:resource="&skos;Concept"/>
		<rdf:type rdf:resource="&upper;DataAttribute"/>
		<rdf:type rdf:resource="&upper;LogicalDataEntity"/>
		<skos:altLabel>IDMP.PhPIDSpSubL3.name</skos:altLabel>
		<skos:definition>Name of the special substance</skos:definition>
		<skos:prefLabel>Phpid sp sub l3 name</skos:prefLabel>
		<idmp:isUMLAttributeOf rdf:resource="&idmp;PhPIDSpSubL3"/>
	</owl:NamedIndividual>
	
	<owl:NamedIndividual rdf:about="&idmp;PhPIDSub">
		<rdf:type rdf:resource="&owl;Class"/>
		<rdf:type rdf:resource="&skos;Concept"/>
		<rdf:type rdf:resource="&upper;DataObject"/>
		<rdf:type rdf:resource="&upper;LogicalDataEntity"/>
		<rdfs:subClassOf rdf:resource="&skos;Concept"/>
		<skos:altLabel>IDMP.PhPIDSub</skos:altLabel>
		<skos:definition>Pharmaceutical Product Substance Stratum Elements. The construct of the pharmaceutical product substance stratum utilizes the active substance(s) with strength, reference strength, administrable dose form and medical device (when applicable).</skos:definition>
		<skos:prefLabel>Phpid sub</skos:prefLabel>
		<skos:related rdf:resource="&idmp;PhPIDSet"/>
		<idmp:hasUMLAttribute rdf:resource="&idmp;PhPID.administerableDoseForm"/>
		<idmp:hasUMLAttribute rdf:resource="&idmp;PhPID.identifier"/>
		<idmp:hasUMLAttribute rdf:resource="&idmp;PhPID.name"/>
		<idmp:hasUMLAttribute rdf:resource="&idmp;PhPID.strength"/>
		<idmp:hasUMLAttribute rdf:resource="&idmp;PhPID.unitOfPresentation"/>
	</owl:NamedIndividual>
	
	<owl:NamedIndividual rdf:about="&idmp;PhPIDSubL1">
		<rdf:type rdf:resource="&owl;Class"/>
		<rdf:type rdf:resource="&skos;Concept"/>
		<rdf:type rdf:resource="&upper;DataObject"/>
		<rdf:type rdf:resource="&upper;LogicalDataEntity"/>
		<rdfs:subClassOf rdf:resource="&skos;Concept"/>
		<skos:altLabel>IDMP.PhPIDSubL1</skos:altLabel>
		<skos:definition>Pharmaceutical Product Specified Substance. Each pharmaceutical product shall have one or more active substances.</skos:definition>
		<skos:prefLabel>Phpid sub l1</skos:prefLabel>
		<skos:related rdf:resource="&idmp;PhPIDSet"/>
		<idmp:hasUMLAttribute rdf:resource="&idmp;PhPIDSubL1.id"/>
		<idmp:hasUMLAttribute rdf:resource="&idmp;PhPIDSubL1.name"/>
	</owl:NamedIndividual>
	
	<owl:NamedIndividual rdf:about="&idmp;PhPIDSubL1.id">
		<rdf:type rdf:resource="&skos;Concept"/>
		<rdf:type rdf:resource="&upper;DataAttribute"/>
		<rdf:type rdf:resource="&upper;LogicalDataEntity"/>
		<skos:altLabel>IDMP.PhPIDSubL1.id</skos:altLabel>
		<skos:definition>Phpid sub l1 id</skos:definition>
		<skos:prefLabel>Phpid sub l1 id</skos:prefLabel>
		<idmp:isUMLAttributeOf rdf:resource="&idmp;PhPIDSubL1"/>
	</owl:NamedIndividual>
	
	<owl:NamedIndividual rdf:about="&idmp;PhPIDSubL1.name">
		<rdf:type rdf:resource="&skos;Concept"/>
		<rdf:type rdf:resource="&upper;DataAttribute"/>
		<rdf:type rdf:resource="&upper;LogicalDataEntity"/>
		<skos:altLabel>IDMP.PhPIDSubL1.name</skos:altLabel>
		<skos:definition>Phpid sub l1 name</skos:definition>
		<skos:prefLabel>Phpid sub l1 name</skos:prefLabel>
		<idmp:isUMLAttributeOf rdf:resource="&idmp;PhPIDSubL1"/>
	</owl:NamedIndividual>
	
	<owl:NamedIndividual rdf:about="&idmp;PhPIDSubL2">
		<rdf:type rdf:resource="&owl;Class"/>
		<rdf:type rdf:resource="&skos;Concept"/>
		<rdf:type rdf:resource="&upper;DataObject"/>
		<rdf:type rdf:resource="&upper;LogicalDataEntity"/>
		<rdfs:subClassOf rdf:resource="&skos;Concept"/>
		<skos:altLabel>IDMP.PhPIDSubL2</skos:altLabel>
		<skos:definition>Pharmaceutical Product Specified Substance Strength. The strength of the Substance(s) or Specified Substance(s) shall be described as a quantity of the substance present in a given quantity of the Pharmaceutical Product.</skos:definition>
		<skos:prefLabel>Phpid sub l2</skos:prefLabel>
		<skos:related rdf:resource="&idmp;PhPIDSet"/>
		<idmp:hasUMLAttribute rdf:resource="&idmp;PhPIDSubL2.id"/>
		<idmp:hasUMLAttribute rdf:resource="&idmp;PhPIDSubL2.name"/>
	</owl:NamedIndividual>
	
	<owl:NamedIndividual rdf:about="&idmp;PhPIDSubL2.id">
		<rdf:type rdf:resource="&skos;Concept"/>
		<rdf:type rdf:resource="&upper;DataAttribute"/>
		<rdf:type rdf:resource="&upper;LogicalDataEntity"/>
		<skos:altLabel>IDMP.PhPIDSubL2.id</skos:altLabel>
		<skos:definition>Phpid sub l2 id</skos:definition>
		<skos:prefLabel>Phpid sub l2 id</skos:prefLabel>
		<idmp:isUMLAttributeOf rdf:resource="&idmp;PhPIDSubL2"/>
	</owl:NamedIndividual>
	
	<owl:NamedIndividual rdf:about="&idmp;PhPIDSubL2.name">
		<rdf:type rdf:resource="&skos;Concept"/>
		<rdf:type rdf:resource="&upper;DataAttribute"/>
		<rdf:type rdf:resource="&upper;LogicalDataEntity"/>
		<skos:altLabel>IDMP.PhPIDSubL2.name</skos:altLabel>
		<skos:definition>Phpid sub l2 name</skos:definition>
		<skos:prefLabel>Phpid sub l2 name</skos:prefLabel>
		<idmp:isUMLAttributeOf rdf:resource="&idmp;PhPIDSubL2"/>
	</owl:NamedIndividual>
	
	<owl:NamedIndividual rdf:about="&idmp;PhPIDSubL3">
		<rdf:type rdf:resource="&owl;Class"/>
		<rdf:type rdf:resource="&skos;Concept"/>
		<rdf:type rdf:resource="&upper;DataObject"/>
		<rdf:type rdf:resource="&upper;LogicalDataEntity"/>
		<rdfs:subClassOf rdf:resource="&skos;Concept"/>
		<skos:altLabel>IDMP.PhPIDSubL3</skos:altLabel>
		<skos:definition>Pharmaceutical Product Specified Substance Form. Defined by special substance vocab, reference strength and administerable dose form</skos:definition>
		<skos:prefLabel>Phpid sub l3</skos:prefLabel>
		<skos:related rdf:resource="&idmp;PhPIDSet"/>
		<idmp:hasUMLAttribute rdf:resource="&idmp;PhPIDSubL3.id"/>
		<idmp:hasUMLAttribute rdf:resource="&idmp;PhPIDSubL3.name"/>
	</owl:NamedIndividual>
	
	<owl:NamedIndividual rdf:about="&idmp;PhPIDSubL3.id">
		<rdf:type rdf:resource="&skos;Concept"/>
		<rdf:type rdf:resource="&upper;DataAttribute"/>
		<rdf:type rdf:resource="&upper;LogicalDataEntity"/>
		<skos:altLabel>IDMP.PhPIDSubL3.id</skos:altLabel>
		<skos:definition>Phpid sub l3 id</skos:definition>
		<skos:prefLabel>Phpid sub l3 id</skos:prefLabel>
		<idmp:isUMLAttributeOf rdf:resource="&idmp;PhPIDSubL3"/>
	</owl:NamedIndividual>
	
	<owl:NamedIndividual rdf:about="&idmp;PhPIDSubL3.name">
		<rdf:type rdf:resource="&skos;Concept"/>
		<rdf:type rdf:resource="&upper;DataAttribute"/>
		<rdf:type rdf:resource="&upper;LogicalDataEntity"/>
		<skos:altLabel>IDMP.PhPIDSubL3.name</skos:altLabel>
		<skos:definition>Phpid sub l3 name</skos:definition>
		<skos:prefLabel>Phpid sub l3 name</skos:prefLabel>
		<idmp:isUMLAttributeOf rdf:resource="&idmp;PhPIDSubL3"/>
	</owl:NamedIndividual>
	
	<owl:NamedIndividual rdf:about="&idmp;Sponsor">
		<rdf:type rdf:resource="&owl;Class"/>
		<rdf:type rdf:resource="&skos;Concept"/>
		<rdf:type rdf:resource="&upper;DataObject"/>
		<rdf:type rdf:resource="&upper;LogicalDataEntity"/>
		<rdfs:subClassOf rdf:resource="&skos;Concept"/>
		<dct:source>Source ISO IDMP 11615:2017</dct:source>
		<skos:altLabel>IDMP.Sponsor</skos:altLabel>
		<skos:definition>Sponsor individual, company, institution or organisation, which takes responsibility for the initiation, management and/or financing of a clinical trial (3.1.11)</skos:definition>
		<skos:prefLabel>Sponsor</skos:prefLabel>
		<skos:related rdf:resource="&idmp;IMPIDAttributeSet"/>
		<idmp:hasUMLAttribute rdf:resource="&idmp;sponsor.legalRepresentative"/>
		<idmp:hasUMLAttribute rdf:resource="&idmp;sponsor.organisation"/>
		<idmp:hasUMLAttribute rdf:resource="&idmp;sponsor.status"/>
	</owl:NamedIndividual>
	
	<owl:NamedIndividual rdf:about="&idmp;Strength">
		<rdf:type rdf:resource="&owl;Class"/>
		<rdf:type rdf:resource="&skos;Concept"/>
		<rdf:type rdf:resource="&upper;DataObject"/>
		<rdf:type rdf:resource="&upper;LogicalDataEntity"/>
		<rdfs:subClassOf rdf:resource="&skos;Concept"/>
		<dct:source>Source ISO IDMP 11615:2017Strength</dct:source>
		<skos:altLabel>IDMP.Strength</skos:altLabel>
		<skos:definition>The strength of the substance or specified substance shall be specified as a quantity of the substance/specified substance present in a given manufactured item or pharmaceutical product. A numerator value and numerator unit as well as a denominator value and denominator unit shall be used.Strength can be expressed in two ways: strength (presentation) and strength (concentration).When the strength of a pharmaceutical product that has undergone a transformation (e.g. reconstitution) is to be specified, it shall be specified using the strength resulting from transformation undertaken exactly in accordance with the regulated product information.</skos:definition>
		<skos:prefLabel>Strength</skos:prefLabel>
		<skos:related rdf:resource="&idmp;referenceStrength"/>
		<skos:related rdf:resource="&idmp;specifiedSubstance"/>
		<idmp:hasUMLAttribute rdf:resource="&idmp;strength.country"/>
		<idmp:hasUMLAttribute rdf:resource="&idmp;strength.measurementPoint"/>
		<idmp:hasUMLAttribute rdf:resource="&idmp;strength.range"/>
	</owl:NamedIndividual>
	
	<owl:NamedIndividual rdf:about="&idmp;clinicalTrialAuthorisation">
		<rdf:type rdf:resource="&owl;Class"/>
		<rdf:type rdf:resource="&skos;Concept"/>
		<rdf:type rdf:resource="&upper;DataObject"/>
		<rdf:type rdf:resource="&upper;LogicalDataEntity"/>
		<rdfs:subClassOf rdf:resource="&skos;Concept"/>
		<skos:altLabel>IDMP.clinicalTrialAuthorisation</skos:altLabel>
		<skos:definition>Authorization granted by a medicines regulatory authority to run a clinical trial in a jurisdiction</skos:definition>
		<skos:prefLabel>Clinical trial authorisation</skos:prefLabel>
		<skos:related rdf:resource="&idmp;IMPIDAttributeSet"/>
		<idmp:hasUMLAttribute rdf:resource="&idmp;clinicalTrialAuthorisation.country"/>
		<idmp:hasUMLAttribute rdf:resource="&idmp;clinicalTrialAuthorisation.investigationCode"/>
		<idmp:hasUMLAttribute rdf:resource="&idmp;clinicalTrialAuthorisation.jurisdictionalInvestigationCode"/>
		<idmp:hasUMLAttribute rdf:resource="&idmp;clinicalTrialAuthorisation.localClinicalTrialAuthorisation"/>
		<idmp:hasUMLAttribute rdf:resource="&idmp;clinicalTrialAuthorisation.productClassification"/>
		<idmp:hasUMLAttribute rdf:resource="&idmp;clinicalTrialAuthorisation.registrationNumber"/>
	</owl:NamedIndividual>
	
	<owl:NamedIndividual rdf:about="&idmp;clinicalTrialAuthorisation.country">
		<rdf:type rdf:resource="&skos;Concept"/>
		<rdf:type rdf:resource="&upper;DataAttribute"/>
		<rdf:type rdf:resource="&upper;LogicalDataEntity"/>
		<skos:altLabel>IDMP.clinicalTrialAuthorisation.country</skos:altLabel>
		<skos:definition>The jurisdiction(s) in which the clinical trial authorization was granted shall be described using ISO 3166-1 alpha-2 codes. It shall be defined using a code data type.</skos:definition>
		<skos:prefLabel>Clinical trial authorisation country</skos:prefLabel>
		<idmp:isUMLAttributeOf rdf:resource="&idmp;clinicalTrialAuthorisation"/>
	</owl:NamedIndividual>
	
	<owl:NamedIndividual rdf:about="&idmp;clinicalTrialAuthorisation.investigationCode">
		<rdf:type rdf:resource="&skos;Concept"/>
		<rdf:type rdf:resource="&upper;DataAttribute"/>
		<rdf:type rdf:resource="&upper;LogicalDataEntity"/>
		<skos:altLabel>IDMP.clinicalTrialAuthorisation.investigationCode</skos:altLabel>
		<skos:definition>The code for an investigational medicinal product as assigned locally for a clinical trial of a set of clinical trials shall be specified.</skos:definition>
		<skos:prefLabel>Investigation code</skos:prefLabel>
		<idmp:isUMLAttributeOf rdf:resource="&idmp;clinicalTrialAuthorisation"/>
	</owl:NamedIndividual>
	
	<owl:NamedIndividual rdf:about="&idmp;clinicalTrialAuthorisation.jurisdictionalInvestigationCode">
		<rdf:type rdf:resource="&skos;Concept"/>
		<rdf:type rdf:resource="&upper;DataAttribute"/>
		<rdf:type rdf:resource="&upper;LogicalDataEntity"/>
		<skos:altLabel>IDMP.clinicalTrialAuthorisation.jurisdictionalInvestigationCode</skos:altLabel>
		<skos:definition>The code for an investigational medicinal product as assigned in a jurisdiction for a clinical trial of a set of clinical trials shall be specified.</skos:definition>
		<skos:prefLabel>Jurisdictional investigation code</skos:prefLabel>
		<idmp:isUMLAttributeOf rdf:resource="&idmp;clinicalTrialAuthorisation"/>
	</owl:NamedIndividual>
	
	<owl:NamedIndividual rdf:about="&idmp;clinicalTrialAuthorisation.localClinicalTrialAuthorisation">
		<rdf:type rdf:resource="&skos;Concept"/>
		<rdf:type rdf:resource="&upper;DataAttribute"/>
		<rdf:type rdf:resource="&upper;LogicalDataEntity"/>
		<skos:altLabel>IDMP.clinicalTrialAuthorisation.localClinicalTrialAuthorisation</skos:altLabel>
		<skos:definition>Local information in relation to a clinical trial authorization (e.g. in a country within a jurisdiction) as granted by a medicines regulatory authority shall be specified, where applicable</skos:definition>
		<skos:prefLabel>Local clinical trial authorisation</skos:prefLabel>
		<idmp:isUMLAttributeOf rdf:resource="&idmp;clinicalTrialAuthorisation"/>
	</owl:NamedIndividual>
	
	<owl:NamedIndividual rdf:about="&idmp;clinicalTrialAuthorisation.productClassification">
		<rdf:type rdf:resource="&skos;Concept"/>
		<rdf:type rdf:resource="&upper;DataAttribute"/>
		<rdf:type rdf:resource="&upper;LogicalDataEntity"/>
		<skos:altLabel>IDMP.clinicalTrialAuthorisation.productClassification</skos:altLabel>
		<skos:definition>If the investigational medicinal product designated in the indication(s) as an orphan drug this shall be set to the value or values of the orphan drug designation reference number(s) within the Product Classification.</skos:definition>
		<skos:prefLabel>Product classification</skos:prefLabel>
		<idmp:isUMLAttributeOf rdf:resource="&idmp;clinicalTrialAuthorisation"/>
	</owl:NamedIndividual>
	
	<owl:NamedIndividual rdf:about="&idmp;clinicalTrialAuthorisation.registrationNumber">
		<rdf:type rdf:resource="&skos;Concept"/>
		<rdf:type rdf:resource="&upper;DataAttribute"/>
		<rdf:type rdf:resource="&upper;LogicalDataEntity"/>
		<skos:altLabel>IDMP.clinicalTrialAuthorisation.registrationNumber</skos:altLabel>
		<skos:definition>The registration number (identifier) for a clinical trial in a jurisdiction shall be specified, where applicable.</skos:definition>
		<skos:prefLabel>Registration number</skos:prefLabel>
		<idmp:isUMLAttributeOf rdf:resource="&idmp;clinicalTrialAuthorisation"/>
	</owl:NamedIndividual>
	
	<owl:AnnotationProperty rdf:about="&idmp;hasUMLAttribute">
	</owl:AnnotationProperty>
	
	<owl:NamedIndividual rdf:about="&idmp;indication">
		<rdf:type rdf:resource="&owl;Class"/>
		<rdf:type rdf:resource="&skos;Concept"/>
		<rdf:type rdf:resource="&upper;DataObject"/>
		<rdf:type rdf:resource="&upper;LogicalDataEntity"/>
		<rdfs:subClassOf rdf:resource="&skos;Concept"/>
		<skos:altLabel>IDMP.indication</skos:altLabel>
		<skos:definition>The authorized indication shall be specified using a controlled term and controlled term identifier of a controlled vocabulary, as applicable. This shall be specified using a CD data type. The authorized indication as described in the summary of product characteristics or the product labelling shall be also described using the Original Text part of the CD data type.</skos:definition>
		<skos:example>Treatment of exocrine pancreatic insufficiency due to cystic fibrosis, or other conditions.</skos:example>
		<skos:prefLabel>Indication</skos:prefLabel>
		<skos:related rdf:resource="&idmp;PhPIDSet"/>
		<skos:related rdf:resource="&idmp;pharmaceuticalProduct"/>
		<idmp:hasUMLAttribute rdf:resource="&idmp;indication.gender"/>
		<idmp:hasUMLAttribute rdf:resource="&idmp;indication.indication"/>
		<idmp:hasUMLAttribute rdf:resource="&idmp;indication.targetAge"/>
		<idmp:hasUMLAttribute rdf:resource="&idmp;indication.targetPopulation"/>
		<idmp:hasUMLAttribute rdf:resource="&idmp;indication.therapeuticUse"/>
		<idmp:hasUMLAttribute rdf:resource="&idmp;indication.underlyingDisease"/>
	</owl:NamedIndividual>
	
	<owl:NamedIndividual rdf:about="&idmp;indication.gender">
		<rdf:type rdf:resource="&skos;Concept"/>
		<rdf:type rdf:resource="&upper;DataAttribute"/>
		<rdf:type rdf:resource="&upper;LogicalDataEntity"/>
		<skos:altLabel>IDMP.indication.gender</skos:altLabel>
		<skos:definition>The target gender as authorized for the medicinal product shall be specified using the ISO/IEC 5218:2004 and held in a CD data type. EXAMPLE For the treatment of men with prostate cancer has gender code male.</skos:definition>
		<skos:prefLabel>Gender</skos:prefLabel>
		<idmp:isUMLAttributeOf rdf:resource="&idmp;indication"/>
	</owl:NamedIndividual>
	
	<owl:NamedIndividual rdf:about="&idmp;indication.indication">
		<rdf:type rdf:resource="&skos;Concept"/>
		<rdf:type rdf:resource="&upper;DataAttribute"/>
		<rdf:type rdf:resource="&upper;LogicalDataEntity"/>
		<skos:altLabel>IDMP.indication.indication</skos:altLabel>
		<skos:definition>The authorized indication shall be specified using a controlled term and controlled term identifier of a controlled vocabulary, as applicable. This shall be specified using a code data type. The authorized indication as described in the summary of product characteristics or the product labelling shall be also described using the Original Text part of the code data type. EXAMPLE Treatment of exocrine pancreatic insufficiency due to cystic fibrosis, or other conditions.</skos:definition>
		<skos:prefLabel>Indication attribute</skos:prefLabel>
		<idmp:isUMLAttributeOf rdf:resource="&idmp;indication"/>
	</owl:NamedIndividual>
	
	<owl:NamedIndividual rdf:about="&idmp;indication.targetAge">
		<rdf:type rdf:resource="&skos;Concept"/>
		<rdf:type rdf:resource="&upper;DataAttribute"/>
		<rdf:type rdf:resource="&upper;LogicalDataEntity"/>
		<skos:altLabel>IDMP.indication.targetAge</skos:altLabel>
		<skos:definition>The age range or age group of the target population as authorized for the medicinal product shall be specified based on a value drawn from ain international reference terminology. EXAMPLE For children older than 12 months and younger than 4 years.</skos:definition>
		<skos:prefLabel>Target age</skos:prefLabel>
		<idmp:isUMLAttributeOf rdf:resource="&idmp;indication"/>
	</owl:NamedIndividual>
	
	<owl:NamedIndividual rdf:about="&idmp;indication.targetPopulation">
		<rdf:type rdf:resource="&skos;Concept"/>
		<rdf:type rdf:resource="&upper;DataAttribute"/>
		<rdf:type rdf:resource="&upper;LogicalDataEntity"/>
		<skos:altLabel>IDMP.indication.targetPopulation</skos:altLabel>
		<skos:definition>The target population for which the medicinal product is indicated shall be specified using a term and a term identifier from a controlled vocabulary, as applicable. EXAMPLE For adults, children, elderly.</skos:definition>
		<skos:prefLabel>Target population</skos:prefLabel>
		<idmp:isUMLAttributeOf rdf:resource="&idmp;indication"/>
	</owl:NamedIndividual>
	
	<owl:NamedIndividual rdf:about="&idmp;indication.therapeuticUse">
		<rdf:type rdf:resource="&skos;Concept"/>
		<rdf:type rdf:resource="&upper;DataAttribute"/>
		<rdf:type rdf:resource="&upper;LogicalDataEntity"/>
		<skos:altLabel>IDMP.indication.therapeuticUse</skos:altLabel>
		<skos:definition>The authorized therapeutic use shall be specified using a term and a term identifier from a controlled vocabulary as applicable. EXAMPLE Prophylaxis, diagnosis, treatment.</skos:definition>
		<skos:prefLabel>Therapeutic use</skos:prefLabel>
		<idmp:isUMLAttributeOf rdf:resource="&idmp;indication"/>
	</owl:NamedIndividual>
	
	<owl:NamedIndividual rdf:about="&idmp;indication.underlyingDisease">
		<rdf:type rdf:resource="&skos;Concept"/>
		<rdf:type rdf:resource="&upper;DataAttribute"/>
		<rdf:type rdf:resource="&upper;LogicalDataEntity"/>
		<skos:altLabel>IDMP.indication.underlyingDisease</skos:altLabel>
		<skos:definition>The underlying disease as referenced in the summary of product characteristics or the product labelling shall be specified using a term and a term identifier from a controlled vocabulary, as applicable. EXAMPLE Treatment of exocrine pancreatic insufficiency due to cystic fibrosis, or other conditions.</skos:definition>
		<skos:prefLabel>Underlying disease</skos:prefLabel>
		<idmp:isUMLAttributeOf rdf:resource="&idmp;indication"/>
	</owl:NamedIndividual>
	
	<owl:NamedIndividual rdf:about="&idmp;investigationalMedicinalProductBatchIdentifier">
		<rdf:type rdf:resource="&owl;Class"/>
		<rdf:type rdf:resource="&skos;Concept"/>
		<rdf:type rdf:resource="&upper;DataObject"/>
		<rdf:type rdf:resource="&upper;LogicalDataEntity"/>
		<rdfs:subClassOf rdf:resource="&skos;Concept"/>
		<skos:altLabel>IDMP.investigationalMedicinalProductBatchIdentifier</skos:altLabel>
		<skos:definition>Application identifier assigned to a specific manufactured item resulting from a manufacturing process at a specific point of time</skos:definition>
		<skos:prefLabel>Investigational medicinal product batch identifier</skos:prefLabel>
		<skos:related rdf:resource="&idmp;IMPIDAttributeSet"/>
	</owl:NamedIndividual>
	
	<owl:NamedIndividual rdf:about="&idmp;investigationalMedicinalProductName">
		<rdf:type rdf:resource="&owl;Class"/>
		<rdf:type rdf:resource="&skos;Concept"/>
		<rdf:type rdf:resource="&upper;DataObject"/>
		<rdf:type rdf:resource="&upper;LogicalDataEntity"/>
		<rdfs:subClassOf rdf:resource="&skos;Concept"/>
		<skos:altLabel>IDMP.investigationalMedicinalProductName</skos:altLabel>
		<skos:definition>Name of pharmaceutical form of an active substance or placebo being tested or used as a reference in a clinical trial, including products already with a marketing authorisation but used or assembled (formulated or packaged) in a way different from the authorised form, or when used for an unauthorised indication, or when used to gain further information about the authorised form</skos:definition>
		<skos:prefLabel>Investigational medicinal product name</skos:prefLabel>
		<skos:related rdf:resource="&idmp;IMPIDAttributeSet"/>
		<idmp:hasUMLAttribute rdf:resource="&idmp;InvestigationalMedicinalProductName.code"/>
		<idmp:hasUMLAttribute rdf:resource="&idmp;InvestigationalMedicinalProductName.containerPart"/>
		<idmp:hasUMLAttribute rdf:resource="&idmp;InvestigationalMedicinalProductName.devicePart"/>
		<idmp:hasUMLAttribute rdf:resource="&idmp;InvestigationalMedicinalProductName.intendedUsePart"/>
		<idmp:hasUMLAttribute rdf:resource="&idmp;InvestigationalMedicinalProductName.inventedNamePart"/>
		<idmp:hasUMLAttribute rdf:resource="&idmp;InvestigationalMedicinalProductName.language"/>
		<idmp:hasUMLAttribute rdf:resource="&idmp;InvestigationalMedicinalProductName.name"/>
		<idmp:hasUMLAttribute rdf:resource="&idmp;InvestigationalMedicinalProductName.pharmaceuticalDoseFormPart"/>
		<idmp:hasUMLAttribute rdf:resource="&idmp;InvestigationalMedicinalProductName.scientificNamePart"/>
		<idmp:hasUMLAttribute rdf:resource="&idmp;InvestigationalMedicinalProductName.strengthNamePart"/>
		<idmp:hasUMLAttribute rdf:resource="&idmp;InvestigationalMedicinalProductName.trademarkOrCompanyPart"/>
		<idmp:hasUMLAttribute rdf:resource="&idmp;InvestigationalMedicinalProductName.year"/>
		<idmp:hasUMLAttribute rdf:resource="&idmp;investigationalMedicinalProductName.country"/>
	</owl:NamedIndividual>
	
	<owl:NamedIndividual rdf:about="&idmp;investigationalMedicinalProductName.country">
		<rdf:type rdf:resource="&skos;Concept"/>
		<rdf:type rdf:resource="&upper;DataAttribute"/>
		<rdf:type rdf:resource="&upper;LogicalDataEntity"/>
		<skos:altLabel>IDMP.investigationalMedicinalProductName.country</skos:altLabel>
		<skos:definition>The jurisdiction(s) in which the clinical trial authorization was granted shall be described using ISO 3166-1 alpha-2 codes. It shall be defined using a code data type.</skos:definition>
		<skos:prefLabel>Investigational medicinal product name country</skos:prefLabel>
		<idmp:isUMLAttributeOf rdf:resource="&idmp;investigationalMedicinalProductName"/>
	</owl:NamedIndividual>
	
	<owl:NamedIndividual rdf:about="&idmp;investigationalMedicinalProductPackageBatchIdentifier">
		<rdf:type rdf:resource="&owl;Class"/>
		<rdf:type rdf:resource="&skos;Concept"/>
		<rdf:type rdf:resource="&upper;DataObject"/>
		<rdf:type rdf:resource="&upper;LogicalDataEntity"/>
		<rdfs:subClassOf rdf:resource="&skos;Concept"/>
		<skos:altLabel>IDMP.investigationalMedicinalProductPackageBatchIdentifier</skos:altLabel>
		<skos:definition>Specific manufacturing release of a product or item by the manufacturer</skos:definition>
		<skos:prefLabel>Investigational medicinal product package batch identifier</skos:prefLabel>
		<skos:related rdf:resource="&idmp;IPCIDAttributeSet"/>
	</owl:NamedIndividual>
	
	<owl:AnnotationProperty rdf:about="&idmp;isUMLAttributeOf">
	</owl:AnnotationProperty>
	
	<owl:NamedIndividual rdf:about="&idmp;localMarketingAuthorisation.GTIN">
		<rdf:type rdf:resource="&skos;Concept"/>
		<rdf:type rdf:resource="&upper;DataAttribute"/>
		<rdf:type rdf:resource="&upper;LogicalDataEntity"/>
		<skos:altLabel>IDMP.localMarketingAuthorisation.GTIN</skos:altLabel>
		<skos:definition>GS1 unique identifier of items that are traded (e.g. Pharmaceuticals, Medical Devices) in the supply chain NOTE 1 A Global Trade Item Number (GTIN) is used to identify any item upon which there is a need to retrieve predefined information and that may be priced or ordered or invoiced at any point in any supply chain. GTINs may be 8, 12, 13 or 14-digits in length. NOTE 2 A Global Trade Item Number (GTIN) is used to identify any item upon which there is a need to retrieve predefined information and that may be priced or ordered or invoiced at any point in any supply chain. GTINs may be 8, 12, 13 or 14-digits in length.</skos:definition>
		<skos:prefLabel>Local marketing authorisation gtin</skos:prefLabel>
		<idmp:isUMLAttributeOf rdf:resource="&idmp;localMarketingAuthorisationInformation"/>
	</owl:NamedIndividual>
	
	<owl:NamedIndividual rdf:about="&idmp;localMarketingAuthorisation.authorisationIdentifier">
		<rdf:type rdf:resource="&skos;Concept"/>
		<rdf:type rdf:resource="&upper;DataAttribute"/>
		<rdf:type rdf:resource="&upper;LogicalDataEntity"/>
		<skos:altLabel>IDMP.localMarketingAuthorisation.authorisationIdentifier</skos:altLabel>
		<skos:definition>The marketing authorization assigned locally within a jurisdiction shall be specified. EXAMPLE In a country a local marketing authorization number is assigned in addition to the authorization number designated at EU level for centrally authorized medicinal products</skos:definition>
		<skos:prefLabel>Authorisation identifier</skos:prefLabel>
		<idmp:isUMLAttributeOf rdf:resource="&idmp;localMarketingAuthorisationInformation"/>
	</owl:NamedIndividual>
	
	<owl:NamedIndividual rdf:about="&idmp;localMarketingAuthorisation.country">
		<rdf:type rdf:resource="&skos;Concept"/>
		<rdf:type rdf:resource="&upper;DataAttribute"/>
		<rdf:type rdf:resource="&upper;LogicalDataEntity"/>
		<skos:altLabel>IDMP.localMarketingAuthorisation.country</skos:altLabel>
		<skos:definition>The country/jurisdiction in which the local marketing authorization has been granted. It should be specified using the ISO 3166-1 alpha-2 codes (including EU).</skos:definition>
		<skos:prefLabel>Local marketing authorisation country</skos:prefLabel>
		<idmp:isUMLAttributeOf rdf:resource="&idmp;localMarketingAuthorisationInformation"/>
	</owl:NamedIndividual>
	
	<owl:NamedIndividual rdf:about="&idmp;localMarketingAuthorisation.legalStatusOfSupply">
		<rdf:type rdf:resource="&skos;Concept"/>
		<rdf:type rdf:resource="&upper;DataAttribute"/>
		<rdf:type rdf:resource="&upper;LogicalDataEntity"/>
		<skos:altLabel>IDMP.localMarketingAuthorisation.legalStatusOfSupply</skos:altLabel>
		<skos:definition>For medicinal products, which are available on medical prescription only, the regulatory medicines authorities may assign additional sub-categories locally, which shall be specified as applicable. A controlled vocabulary for different categories of legal status of supply shall be applied. The controlled term and the controlled term identifier shall be specified.</skos:definition>
		<skos:prefLabel>Local marketing authorisation legal status of supply</skos:prefLabel>
		<idmp:isUMLAttributeOf rdf:resource="&idmp;localMarketingAuthorisationInformation"/>
	</owl:NamedIndividual>
	
	<owl:NamedIndividual rdf:about="&idmp;localMarketingAuthorisation.marketingStart">
		<rdf:type rdf:resource="&skos;Concept"/>
		<rdf:type rdf:resource="&upper;DataAttribute"/>
		<rdf:type rdf:resource="&upper;LogicalDataEntity"/>
		<skos:altLabel>IDMP.localMarketingAuthorisation.marketingStart</skos:altLabel>
		<skos:definition>The date when the medicinal product is “placed on the market” by the marketing authorization holder or where applicable the manufacturer/distributor- shall be provided. The date of “placed on the market” refers to the date of release of the medicinal product into the distribution chain. A complete date consisting of day, month and year shall be specified using the ISO 8601 date format.</skos:definition>
		<skos:prefLabel>Marketing start</skos:prefLabel>
		<idmp:isUMLAttributeOf rdf:resource="&idmp;localMarketingAuthorisationInformation"/>
	</owl:NamedIndividual>
	
	<owl:NamedIndividual rdf:about="&idmp;localMarketingAuthorisation.marketingStop">
		<rdf:type rdf:resource="&skos;Concept"/>
		<rdf:type rdf:resource="&upper;DataAttribute"/>
		<rdf:type rdf:resource="&upper;LogicalDataEntity"/>
		<skos:altLabel>IDMP.localMarketingAuthorisation.marketingStop</skos:altLabel>
		<skos:definition>The date when a medicinal product is no longer placed on the market by the marketing authorization holder or where applicable the manufacturer/distributor- shall be provided. A complete date consisting of day, month and year should be specified shall be specified using the ISO 8601 date format.</skos:definition>
		<skos:prefLabel>Marketing stop</skos:prefLabel>
		<idmp:isUMLAttributeOf rdf:resource="&idmp;localMarketingAuthorisationInformation"/>
	</owl:NamedIndividual>
	
	<owl:NamedIndividual rdf:about="&idmp;localMarketingAuthorisationInformation">
		<rdf:type rdf:resource="&owl;Class"/>
		<rdf:type rdf:resource="&skos;Concept"/>
		<rdf:type rdf:resource="&upper;DataObject"/>
		<rdf:type rdf:resource="&upper;LogicalDataEntity"/>
		<rdfs:subClassOf rdf:resource="&skos;Concept"/>
		<skos:altLabel>IDMP.localMarketingAuthorisationInformation</skos:altLabel>
		<skos:definition>Local marketing authorization is intended to provide for additional local information in a jurisdiction</skos:definition>
		<skos:prefLabel>Local marketing authorisation information</skos:prefLabel>
		<idmp:hasUMLAttribute rdf:resource="&idmp;localMarketingAuthorisation.GTIN"/>
		<idmp:hasUMLAttribute rdf:resource="&idmp;localMarketingAuthorisation.authorisationIdentifier"/>
		<idmp:hasUMLAttribute rdf:resource="&idmp;localMarketingAuthorisation.country"/>
		<idmp:hasUMLAttribute rdf:resource="&idmp;localMarketingAuthorisation.legalStatusOfSupply"/>
		<idmp:hasUMLAttribute rdf:resource="&idmp;localMarketingAuthorisation.marketingStart"/>
		<idmp:hasUMLAttribute rdf:resource="&idmp;localMarketingAuthorisation.marketingStop"/>
	</owl:NamedIndividual>
	
	<owl:NamedIndividual rdf:about="&idmp;manufacturedItem">
		<rdf:type rdf:resource="&owl;Class"/>
		<rdf:type rdf:resource="&skos;Concept"/>
		<rdf:type rdf:resource="&upper;DataObject"/>
		<rdf:type rdf:resource="&upper;LogicalDataEntity"/>
		<rdfs:subClassOf rdf:resource="&skos;Concept"/>
		<skos:altLabel>IDMP.manufacturedItem</skos:altLabel>
		<skos:definition>Description of the qualitative and quantitative composition of the product as contained in the packaging of the medicinal product. A medicinal product may contain one or more manufactured items. In many instances the manufactured item is equal to the pharmaceutical product. However, there are instances where the manufactured item(s) must undergo a transformation before being administered to the patient (as the pharmaceutical product) and the two are not equal. The manufactured item is not in direct contact with the outer packaging except where the outer packaging also serves as the immediate container.</skos:definition>
		<skos:prefLabel>Manufactured item</skos:prefLabel>
		<skos:related rdf:resource="&idmp;packageItem"/>
		<idmp:hasUMLAttribute rdf:resource="&idmp;manufacturedItem.ingredientSet"/>
		<idmp:hasUMLAttribute rdf:resource="&idmp;manufacturedItem.manufacturedDoseForm"/>
		<idmp:hasUMLAttribute rdf:resource="&idmp;manufacturedItem.packSize"/>
		<idmp:hasUMLAttribute rdf:resource="&idmp;manufacturedItem.unitOfPresentation"/>
	</owl:NamedIndividual>
	
	<owl:NamedIndividual rdf:about="&idmp;manufacturedItem.ingredientSet">
		<rdf:type rdf:resource="&skos;Concept"/>
		<rdf:type rdf:resource="&upper;DataAttribute"/>
		<rdf:type rdf:resource="&upper;LogicalDataEntity"/>
		<skos:altLabel>IDMP.manufacturedItem.ingredientSet</skos:altLabel>
		<skos:definition>Reference attribute from Ingredient class</skos:definition>
		<skos:prefLabel>Manufactured item ingredient set</skos:prefLabel>
		<idmp:isUMLAttributeOf rdf:resource="&idmp;manufacturedItem"/>
	</owl:NamedIndividual>
	
	<owl:NamedIndividual rdf:about="&idmp;manufacturedItem.manufacturedDoseForm">
		<rdf:type rdf:resource="&skos;Concept"/>
		<rdf:type rdf:resource="&upper;DataAttribute"/>
		<rdf:type rdf:resource="&upper;LogicalDataEntity"/>
		<skos:altLabel>IDMP.manufacturedItem.manufacturedDoseForm</skos:altLabel>
		<skos:definition>This describes the pharmaceutical dose form of the pharmaceutical item as supplied by the manufacturer. A term and a term identifier as defined in ISO/DIS 11239 and the resulting controlled vocabulary shall be specified. It is to be provided using a CD data type. EXAMPLE Values are: Tablet, Capsule, Oral Solution, Powder for solution for injection.</skos:definition>
		<skos:prefLabel>Manufactured dose form</skos:prefLabel>
		<idmp:isUMLAttributeOf rdf:resource="&idmp;manufacturedItem"/>
	</owl:NamedIndividual>
	
	<owl:NamedIndividual rdf:about="&idmp;manufacturedItem.packSize">
		<rdf:type rdf:resource="&skos;Concept"/>
		<rdf:type rdf:resource="&upper;DataAttribute"/>
		<rdf:type rdf:resource="&upper;LogicalDataEntity"/>
		<skos:altLabel>IDMP.manufacturedItem.packSize</skos:altLabel>
		<skos:definition>This is the size of the ‘Manufactured Item’. It shall be specified using a PQ data type and the units shall be specified as a symbol and a symbol identifier as defined in ISO/DIS 11240 and the resulting controlled vocabulary.</skos:definition>
		<skos:prefLabel>Manufactured item pack size</skos:prefLabel>
		<idmp:isUMLAttributeOf rdf:resource="&idmp;manufacturedItem"/>
	</owl:NamedIndividual>
	
	<owl:NamedIndividual rdf:about="&idmp;manufacturedItem.unitOfPresentation">
		<rdf:type rdf:resource="&skos;Concept"/>
		<rdf:type rdf:resource="&upper;DataAttribute"/>
		<rdf:type rdf:resource="&upper;LogicalDataEntity"/>
		<skos:altLabel>IDMP.manufacturedItem.unitOfPresentation</skos:altLabel>
		<skos:definition>This specifies the “real world” units in which the ‘Pack Size’ of the ‘Manufactured Item’ is described. It is a term and a term identifier as defined in ISO/DIS 11239 and its resulting controlled vocabulary. It is to be specified using a CD data type.</skos:definition>
		<skos:prefLabel>Unit of presentation</skos:prefLabel>
		<skos:related rdf:resource="&idmp;packageItem"/>
		<idmp:isUMLAttributeOf rdf:resource="&idmp;manufacturedItem"/>
	</owl:NamedIndividual>
	
	<owl:NamedIndividual rdf:about="&idmp;manufacturingAuthorisation">
		<rdf:type rdf:resource="&owl;Class"/>
		<rdf:type rdf:resource="&skos;Concept"/>
		<rdf:type rdf:resource="&upper;DataObject"/>
		<rdf:type rdf:resource="&upper;LogicalDataEntity"/>
		<rdfs:subClassOf rdf:resource="&skos;Concept"/>
		<skos:altLabel>IDMP.manufacturingAuthorisation</skos:altLabel>
		<skos:definition>Details of the ‘Manufacturing Authorization ’ granted by a regulatory medicines authority shall be provided.</skos:definition>
		<skos:prefLabel>Manufacturing authorisation</skos:prefLabel>
		<skos:related rdf:resource="&idmp;marketingAuthorisation"/>
		<idmp:hasUMLAttribute rdf:resource="&idmp;manufacturingAuthorisation.authorisationAuthority"/>
		<idmp:hasUMLAttribute rdf:resource="&idmp;manufacturingAuthorisation.authorisationDate"/>
		<idmp:hasUMLAttribute rdf:resource="&idmp;manufacturingAuthorisation.holder"/>
	</owl:NamedIndividual>
	
	<owl:NamedIndividual rdf:about="&idmp;manufacturingAuthorisation.authorisationAuthority">
		<rdf:type rdf:resource="&skos;Concept"/>
		<rdf:type rdf:resource="&upper;DataAttribute"/>
		<rdf:type rdf:resource="&upper;LogicalDataEntity"/>
		<skos:altLabel>IDMP.manufacturingAuthorisation.authorisationAuthority</skos:altLabel>
		<skos:definition>Details in relation to the organisation that granted the manufacturing authorization shall be provided. This shall be specified using an ‘Organisation’ class</skos:definition>
		<skos:prefLabel>Authorisation authority</skos:prefLabel>
		<idmp:isUMLAttributeOf rdf:resource="&idmp;manufacturingAuthorisation"/>
	</owl:NamedIndividual>
	
	<owl:NamedIndividual rdf:about="&idmp;manufacturingAuthorisation.authorisationDate">
		<rdf:type rdf:resource="&skos;Concept"/>
		<rdf:type rdf:resource="&upper;DataAttribute"/>
		<rdf:type rdf:resource="&upper;LogicalDataEntity"/>
		<skos:altLabel>IDMP.manufacturingAuthorisation.authorisationDate</skos:altLabel>
		<skos:definition>The date when the manufacturing authorization was issued by the regulatory authority shall be specified usingthe ISO 8601 date format.</skos:definition>
		<skos:prefLabel>Manufacturing authorisation date of authorisation</skos:prefLabel>
		<idmp:isUMLAttributeOf rdf:resource="&idmp;manufacturingAuthorisation"/>
	</owl:NamedIndividual>
	
	<owl:NamedIndividual rdf:about="&idmp;manufacturingAuthorisation.holder">
		<rdf:type rdf:resource="&skos;Concept"/>
		<rdf:type rdf:resource="&upper;DataAttribute"/>
		<rdf:type rdf:resource="&upper;LogicalDataEntity"/>
		<skos:altLabel>IDMP.manufacturingAuthorisation.holder</skos:altLabel>
		<skos:definition>Details in relation to the organisation that holds the manufacturing authorization shall be provided. This shall be specified using an ‘Organisation’ class.</skos:definition>
		<skos:prefLabel>Manufacturing authorisation holder</skos:prefLabel>
		<idmp:isUMLAttributeOf rdf:resource="&idmp;manufacturingAuthorisation"/>
	</owl:NamedIndividual>
	
	<owl:NamedIndividual rdf:about="&idmp;marketingAuthorisation">
		<rdf:type rdf:resource="&owl;Class"/>
		<rdf:type rdf:resource="&skos;Concept"/>
		<rdf:type rdf:resource="&upper;DataObject"/>
		<rdf:type rdf:resource="&upper;LogicalDataEntity"/>
		<rdfs:subClassOf rdf:resource="&skos;Concept"/>
		<skos:altLabel>IDMP.marketingAuthorisation</skos:altLabel>
		<skos:definition>Authorization issued from a medicines regulatory authority that a medicinal product may be placed on the market</skos:definition>
		<skos:prefLabel>Marketing authorisation</skos:prefLabel>
		<skos:related rdf:resource="&idmp;MPIDAttributeSet"/>
		<skos:related rdf:resource="&idmp;Organisation"/>
		<skos:related rdf:resource="&idmp;PCIDAttributeSet"/>
		<skos:related rdf:resource="&idmp;localMarketingAuthorisationInformation"/>
		<skos:related rdf:resource="&idmp;marketingAuthorisation"/>
		<idmp:hasUMLAttribute rdf:resource="&idmp;marketingAuthorisation.GTIN"/>
		<idmp:hasUMLAttribute rdf:resource="&idmp;marketingAuthorisation.authorisationDate"/>
		<idmp:hasUMLAttribute rdf:resource="&idmp;marketingAuthorisation.authorisedCombinedPharmaceuticalDoseForm"/>
		<idmp:hasUMLAttribute rdf:resource="&idmp;marketingAuthorisation.country"/>
		<idmp:hasUMLAttribute rdf:resource="&idmp;marketingAuthorisation.holder"/>
		<idmp:hasUMLAttribute rdf:resource="&idmp;marketingAuthorisation.legalStatusOfSupply"/>
		<idmp:hasUMLAttribute rdf:resource="&idmp;marketingAuthorisation.marketingAuthorisationNumber"/>
		<idmp:hasUMLAttribute rdf:resource="&idmp;marketingAuthorisation.productClassification"/>
		<idmp:hasUMLAttribute rdf:resource="&idmp;marketingAuthorisation.regulator"/>
		<idmp:hasUMLAttribute rdf:resource="&idmp;marketingAuthorisation.status"/>
	</owl:NamedIndividual>
	
	<owl:NamedIndividual rdf:about="&idmp;marketingAuthorisation.GTIN">
		<rdf:type rdf:resource="&skos;Concept"/>
		<rdf:type rdf:resource="&upper;DataAttribute"/>
		<rdf:type rdf:resource="&upper;LogicalDataEntity"/>
		<skos:altLabel>IDMP.marketingAuthorisation.GTIN</skos:altLabel>
		<skos:definition>Unique identifier of items that are traded (e.g. Pharmaceuticals, Medical Devices) in the supply chain. A Global Trade Item Number (GTIN) is used to identify any item upon which there is a need to retrieve predefined information and that may be priced or ordered or invoiced at any point in any supply chain. GTINs may be 8, 12, 13 or 14-digits in length.</skos:definition>
		<skos:prefLabel>Marketing authorisation gtin</skos:prefLabel>
		<idmp:isUMLAttributeOf rdf:resource="&idmp;marketingAuthorisation"/>
	</owl:NamedIndividual>
	
	<owl:NamedIndividual rdf:about="&idmp;marketingAuthorisation.authorisationDate">
		<rdf:type rdf:resource="&skos;Concept"/>
		<rdf:type rdf:resource="&upper;DataAttribute"/>
		<rdf:type rdf:resource="&upper;LogicalDataEntity"/>
		<skos:altLabel>IDMP.marketingAuthorisation.authorisationDate</skos:altLabel>
		<skos:definition>The date when the manufacturing authorization was issued by the regulatory authority shall be specified using the ISO 8601 date format.</skos:definition>
		<skos:prefLabel>Marketing authorisation date of authorisation</skos:prefLabel>
		<idmp:isUMLAttributeOf rdf:resource="&idmp;marketingAuthorisation"/>
	</owl:NamedIndividual>
	
	<owl:NamedIndividual rdf:about="&idmp;marketingAuthorisation.authorisedCombinedPharmaceuticalDoseForm">
		<rdf:type rdf:resource="&skos;Concept"/>
		<rdf:type rdf:resource="&upper;DataAttribute"/>
		<rdf:type rdf:resource="&upper;LogicalDataEntity"/>
		<skos:altLabel>IDMP.marketingAuthorisation.authorisedCombinedPharmaceuticalDoseForm</skos:altLabel>
		<skos:definition>Where the Pharmaceutical Dose Form is a compound expression made from two constituent dose forms the authorized name for the combination shall be held in this attribute. It shall be held in a code data type.</skos:definition>
		<skos:prefLabel>Authorised combined pharmaceutical dose form</skos:prefLabel>
		<idmp:isUMLAttributeOf rdf:resource="&idmp;marketingAuthorisation"/>
	</owl:NamedIndividual>
	
	<owl:NamedIndividual rdf:about="&idmp;marketingAuthorisation.country">
		<rdf:type rdf:resource="&skos;Concept"/>
		<rdf:type rdf:resource="&upper;DataAttribute"/>
		<rdf:type rdf:resource="&upper;LogicalDataEntity"/>
		<skos:altLabel>IDMP.marketingAuthorisation.country</skos:altLabel>
		<skos:definition>This code segment shall reflect the country code of that jurisdiction, where the medicinal product is authorized [ISO 3166-1-alpha-2 code elements].</skos:definition>
		<skos:prefLabel>Marketing authorisation country</skos:prefLabel>
		<idmp:isUMLAttributeOf rdf:resource="&idmp;marketingAuthorisation"/>
	</owl:NamedIndividual>
	
	<owl:NamedIndividual rdf:about="&idmp;marketingAuthorisation.holder">
		<rdf:type rdf:resource="&skos;Concept"/>
		<rdf:type rdf:resource="&upper;DataAttribute"/>
		<rdf:type rdf:resource="&upper;LogicalDataEntity"/>
		<skos:altLabel>IDMP.marketingAuthorisation.holder</skos:altLabel>
		<skos:definition>Entity/organisation that holds the authorization for the manufacturing process</skos:definition>
		<skos:prefLabel>Marketing authorisation holder</skos:prefLabel>
		<idmp:isUMLAttributeOf rdf:resource="&idmp;marketingAuthorisation"/>
	</owl:NamedIndividual>
	
	<owl:NamedIndividual rdf:about="&idmp;marketingAuthorisation.legalStatusOfSupply">
		<rdf:type rdf:resource="&skos;Concept"/>
		<rdf:type rdf:resource="&upper;DataAttribute"/>
		<rdf:type rdf:resource="&upper;LogicalDataEntity"/>
		<skos:altLabel>IDMP.marketingAuthorisation.legalStatusOfSupply</skos:altLabel>
		<skos:definition>Marketing Authorization in relation to the jurisdiction and the legal status of supply (e.g. prescription only or OTC)</skos:definition>
		<skos:prefLabel>Marketing authorisation legal status of supply</skos:prefLabel>
		<idmp:isUMLAttributeOf rdf:resource="&idmp;marketingAuthorisation"/>
	</owl:NamedIndividual>
	
	<owl:NamedIndividual rdf:about="&idmp;marketingAuthorisation.marketingAuthorisationNumber">
		<rdf:type rdf:resource="&skos;Concept"/>
		<rdf:type rdf:resource="&upper;DataAttribute"/>
		<rdf:type rdf:resource="&upper;LogicalDataEntity"/>
		<skos:altLabel>IDMP.marketingAuthorisation.marketingAuthorisationNumber</skos:altLabel>
		<skos:definition>Code or identifier assigned by a medicines regulatory authority to a medicinal product</skos:definition>
		<skos:prefLabel>Marketing authorisation number</skos:prefLabel>
		<idmp:isUMLAttributeOf rdf:resource="&idmp;marketingAuthorisation"/>
	</owl:NamedIndividual>
	
	<owl:NamedIndividual rdf:about="&idmp;marketingAuthorisation.productClassification">
		<rdf:type rdf:resource="&skos;Concept"/>
		<rdf:type rdf:resource="&upper;DataAttribute"/>
		<rdf:type rdf:resource="&upper;LogicalDataEntity"/>
		<skos:altLabel>IDMP.marketingAuthorisation.productClassification</skos:altLabel>
		<skos:definition>A means of identifying any external classification system to which the product belongs.</skos:definition>
		<skos:prefLabel>Product classification</skos:prefLabel>
		<skos:related rdf:resource="&idmp;MPIDAttributeSet"/>
		<idmp:isUMLAttributeOf rdf:resource="&idmp;marketingAuthorisation"/>
	</owl:NamedIndividual>
	
	<owl:NamedIndividual rdf:about="&idmp;marketingAuthorisation.regulator">
		<rdf:type rdf:resource="&skos;Concept"/>
		<rdf:type rdf:resource="&upper;DataAttribute"/>
		<rdf:type rdf:resource="&upper;LogicalDataEntity"/>
		<skos:altLabel>IDMP.marketingAuthorisation.regulator</skos:altLabel>
		<skos:definition>Details in relation to the regulatory medicines authority that granted the marketing authorization in a jurisdiction shall be specified using an Organisation class</skos:definition>
		<skos:prefLabel>Marketing authorisation regulator</skos:prefLabel>
		<idmp:isUMLAttributeOf rdf:resource="&idmp;marketingAuthorisation"/>
	</owl:NamedIndividual>
	
	<owl:NamedIndividual rdf:about="&idmp;marketingAuthorisation.status">
		<rdf:type rdf:resource="&skos;Concept"/>
		<rdf:type rdf:resource="&upper;DataAttribute"/>
		<rdf:type rdf:resource="&upper;LogicalDataEntity"/>
		<skos:altLabel>IDMP.marketingAuthorisation.status</skos:altLabel>
		<skos:definition>The status of the marketing authorizationshall be specified using a code data type. EXAMPLE Active, Suspended, Expired, Revoked</skos:definition>
		<skos:prefLabel>Marketing authorisation status</skos:prefLabel>
		<idmp:isUMLAttributeOf rdf:resource="&idmp;marketingAuthorisation"/>
	</owl:NamedIndividual>
	
	<owl:NamedIndividual rdf:about="&idmp;marketingAuthorisationProcedure">
		<rdf:type rdf:resource="&owl;Class"/>
		<rdf:type rdf:resource="&skos;Concept"/>
		<rdf:type rdf:resource="&upper;DataObject"/>
		<rdf:type rdf:resource="&upper;LogicalDataEntity"/>
		<rdfs:subClassOf rdf:resource="&skos;Concept"/>
		<dct:source>ISO IDMP 11615:2017</dct:source>
		<skos:altLabel>IDMP.Marketing Authorisation Procedure</skos:altLabel>
		<skos:definition>Marketing Authorisation Procedure formal procedure applied by a Medicines Regulatory Agency (3.1.56) to grant a marketing authorisation (3.1.40), amend an existing one, extend its duration or to withdraw it.Note 1 to entry: Marketing authorisation procedure and authorisation procedure (3.1.6) are synonymous.</skos:definition>
		<skos:prefLabel>Marketing authorisation procedure</skos:prefLabel>
		<skos:related rdf:resource="&idmp;marketingAuthorisation"/>
		<idmp:hasUMLAttribute rdf:resource="&idmp;marketingAuthorisationProcedure.date"/>
		<idmp:hasUMLAttribute rdf:resource="&idmp;marketingAuthorisationProcedure.documentIdentifier"/>
		<idmp:hasUMLAttribute rdf:resource="&idmp;marketingAuthorisationProcedure.procedureIdentifier"/>
		<idmp:hasUMLAttribute rdf:resource="&idmp;marketingAuthorisationProcedure.procedureReferenceCode"/>
		<idmp:hasUMLAttribute rdf:resource="&idmp;marketingAuthorisationProcedure.procedureType"/>
	</owl:NamedIndividual>
	
	<owl:NamedIndividual rdf:about="&idmp;marketingAuthorisationProcedure.date">
		<rdf:type rdf:resource="&skos;Concept"/>
		<rdf:type rdf:resource="&upper;DataAttribute"/>
		<rdf:type rdf:resource="&upper;LogicalDataEntity"/>
		<skos:altLabel>IDMP.marketingAuthorisationProcedure.date</skos:altLabel>
		<skos:definition>The date when the procedure described as ‘Procedure Type’, took effect. A complete date consisting of day, month and year shall be specified using the ISO 8601 date format.</skos:definition>
		<skos:prefLabel>Marketing authorisation procedure date</skos:prefLabel>
		<idmp:isUMLAttributeOf rdf:resource="&idmp;marketingAuthorisationProcedure"/>
	</owl:NamedIndividual>
	
	<owl:NamedIndividual rdf:about="&idmp;marketingAuthorisationProcedure.documentIdentifier">
		<rdf:type rdf:resource="&skos;Concept"/>
		<rdf:type rdf:resource="&upper;DataAttribute"/>
		<rdf:type rdf:resource="&upper;LogicalDataEntity"/>
		<skos:altLabel>IDMP.marketingAuthorisationProcedure.documentIdentifier</skos:altLabel>
		<skos:definition>The reference number of the regulatory document formally granting an authorization /update of an exisiting medicinal product authorization by the regulatory medicines agency in a jurisdiction shall be specified.</skos:definition>
		<skos:prefLabel>Document identifier</skos:prefLabel>
		<idmp:isUMLAttributeOf rdf:resource="&idmp;marketingAuthorisationProcedure"/>
	</owl:NamedIndividual>
	
	<owl:NamedIndividual rdf:about="&idmp;marketingAuthorisationProcedure.procedureIdentifier">
		<rdf:type rdf:resource="&skos;Concept"/>
		<rdf:type rdf:resource="&upper;DataAttribute"/>
		<rdf:type rdf:resource="&upper;LogicalDataEntity"/>
		<skos:altLabel>IDMP.marketingAuthorisationProcedure.procedureIdentifier</skos:altLabel>
		<skos:definition>The unique identifier for the specific instance of procedure shall be provided and defined using an II data type.</skos:definition>
		<skos:prefLabel>Procedure identifier</skos:prefLabel>
		<idmp:isUMLAttributeOf rdf:resource="&idmp;marketingAuthorisationProcedure"/>
	</owl:NamedIndividual>
	
	<owl:NamedIndividual rdf:about="&idmp;marketingAuthorisationProcedure.procedureReferenceCode">
		<rdf:type rdf:resource="&skos;Concept"/>
		<rdf:type rdf:resource="&upper;DataAttribute"/>
		<rdf:type rdf:resource="&upper;LogicalDataEntity"/>
		<skos:altLabel>IDMP.marketingAuthorisationProcedure.procedureReferenceCode</skos:altLabel>
		<skos:definition>The regulatory authorization procedure as applicable in a jurisdiction shall be specifiedauthorization . A controlled vocabulary for regulatory authorization procedures shall be applied. The controlled term and the controlled term identifier shall be specified. EXAMPLE Central authorization procedure in the EU, a product marketed under an approved Biologic License Application (BLA) in the US.</skos:definition>
		<skos:prefLabel>Procedure reference code</skos:prefLabel>
		<idmp:isUMLAttributeOf rdf:resource="&idmp;marketingAuthorisationProcedure"/>
	</owl:NamedIndividual>
	
	<owl:NamedIndividual rdf:about="&idmp;marketingAuthorisationProcedure.procedureType">
		<rdf:type rdf:resource="&skos;Concept"/>
		<rdf:type rdf:resource="&upper;DataAttribute"/>
		<rdf:type rdf:resource="&upper;LogicalDataEntity"/>
		<skos:altLabel>IDMP.marketingAuthorisationProcedure.procedureType</skos:altLabel>
		<skos:definition>The procedure type shall be specified in relation to the marketing authorization authorization,. A controlled vocabulary for regulatory procedure types shall be applied. The controlled term and the controlled term identifier shall be specified.EXAMPLE Initial authorization, variation, renewal, line extension.</skos:definition>
		<skos:prefLabel>Procedure type</skos:prefLabel>
		<idmp:isUMLAttributeOf rdf:resource="&idmp;marketingAuthorisationProcedure"/>
	</owl:NamedIndividual>
	
	<owl:NamedIndividual rdf:about="&idmp;medicalDevice">
		<rdf:type rdf:resource="&owl;Class"/>
		<rdf:type rdf:resource="&skos;Concept"/>
		<rdf:type rdf:resource="&upper;DataObject"/>
		<rdf:type rdf:resource="&upper;LogicalDataEntity"/>
		<rdfs:subClassOf rdf:resource="&skos;Concept"/>
		<skos:altLabel>IDMP.medicalDevice</skos:altLabel>
		<skos:definition>Any instrument, apparatus, appliance, software, material or other article, whether used alone or in combination, including the software intended by its manufacturer to be used specifically for diagnostic and/or therapeutic purposes and necessary for its proper application, intended by the manufacturer to be used for human beings for the purpose of: Diagnosis, prevention, monitoring, treatment or alleviation of disease. Diagnosis, monitoring, treatment, alleviation of or compensation for an injury or handicap. Investigation, replacement or modification of the anatomy or of a physiological process. Control of conception, and which does not achieve its principal intended action in or on the human body by pharmacological, immunological or metabolic means, but which may be assisted in its function by such means.</skos:definition>
		<skos:prefLabel>Medical device</skos:prefLabel>
		<skos:related rdf:resource="&idmp;pharmaceuticalProduct"/>
		<idmp:hasUMLAttribute rdf:resource="&idmp;medicalDevice.UDI"/>
		<idmp:hasUMLAttribute rdf:resource="&idmp;medicalDevice.hasAllergens"/>
		<idmp:hasUMLAttribute rdf:resource="&idmp;medicalDevice.ingredientSet"/>
		<idmp:hasUMLAttribute rdf:resource="&idmp;medicalDevice.isSterile"/>
		<idmp:hasUMLAttribute rdf:resource="&idmp;medicalDevice.isSterilizationRequired"/>
		<idmp:hasUMLAttribute rdf:resource="&idmp;medicalDevice.manufacturer"/>
		<idmp:hasUMLAttribute rdf:resource="&idmp;medicalDevice.modelNumber"/>
		<idmp:hasUMLAttribute rdf:resource="&idmp;medicalDevice.name"/>
		<idmp:hasUMLAttribute rdf:resource="&idmp;medicalDevice.nomenclature"/>
		<idmp:hasUMLAttribute rdf:resource="&idmp;medicalDevice.otherCharacteristics"/>
		<idmp:hasUMLAttribute rdf:resource="&idmp;medicalDevice.physicalCharacteristics"/>
		<idmp:hasUMLAttribute rdf:resource="&idmp;medicalDevice.restrictedUseCount"/>
		<idmp:hasUMLAttribute rdf:resource="&idmp;medicalDevice.tradeName"/>
	</owl:NamedIndividual>
	
	<owl:NamedIndividual rdf:about="&idmp;medicalDevice.UDI">
		<rdf:type rdf:resource="&skos;Concept"/>
		<rdf:type rdf:resource="&upper;DataAttribute"/>
		<rdf:type rdf:resource="&upper;LogicalDataEntity"/>
		<skos:altLabel>IDMP.medicalDevice.UDI</skos:altLabel>
		<skos:definition>If the component has a Unique Device Identifier it should be recorded here.</skos:definition>
		<skos:prefLabel>Medical device udi</skos:prefLabel>
		<idmp:isUMLAttributeOf rdf:resource="&idmp;medicalDevice"/>
	</owl:NamedIndividual>
	
	<owl:NamedIndividual rdf:about="&idmp;medicalDevice.hasAllergens">
		<rdf:type rdf:resource="&skos;Concept"/>
		<rdf:type rdf:resource="&upper;DataAttribute"/>
		<rdf:type rdf:resource="&upper;LogicalDataEntity"/>
		<skos:altLabel>IDMP.medicalDevice.hasAllergens</skos:altLabel>
		<skos:definition>It shall be specified, if in accordance with the label or the instruction for use the medical device is containing allergens/materials of concern (Yes/No value).</skos:definition>
		<skos:prefLabel>Has allergens</skos:prefLabel>
		<idmp:isUMLAttributeOf rdf:resource="&idmp;medicalDevice"/>
	</owl:NamedIndividual>
	
	<owl:NamedIndividual rdf:about="&idmp;medicalDevice.ingredientSet">
		<rdf:type rdf:resource="&skos;Concept"/>
		<rdf:type rdf:resource="&upper;DataAttribute"/>
		<rdf:type rdf:resource="&upper;LogicalDataEntity"/>
		<skos:altLabel>IDMP.medicalDevice.ingredientSet</skos:altLabel>
		<skos:definition>Reference attribute from Ingredient class</skos:definition>
		<skos:prefLabel>Ingredient set</skos:prefLabel>
		<idmp:isUMLAttributeOf rdf:resource="&idmp;medicalDevice"/>
	</owl:NamedIndividual>
	
	<owl:NamedIndividual rdf:about="&idmp;medicalDevice.isSterile">
		<rdf:type rdf:resource="&skos;Concept"/>
		<rdf:type rdf:resource="&upper;DataAttribute"/>
		<rdf:type rdf:resource="&upper;LogicalDataEntity"/>
		<skos:altLabel>IDMP.medicalDevice.isSterile</skos:altLabel>
		<skos:definition>It shall be specified if the package for the medical device is sterile or not when supplied (Yes/No value).</skos:definition>
		<skos:prefLabel>Is sterile</skos:prefLabel>
		<idmp:isUMLAttributeOf rdf:resource="&idmp;medicalDevice"/>
	</owl:NamedIndividual>
	
	<owl:NamedIndividual rdf:about="&idmp;medicalDevice.isSterilizationRequired">
		<rdf:type rdf:resource="&skos;Concept"/>
		<rdf:type rdf:resource="&upper;DataAttribute"/>
		<rdf:type rdf:resource="&upper;LogicalDataEntity"/>
		<skos:altLabel>IDMP.medicalDevice.isSterilizationRequired</skos:altLabel>
		<skos:definition>It shall be specified if the medical device shall be sterilized before use (Yes/No value).</skos:definition>
		<skos:prefLabel>Is sterilization required</skos:prefLabel>
		<idmp:isUMLAttributeOf rdf:resource="&idmp;medicalDevice"/>
	</owl:NamedIndividual>
	
	<owl:NamedIndividual rdf:about="&idmp;medicalDevice.manufacturer">
		<rdf:type rdf:resource="&skos;Concept"/>
		<rdf:type rdf:resource="&upper;DataAttribute"/>
		<rdf:type rdf:resource="&upper;LogicalDataEntity"/>
		<skos:altLabel>IDMP.medicalDevice.manufacturer</skos:altLabel>
		<skos:definition>The trade name of the medical device shall be specified, where applicable.</skos:definition>
		<skos:prefLabel>Medical device manufacturer</skos:prefLabel>
		<idmp:isUMLAttributeOf rdf:resource="&idmp;medicalDevice"/>
	</owl:NamedIndividual>
	
	<owl:NamedIndividual rdf:about="&idmp;medicalDevice.modelNumber">
		<rdf:type rdf:resource="&skos;Concept"/>
		<rdf:type rdf:resource="&upper;DataAttribute"/>
		<rdf:type rdf:resource="&upper;LogicalDataEntity"/>
		<skos:altLabel>IDMP.medicalDevice.modelNumber</skos:altLabel>
		<skos:definition>The device model or reference number shall be specified, where applicable.</skos:definition>
		<skos:prefLabel>Model number</skos:prefLabel>
		<idmp:isUMLAttributeOf rdf:resource="&idmp;medicalDevice"/>
	</owl:NamedIndividual>
	
	<owl:NamedIndividual rdf:about="&idmp;medicalDevice.name">
		<rdf:type rdf:resource="&skos;Concept"/>
		<rdf:type rdf:resource="&upper;DataAttribute"/>
		<rdf:type rdf:resource="&upper;LogicalDataEntity"/>
		<skos:altLabel>IDMP.medicalDevice.name</skos:altLabel>
		<skos:definition>Name of the device that is part of a pharmaceutical product</skos:definition>
		<skos:prefLabel>Medical device name</skos:prefLabel>
		<idmp:isUMLAttributeOf rdf:resource="&idmp;medicalDevice"/>
	</owl:NamedIndividual>
	
	<owl:NamedIndividual rdf:about="&idmp;medicalDevice.nomenclature">
		<rdf:type rdf:resource="&skos;Concept"/>
		<rdf:type rdf:resource="&upper;DataAttribute"/>
		<rdf:type rdf:resource="&upper;LogicalDataEntity"/>
		<skos:altLabel>IDMP.medicalDevice.nomenclature</skos:altLabel>
		<skos:definition>A global nomenclature code shall be specified of internationally recognised coded descriptors in the format of preferred terms with definitions used to generically identify medical devices and related health care products(e.g.: Global Medical Device Nomenclature (GMDN) as defined in ISO 15225).</skos:definition>
		<skos:prefLabel>Nomenclature</skos:prefLabel>
		<idmp:isUMLAttributeOf rdf:resource="&idmp;medicalDevice"/>
	</owl:NamedIndividual>
	
	<owl:NamedIndividual rdf:about="&idmp;medicalDevice.otherCharacteristics">
		<rdf:type rdf:resource="&skos;Concept"/>
		<rdf:type rdf:resource="&upper;DataAttribute"/>
		<rdf:type rdf:resource="&upper;LogicalDataEntity"/>
		<skos:altLabel>IDMP.medicalDevice.otherCharacteristics</skos:altLabel>
		<skos:definition>Zero or more other observations shall be made about the characteristics of the ‘Packaged Medicinal Product’, where applicable. They are represented by naming the characteristic in the ‘Code’ attribute using a CD data type, and then if required providing a ‘Value’ for the characteristic named using an ANY data type. This facility is useful for capturing unusual details not explicitly catered for in the other attributes.</skos:definition>
		<skos:prefLabel>Other characteristics</skos:prefLabel>
		<idmp:isUMLAttributeOf rdf:resource="&idmp;medicalDevice"/>
	</owl:NamedIndividual>
	
	<owl:NamedIndividual rdf:about="&idmp;medicalDevice.physicalCharacteristics">
		<rdf:type rdf:resource="&skos;Concept"/>
		<rdf:type rdf:resource="&upper;DataAttribute"/>
		<rdf:type rdf:resource="&upper;LogicalDataEntity"/>
		<skos:altLabel>IDMP.medicalDevice.physicalCharacteristics</skos:altLabel>
		<skos:definition>The physical attributes of the ‘Medical Device’ such as height, weight, width, depth, volume, colour and shape shall be provided. One or more images of the ‘Medical Device’ shall be included as applicable.</skos:definition>
		<skos:prefLabel>Physical characteristics</skos:prefLabel>
		<idmp:isUMLAttributeOf rdf:resource="&idmp;medicalDevice"/>
	</owl:NamedIndividual>
	
	<owl:NamedIndividual rdf:about="&idmp;medicalDevice.restrictedUseCount">
		<rdf:type rdf:resource="&skos;Concept"/>
		<rdf:type rdf:resource="&upper;DataAttribute"/>
		<rdf:type rdf:resource="&upper;LogicalDataEntity"/>
		<skos:altLabel>IDMP.medicalDevice.restrictedUseCount</skos:altLabel>
		<skos:definition>If the medical device&apos;s label indicates a limited number of times of use, the number shall be specified using an integer data type.</skos:definition>
		<skos:prefLabel>Restricted use count</skos:prefLabel>
		<idmp:isUMLAttributeOf rdf:resource="&idmp;medicalDevice"/>
	</owl:NamedIndividual>
	
	<owl:NamedIndividual rdf:about="&idmp;medicalDevice.tradeName">
		<rdf:type rdf:resource="&skos;Concept"/>
		<rdf:type rdf:resource="&upper;DataAttribute"/>
		<rdf:type rdf:resource="&upper;LogicalDataEntity"/>
		<skos:altLabel>IDMP.medicalDevice.tradeName</skos:altLabel>
		<skos:definition>The trade name of the medical device shall be specified, where applicable.</skos:definition>
		<skos:prefLabel>Trade name</skos:prefLabel>
		<idmp:isUMLAttributeOf rdf:resource="&idmp;medicalDevice"/>
	</owl:NamedIndividual>
	
	<owl:NamedIndividual rdf:about="&idmp;medicinalProductBatchIdentifier">
		<rdf:type rdf:resource="&owl;Class"/>
		<rdf:type rdf:resource="&skos;Concept"/>
		<rdf:type rdf:resource="&upper;DataObject"/>
		<rdf:type rdf:resource="&upper;LogicalDataEntity"/>
		<rdfs:subClassOf rdf:resource="&skos;Concept"/>
		<skos:altLabel>IDMP.medicinalProductBatchIdentifier</skos:altLabel>
		<skos:definition>Carries the batch number and the expiration date when created a medicinal product level.</skos:definition>
		<skos:prefLabel>Medicinal product batch identifier</skos:prefLabel>
		<skos:related rdf:resource="&idmp;MPIDAttributeSet"/>
		<idmp:hasUMLAttribute rdf:resource="&idmp;Medicinalproductbatchidentifier.batchId"/>
		<idmp:hasUMLAttribute rdf:resource="&idmp;medicinalProductBatchIdentifier.BAID1"/>
		<idmp:hasUMLAttribute rdf:resource="&idmp;medicinalProductBatchIdentifier.expirationDate"/>
	</owl:NamedIndividual>
	
	<owl:NamedIndividual rdf:about="&idmp;medicinalProductBatchIdentifier.BAID1">
		<rdf:type rdf:resource="&skos;Concept"/>
		<rdf:type rdf:resource="&upper;DataAttribute"/>
		<rdf:type rdf:resource="&upper;LogicalDataEntity"/>
		<skos:altLabel>IDMP.medicinalProductBatchIdentifier.BAID1</skos:altLabel>
		<skos:definition>Unique identifier allocated to a specific batch of an investigational medicinal product supplementary to any existing identifier as ascribed by a medicines regulatory authority in a jurisdiction and a batch number as assigned by a manufacturer. This is for indexing purposes and to contribute to improving patient safety by allowing for the unique identification of medicinal products worldwide.</skos:definition>
		<skos:prefLabel>Baid1</skos:prefLabel>
		<idmp:isUMLAttributeOf rdf:resource="&idmp;medicinalProductBatchIdentifier"/>
	</owl:NamedIndividual>
	
	<owl:NamedIndividual rdf:about="&idmp;medicinalProductBatchIdentifier.expirationDate">
		<rdf:type rdf:resource="&skos;Concept"/>
		<rdf:type rdf:resource="&upper;DataAttribute"/>
		<rdf:type rdf:resource="&upper;LogicalDataEntity"/>
		<skos:altLabel>IDMP.medicinalProductBatchIdentifier.expirationDate</skos:altLabel>
		<skos:definition>Optional attribute that specifies the expiration date of the batch</skos:definition>
		<skos:prefLabel>Medicinal product batch identifier expiration date</skos:prefLabel>
		<idmp:isUMLAttributeOf rdf:resource="&idmp;medicinalProductBatchIdentifier"/>
	</owl:NamedIndividual>
	
	<owl:NamedIndividual rdf:about="&idmp;medicinalProductName">
		<rdf:type rdf:resource="&owl;Class"/>
		<rdf:type rdf:resource="&skos;Concept"/>
		<rdf:type rdf:resource="&upper;DataObject"/>
		<rdf:type rdf:resource="&upper;LogicalDataEntity"/>
		<rdfs:subClassOf rdf:resource="&skos;Concept"/>
		<skos:altLabel>IDMP.medicinalProductName</skos:altLabel>
		<skos:definition>The name of the medicinal product as authorized by a medicines regulatory authority in a jurisdiction together with an analysis of the name into various parts.</skos:definition>
		<skos:prefLabel>Medicinal product name</skos:prefLabel>
		<skos:related rdf:resource="&idmp;MPIDAttributeSet"/>
		<idmp:hasUMLAttribute rdf:resource="&idmp;medicinalProductName.containerPart"/>
		<idmp:hasUMLAttribute rdf:resource="&idmp;medicinalProductName.country"/>
		<idmp:hasUMLAttribute rdf:resource="&idmp;medicinalProductName.devicePart"/>
		<idmp:hasUMLAttribute rdf:resource="&idmp;medicinalProductName.intendedUsePart"/>
		<idmp:hasUMLAttribute rdf:resource="&idmp;medicinalProductName.inventedNamePart"/>
		<idmp:hasUMLAttribute rdf:resource="&idmp;medicinalProductName.language"/>
		<idmp:hasUMLAttribute rdf:resource="&idmp;medicinalProductName.name"/>
		<idmp:hasUMLAttribute rdf:resource="&idmp;medicinalProductName.pharmaceuticalFormPart"/>
		<idmp:hasUMLAttribute rdf:resource="&idmp;medicinalProductName.scientificNamePart"/>
		<idmp:hasUMLAttribute rdf:resource="&idmp;medicinalProductName.strengthNamePart"/>
		<idmp:hasUMLAttribute rdf:resource="&idmp;medicinalProductName.trademarkOrCompanyPart"/>
		<idmp:hasUMLAttribute rdf:resource="&idmp;medicinalProductName.year"/>
	</owl:NamedIndividual>
	
	<owl:NamedIndividual rdf:about="&idmp;medicinalProductName.containerPart">
		<rdf:type rdf:resource="&skos;Concept"/>
		<rdf:type rdf:resource="&upper;DataAttribute"/>
		<rdf:type rdf:resource="&upper;LogicalDataEntity"/>
		<skos:altLabel>IDMP.medicinalProductName.containerPart</skos:altLabel>
		<skos:definition>The container, if reflected in the medicinal product name, shall be specified.EXAMPLE For the medicinal product name ‘LXA – 10 mg/ ml - Solution for injection – Subcutaneous use - Vial (glass) - 4 ml - 1 Vial’, the container part is ‘vial (glass)’.</skos:definition>
		<skos:prefLabel>Container part</skos:prefLabel>
		<idmp:isUMLAttributeOf rdf:resource="&idmp;medicinalProductName"/>
	</owl:NamedIndividual>
	
	<owl:NamedIndividual rdf:about="&idmp;medicinalProductName.country">
		<rdf:type rdf:resource="&skos;Concept"/>
		<rdf:type rdf:resource="&upper;DataAttribute"/>
		<rdf:type rdf:resource="&upper;LogicalDataEntity"/>
		<skos:altLabel>IDMP.medicinalProductName.country</skos:altLabel>
		<skos:definition>The country or jurisdiction where the medicinal product name is applicable shall be described using ISO 3166-1 alpha-2 codes. It shall be defined using a code data type.</skos:definition>
		<skos:prefLabel>Medicinal product name country</skos:prefLabel>
		<idmp:isUMLAttributeOf rdf:resource="&idmp;medicinalProductName"/>
	</owl:NamedIndividual>
	
	<owl:NamedIndividual rdf:about="&idmp;medicinalProductName.devicePart">
		<rdf:type rdf:resource="&skos;Concept"/>
		<rdf:type rdf:resource="&upper;DataAttribute"/>
		<rdf:type rdf:resource="&upper;LogicalDataEntity"/>
		<skos:altLabel>IDMP.medicinalProductName.devicePart</skos:altLabel>
		<skos:definition>The device, if reflected in the medicinal product name, shall be specified.EXAMPLE For the medicinal product name ‘LXA ‘Drug XYZ® Accuhaler 200 mg for adults’, the device part is ‘Accuhaler’.</skos:definition>
		<skos:prefLabel>Device part</skos:prefLabel>
		<idmp:isUMLAttributeOf rdf:resource="&idmp;medicinalProductName"/>
	</owl:NamedIndividual>
	
	<owl:NamedIndividual rdf:about="&idmp;medicinalProductName.intendedUsePart">
		<rdf:type rdf:resource="&skos;Concept"/>
		<rdf:type rdf:resource="&upper;DataAttribute"/>
		<rdf:type rdf:resource="&upper;LogicalDataEntity"/>
		<skos:altLabel>IDMP.medicinalProductName.intendedUsePart</skos:altLabel>
		<skos:definition>The intended use, if reflected in the medicinal product name, shall be specified. EXAMPLE For the medicinal product name ‘Drug-BI Caplets - Heartburn Relief’, the intended use part is ‘Heartburn Relief’.</skos:definition>
		<skos:prefLabel>Intended use part</skos:prefLabel>
		<idmp:isUMLAttributeOf rdf:resource="&idmp;medicinalProductName"/>
	</owl:NamedIndividual>
	
	<owl:NamedIndividual rdf:about="&idmp;medicinalProductName.inventedNamePart">
		<rdf:type rdf:resource="&skos;Concept"/>
		<rdf:type rdf:resource="&upper;DataAttribute"/>
		<rdf:type rdf:resource="&upper;LogicalDataEntity"/>
		<skos:altLabel>IDMP.medicinalProductName.inventedNamePart</skos:altLabel>
		<skos:definition>The invented name (i.e. trade name) of the medicinal product without e.g. the trademark or any other descriptors reflected in the product name shall be specified. EXAMPLE For the medicinal product name ‘Drug XYZ® Accuhaler 200 mg for adults’ the invented (trade) name element is ‘Drug XYZ’.</skos:definition>
		<skos:prefLabel>Invented name part</skos:prefLabel>
		<idmp:isUMLAttributeOf rdf:resource="&idmp;medicinalProductName"/>
	</owl:NamedIndividual>
	
	<owl:NamedIndividual rdf:about="&idmp;medicinalProductName.language">
		<rdf:type rdf:resource="&skos;Concept"/>
		<rdf:type rdf:resource="&upper;DataAttribute"/>
		<rdf:type rdf:resource="&upper;LogicalDataEntity"/>
		<skos:altLabel>IDMP.medicinalProductName.language</skos:altLabel>
		<skos:definition>The ISO 639-2 Language Code of the medicinal product name as applicable in the jurisdiction shall be specified. The Language shall be defined using a code data type.</skos:definition>
		<skos:prefLabel>Language code of medicinal product name</skos:prefLabel>
		<idmp:isUMLAttributeOf rdf:resource="&idmp;medicinalProductName"/>
	</owl:NamedIndividual>
	
	<owl:NamedIndividual rdf:about="&idmp;medicinalProductName.name">
		<rdf:type rdf:resource="&skos;Concept"/>
		<rdf:type rdf:resource="&upper;DataAttribute"/>
		<rdf:type rdf:resource="&upper;LogicalDataEntity"/>
		<skos:altLabel>IDMP.medicinalProductName.name</skos:altLabel>
		<skos:definition>Name of the medicinal product</skos:definition>
		<skos:prefLabel>Name of medicinal product</skos:prefLabel>
		<idmp:isUMLAttributeOf rdf:resource="&idmp;medicinalProductName"/>
	</owl:NamedIndividual>
	
	<owl:NamedIndividual rdf:about="&idmp;medicinalProductName.pharmaceuticalFormPart">
		<rdf:type rdf:resource="&skos;Concept"/>
		<rdf:type rdf:resource="&upper;DataAttribute"/>
		<rdf:type rdf:resource="&upper;LogicalDataEntity"/>
		<skos:altLabel>IDMP.medicinalProductName.pharmaceuticalFormPart</skos:altLabel>
		<skos:definition>The pharmaceutical dose form, if reflected in the medicinal product name, shall be specified. This pharmaceutical dose form name part may differ from the concept of ‘Administrable Dose Form’ and ‘Manufactured Dose Form’ as described in section X. EXAMPLE For the medicinal product name ‘Novo-DrugX EASY-TO-SWALLOW CAPLETS’, the pharmaceutical dose form name element is ‘EASY-TO-SWALLOW CAPLETS’.</skos:definition>
		<skos:prefLabel>Pharmaceutical form part</skos:prefLabel>
		<idmp:isUMLAttributeOf rdf:resource="&idmp;medicinalProductName"/>
	</owl:NamedIndividual>
	
	<owl:NamedIndividual rdf:about="&idmp;medicinalProductName.scientificNamePart">
		<rdf:type rdf:resource="&skos;Concept"/>
		<rdf:type rdf:resource="&upper;DataAttribute"/>
		<rdf:type rdf:resource="&upper;LogicalDataEntity"/>
		<skos:altLabel>IDMP.medicinalProductName.scientificNamePart</skos:altLabel>
		<skos:definition>The scientific or common (i.e. generic) name of the medicinal product without any other descriptors shall be specified. EXAMPLE For the medicinal product name ‘Irbesartan/Hydrochlorothiazide Pharma KK’ the common (generic) name element is ‘Irbesartan/Hydrochlorothiazide’.</skos:definition>
		<skos:prefLabel>Scientific name part</skos:prefLabel>
		<idmp:isUMLAttributeOf rdf:resource="&idmp;medicinalProductName"/>
	</owl:NamedIndividual>
	
	<owl:NamedIndividual rdf:about="&idmp;medicinalProductName.strengthNamePart">
		<rdf:type rdf:resource="&skos;Concept"/>
		<rdf:type rdf:resource="&upper;DataAttribute"/>
		<rdf:type rdf:resource="&upper;LogicalDataEntity"/>
		<skos:altLabel>IDMP.medicinalProductName.strengthNamePart</skos:altLabel>
		<skos:definition>The strength, if reflected in the medicinal product name, shall be specified. This strength name part may differ from the concept of ‘Strength’ as described in section 5.13.5. The use of decimal points shall be accommodated, if required. EXAMPLE For the medicinal product name ‘Drug K Forte (Paracetamol 500mg, dihydrocodeine tartrate 30mg)’, the strength name part is ‘Forte’.</skos:definition>
		<skos:prefLabel>Strength name part</skos:prefLabel>
		<idmp:isUMLAttributeOf rdf:resource="&idmp;medicinalProductName"/>
	</owl:NamedIndividual>
	
	<owl:NamedIndividual rdf:about="&idmp;medicinalProductName.trademarkOrCompanyPart">
		<rdf:type rdf:resource="&skos;Concept"/>
		<rdf:type rdf:resource="&upper;DataAttribute"/>
		<rdf:type rdf:resource="&upper;LogicalDataEntity"/>
		<skos:altLabel>IDMP.medicinalProductName.trademarkOrCompanyPart</skos:altLabel>
		<skos:definition>The trademark, if present in the medicinal product name, shall be provided.</skos:definition>
		<skos:prefLabel>Trademark or company part</skos:prefLabel>
		<idmp:isUMLAttributeOf rdf:resource="&idmp;medicinalProductName"/>
	</owl:NamedIndividual>
	
	<owl:NamedIndividual rdf:about="&idmp;medicinalProductName.year">
		<rdf:type rdf:resource="&skos;Concept"/>
		<rdf:type rdf:resource="&upper;DataAttribute"/>
		<rdf:type rdf:resource="&upper;LogicalDataEntity"/>
		<skos:altLabel>IDMP.medicinalProductName.year</skos:altLabel>
		<skos:definition>The time/period, if present in the medicinal product name, shall be provided.EXAMPLE For an influenza vaccine with the medicinal product name ‘Drug-FLU season 2008/2009’, the time/period is ‘2008/2009’.</skos:definition>
		<skos:prefLabel>Year</skos:prefLabel>
		<idmp:isUMLAttributeOf rdf:resource="&idmp;medicinalProductName"/>
	</owl:NamedIndividual>
	
	<owl:NamedIndividual rdf:about="&idmp;medicinalProductPackageBatchIdentifier">
		<rdf:type rdf:resource="&owl;Class"/>
		<rdf:type rdf:resource="&skos;Concept"/>
		<rdf:type rdf:resource="&upper;DataObject"/>
		<rdf:type rdf:resource="&upper;LogicalDataEntity"/>
		<rdfs:subClassOf rdf:resource="&skos;Concept"/>
		<skos:altLabel>IDMP.medicinalProductPackageBatchIdentifier</skos:altLabel>
		<skos:definition>Carries the batch number and the expiration date when created a medicinal product package level.</skos:definition>
		<skos:prefLabel>Medicinal product package batch identifier</skos:prefLabel>
		<skos:related rdf:resource="&idmp;PCIDAttributeSet"/>
		<idmp:hasUMLAttribute rdf:resource="&idmp;medicinalProductPackageBatchIdentifier.BAID2"/>
		<idmp:hasUMLAttribute rdf:resource="&idmp;medicinalProductPackageBatchIdentifier.batchIdentifier"/>
		<idmp:hasUMLAttribute rdf:resource="&idmp;medicinalProductPackageBatchIdentifier.expirationDate"/>
	</owl:NamedIndividual>
	
	<owl:NamedIndividual rdf:about="&idmp;medicinalProductPackageBatchIdentifier.BAID2">
		<rdf:type rdf:resource="&skos;Concept"/>
		<rdf:type rdf:resource="&upper;DataAttribute"/>
		<rdf:type rdf:resource="&upper;LogicalDataEntity"/>
		<skos:altLabel>IDMP.medicinalProductPackageBatchIdentifier.BAID2</skos:altLabel>
		<skos:definition>Unique identifier allocated to a specific batch of an investigational medicinal product package supplementary to any existing identifier as ascribed by a medicines regulatory authority in a jurisdiction and a batch number as assigned by a manufacturer. This is for indexing purposes and to contribute to improving patient safety by allowing for the uniqueidentification of medicinal products worldwide.</skos:definition>
		<skos:prefLabel>Baid2</skos:prefLabel>
		<idmp:isUMLAttributeOf rdf:resource="&idmp;medicinalProductPackageBatchIdentifier"/>
	</owl:NamedIndividual>
	
	<owl:NamedIndividual rdf:about="&idmp;medicinalProductPackageBatchIdentifier.batchIdentifier">
		<rdf:type rdf:resource="&skos;Concept"/>
		<rdf:type rdf:resource="&upper;DataAttribute"/>
		<rdf:type rdf:resource="&upper;LogicalDataEntity"/>
		<skos:altLabel>IDMP.medicinalProductPackageBatchIdentifier.batchIdentifier</skos:altLabel>
		<skos:definition>Batch identifier of the medicinal product package</skos:definition>
		<skos:prefLabel>Batch id</skos:prefLabel>
		<idmp:isUMLAttributeOf rdf:resource="&idmp;medicinalProductPackageBatchIdentifier"/>
	</owl:NamedIndividual>
	
	<owl:NamedIndividual rdf:about="&idmp;medicinalProductPackageBatchIdentifier.expirationDate">
		<rdf:type rdf:resource="&skos;Concept"/>
		<rdf:type rdf:resource="&upper;DataAttribute"/>
		<rdf:type rdf:resource="&upper;LogicalDataEntity"/>
		<skos:altLabel>IDMP.medicinalProductPackageBatchIdentifier.expirationDate</skos:altLabel>
		<skos:definition>Optional attribute that specifies the expiration date of the product package batch</skos:definition>
		<skos:prefLabel>Medicinal product package batch identifier expiration date</skos:prefLabel>
		<idmp:isUMLAttributeOf rdf:resource="&idmp;medicinalProductPackageBatchIdentifier"/>
	</owl:NamedIndividual>
	
	<owl:NamedIndividual rdf:about="&idmp;organisation.address">
		<rdf:type rdf:resource="&skos;Concept"/>
		<rdf:type rdf:resource="&upper;DataAttribute"/>
		<rdf:type rdf:resource="&upper;LogicalDataEntity"/>
		<skos:altLabel>IDMP.organisation.address</skos:altLabel>
		<skos:definition>The address of the organisation using AD ISO Data Type shall be provided.</skos:definition>
		<skos:prefLabel>Organisation address</skos:prefLabel>
		<idmp:isUMLAttributeOf rdf:resource="&idmp;Organisation"/>
	</owl:NamedIndividual>
	
	<owl:NamedIndividual rdf:about="&idmp;organisation.identifier">
		<rdf:type rdf:resource="&skos;Concept"/>
		<rdf:type rdf:resource="&upper;DataAttribute"/>
		<rdf:type rdf:resource="&upper;LogicalDataEntity"/>
		<skos:altLabel>IDMP.organisation.identifier</skos:altLabel>
		<skos:definition>The unique identifier of the organisation shall be provided. An international coding system for unique organisation identifiers shall be used.</skos:definition>
		<skos:prefLabel>Organisation identifier</skos:prefLabel>
		<idmp:isUMLAttributeOf rdf:resource="&idmp;Organisation"/>
	</owl:NamedIndividual>
	
	<owl:NamedIndividual rdf:about="&idmp;organisation.name">
		<rdf:type rdf:resource="&skos;Concept"/>
		<rdf:type rdf:resource="&upper;DataAttribute"/>
		<rdf:type rdf:resource="&upper;LogicalDataEntity"/>
		<skos:altLabel>IDMP.organisation.name</skos:altLabel>
		<skos:definition>Name of the legal entity or organization</skos:definition>
		<skos:prefLabel>Organisation name</skos:prefLabel>
		<idmp:isUMLAttributeOf rdf:resource="&idmp;Organisation"/>
	</owl:NamedIndividual>
	
	<owl:NamedIndividual rdf:about="&idmp;otherCharacteristics">
		<rdf:type rdf:resource="&owl;Class"/>
		<rdf:type rdf:resource="&skos;Concept"/>
		<rdf:type rdf:resource="&upper;DataObject"/>
		<rdf:type rdf:resource="&upper;LogicalDataEntity"/>
		<rdfs:subClassOf rdf:resource="&skos;Concept"/>
		<dct:source>Source ISO IDMP 11615:2017</dct:source>
		<skos:altLabel>IDMP.Other Characteristics</skos:altLabel>
		<skos:altLabel>IDMP.Physical Characteristics</skos:altLabel>
		<skos:definition>The description of the height, weight, width, depth, volume, colour, shape, etc., of an itemWhere applicable for a package item (container), package (component), manufactured item or device, its physical characteristics can be specified. One or more images can be provided as applicable.A package item (and most particularly the outermost packaging) or a package component, as well as a device and a manufactured item, can have their physical characteristics described, including an image of the item as required.In addition, the packaged item (container), the device and the manufactured item may have a set of other characteristics associated with them.</skos:definition>
		<skos:prefLabel>Other characteristics</skos:prefLabel>
		<skos:prefLabel>Physical characteristics</skos:prefLabel>
		<skos:related rdf:resource="&idmp;PCIDAttributeSet"/>
		<skos:related rdf:resource="&idmp;medicalDevice"/>
		<idmp:hasUMLAttribute rdf:resource="&idmp;otherCharacteristics.code"/>
		<idmp:hasUMLAttribute rdf:resource="&idmp;otherCharacteristics.value"/>
		<idmp:hasUMLAttribute rdf:resource="&idmp;physicalCharacteristics.colour"/>
		<idmp:hasUMLAttribute rdf:resource="&idmp;physicalCharacteristics.depth"/>
		<idmp:hasUMLAttribute rdf:resource="&idmp;physicalCharacteristics.height"/>
		<idmp:hasUMLAttribute rdf:resource="&idmp;physicalCharacteristics.image"/>
		<idmp:hasUMLAttribute rdf:resource="&idmp;physicalCharacteristics.imprint"/>
		<idmp:hasUMLAttribute rdf:resource="&idmp;physicalCharacteristics.shape"/>
		<idmp:hasUMLAttribute rdf:resource="&idmp;physicalCharacteristics.volume"/>
		<idmp:hasUMLAttribute rdf:resource="&idmp;physicalCharacteristics.weight"/>
		<idmp:hasUMLAttribute rdf:resource="&idmp;physicalCharacteristics.width"/>
	</owl:NamedIndividual>
	
	<owl:NamedIndividual rdf:about="&idmp;otherCharacteristics.code">
		<rdf:type rdf:resource="&skos;Concept"/>
		<rdf:type rdf:resource="&upper;DataAttribute"/>
		<rdf:type rdf:resource="&upper;LogicalDataEntity"/>
		<skos:altLabel>IDMP.otherCharacteristics.code</skos:altLabel>
		<skos:definition>Zero or more other observations shall be made about the characteristics of the ‘Packaged Medicinal Product’, where applicable. They are represented by naming the characteristic in the ‘Code’ attribute using a CD data type, and then if required providing a ‘Value’ for the characteristic named using an ANY data type. This facility is useful for capturing unusual details not explicitly catered for in the other attributes.</skos:definition>
		<skos:prefLabel>Other characteristics code</skos:prefLabel>
		<idmp:isUMLAttributeOf rdf:resource="&idmp;otherCharacteristics"/>
	</owl:NamedIndividual>
	
	<owl:NamedIndividual rdf:about="&idmp;otherCharacteristics.value">
		<rdf:type rdf:resource="&skos;Concept"/>
		<rdf:type rdf:resource="&upper;DataAttribute"/>
		<rdf:type rdf:resource="&upper;LogicalDataEntity"/>
		<skos:altLabel>IDMP.otherCharacteristics.value</skos:altLabel>
		<skos:definition>Zero or more other observations shall be made about the characteristics of the ‘Packaged Medicinal Product’, where applicable. They are represented by naming the characteristic in the ‘Code’ attribute using a CD data type, and then if required providing a ‘Value’ for the characteristic named using an ANY data type. This facility is useful for capturing unusual details not explicitly catered for in the other attributes.</skos:definition>
		<skos:prefLabel>Other characteristics value</skos:prefLabel>
		<idmp:isUMLAttributeOf rdf:resource="&idmp;otherCharacteristics"/>
	</owl:NamedIndividual>
	
	<owl:NamedIndividual rdf:about="&idmp;outerPackaging">
		<rdf:type rdf:resource="&owl;Class"/>
		<rdf:type rdf:resource="&skos;Concept"/>
		<rdf:type rdf:resource="&upper;DataObject"/>
		<rdf:type rdf:resource="&upper;LogicalDataEntity"/>
		<rdfs:subClassOf rdf:resource="&skos;Concept"/>
		<skos:altLabel>IDMP.outerPackaging</skos:altLabel>
		<skos:definition>External container in which a medicinal product is supplied. The manufactured item or pharmaceutical product is not in direct contact with the outer packaging except where the outer packaging also serves as the immediate container. An alternative, compatible definition of outer packaging is given in Directive 92/27/EEC.</skos:definition>
		<skos:example>Box, carton.</skos:example>
		<skos:prefLabel>Outer packaging</skos:prefLabel>
		<skos:related rdf:resource="&idmp;PCIDAttributeSet"/>
		<idmp:hasUMLAttribute rdf:resource="&idmp;outerPackaging.alternates"/>
		<idmp:hasUMLAttribute rdf:resource="&idmp;outerPackaging.material"/>
	</owl:NamedIndividual>
	
	<owl:NamedIndividual rdf:about="&idmp;outerPackaging.alternates">
		<rdf:type rdf:resource="&skos;Concept"/>
		<rdf:type rdf:resource="&upper;DataAttribute"/>
		<rdf:type rdf:resource="&upper;LogicalDataEntity"/>
		<skos:altLabel>IDMP.outerPackaging.alternates</skos:altLabel>
		<skos:definition>This is a pointer to further sets of ‘Materials’ that represent alternative parts of the packaging.</skos:definition>
		<skos:prefLabel>Outer packaging alternates</skos:prefLabel>
		<idmp:isUMLAttributeOf rdf:resource="&idmp;outerPackaging"/>
	</owl:NamedIndividual>
	
	<owl:NamedIndividual rdf:about="&idmp;outerPackaging.material">
		<rdf:type rdf:resource="&skos;Concept"/>
		<rdf:type rdf:resource="&upper;DataAttribute"/>
		<rdf:type rdf:resource="&upper;LogicalDataEntity"/>
		<skos:altLabel>IDMP.outerPackaging.material</skos:altLabel>
		<skos:definition>A value drawn from a value set specified in ISO/DIS 11238 shall be provided. It shall be specified using a code data type.</skos:definition>
		<skos:prefLabel>Outer packaging material</skos:prefLabel>
		<idmp:isUMLAttributeOf rdf:resource="&idmp;outerPackaging"/>
	</owl:NamedIndividual>
	
	<owl:NamedIndividual rdf:about="&idmp;packageItem">
		<rdf:type rdf:resource="&owl;Class"/>
		<rdf:type rdf:resource="&skos;Concept"/>
		<rdf:type rdf:resource="&upper;DataObject"/>
		<rdf:type rdf:resource="&upper;LogicalDataEntity"/>
		<rdfs:subClassOf rdf:resource="&skos;Concept"/>
		<skos:altLabel>IDMP.packageItem</skos:altLabel>
		<skos:definition>These are the distinct kinds of items that make up the package. There will only be more than one instance of this class if the Package Medicinal Product is a kit or includes an administration device.</skos:definition>
		<skos:prefLabel>Package item</skos:prefLabel>
		<skos:related rdf:resource="&idmp;IPCIDAttributeSet"/>
		<skos:related rdf:resource="&idmp;PCIDAttributeSet"/>
		<idmp:hasUMLAttribute rdf:resource="&idmp;packageItem.itemsInPackage"/>
		<idmp:hasUMLAttribute rdf:resource="&idmp;packageItem.packageType"/>
		<idmp:hasUMLAttribute rdf:resource="&idmp;packageItem.type"/>
	</owl:NamedIndividual>
	
	<owl:NamedIndividual rdf:about="&idmp;packageItem.itemsInPackage">
		<rdf:type rdf:resource="&skos;Concept"/>
		<rdf:type rdf:resource="&upper;DataAttribute"/>
		<rdf:type rdf:resource="&upper;LogicalDataEntity"/>
		<skos:altLabel>IDMP.packageItem.itemsInPackage</skos:altLabel>
		<skos:definition>The number (quantity) of identical items per package shall be described using an INT data type.</skos:definition>
		<skos:prefLabel>Items in package of package item</skos:prefLabel>
		<idmp:isUMLAttributeOf rdf:resource="&idmp;packageItem"/>
	</owl:NamedIndividual>
	
	<owl:NamedIndividual rdf:about="&idmp;packageItem.packageType">
		<rdf:type rdf:resource="&skos;Concept"/>
		<rdf:type rdf:resource="&upper;DataAttribute"/>
		<rdf:type rdf:resource="&upper;LogicalDataEntity"/>
		<skos:altLabel>IDMP.packageItem.packageType</skos:altLabel>
		<skos:definition>Package Type describes the physical type of the container of the medicine. This is a term and a term identifier specified in ISO/DIS 11239 and its resulting controlled vocabulary. It is to be specified using a code data type. EXAMPLE Pre-Filled Pen, Blister, Tube.</skos:definition>
		<skos:prefLabel>Package item package type</skos:prefLabel>
		<idmp:isUMLAttributeOf rdf:resource="&idmp;packageItem"/>
	</owl:NamedIndividual>
	
	<owl:NamedIndividual rdf:about="&idmp;packageItem.type">
		<rdf:type rdf:resource="&skos;Concept"/>
		<rdf:type rdf:resource="&upper;DataAttribute"/>
		<rdf:type rdf:resource="&upper;LogicalDataEntity"/>
		<skos:altLabel>IDMP.packageItem.type</skos:altLabel>
		<skos:definition>The value for the ‘Packaged Item Type’ shall be described using a CD data type and using a defined value set. EXAMPLE Container: for example, bottle amber PET with polypropylene child resistant closure fitted with expanded polythene liner. Pharmaceutical Item: for example, a pessary. (Administration) Device: for example, an applicator for a cream or a spoon with a 5 ml and 2.5 ml measure.</skos:definition>
		<skos:prefLabel>Package item type code</skos:prefLabel>
		<idmp:isUMLAttributeOf rdf:resource="&idmp;packageItem"/>
	</owl:NamedIndividual>
	
	<owl:NamedIndividual rdf:about="&idmp;packageItemPart">
		<rdf:type rdf:resource="&owl;Class"/>
		<rdf:type rdf:resource="&skos;Concept"/>
		<rdf:type rdf:resource="&upper;DataObject"/>
		<rdf:type rdf:resource="&upper;LogicalDataEntity"/>
		<rdfs:subClassOf rdf:resource="&skos;Concept"/>
		<skos:altLabel>IDMP.packageItemPart</skos:altLabel>
		<skos:definition>The ‘Package Item Part’ class shall describe the inner packaging, which is in direct contact with the medicine contained in the package. ‘Package Item’ shall include administration devices such as pre-filled injection pens. For devices where a unique device identifier is available, this shall be specified. Administration devices such as spoons or applicators should also be specified here.</skos:definition>
		<skos:prefLabel>Package item part</skos:prefLabel>
		<skos:related rdf:resource="&idmp;packageItem"/>
		<idmp:hasUMLAttribute rdf:resource="&idmp;packageItemPart.UDI"/>
		<idmp:hasUMLAttribute rdf:resource="&idmp;packageItemPart.alternate"/>
		<idmp:hasUMLAttribute rdf:resource="&idmp;packageItemPart.componentPart"/>
		<idmp:hasUMLAttribute rdf:resource="&idmp;packageItemPart.material"/>
	</owl:NamedIndividual>
	
	<owl:NamedIndividual rdf:about="&idmp;packageItemPart.UDI">
		<rdf:type rdf:resource="&skos;Concept"/>
		<rdf:type rdf:resource="&upper;DataAttribute"/>
		<rdf:type rdf:resource="&upper;LogicalDataEntity"/>
		<skos:altLabel>IDMP.packageItemPart.UDI</skos:altLabel>
		<skos:definition>Unique identifier assigned to a medicinal product</skos:definition>
		<skos:prefLabel>Package item part udi</skos:prefLabel>
		<idmp:isUMLAttributeOf rdf:resource="&idmp;packageItemPart"/>
	</owl:NamedIndividual>
	
	<owl:NamedIndividual rdf:about="&idmp;packageItemPart.alternate">
		<rdf:type rdf:resource="&skos;Concept"/>
		<rdf:type rdf:resource="&upper;DataAttribute"/>
		<rdf:type rdf:resource="&upper;LogicalDataEntity"/>
		<skos:altLabel>IDMP.packageItemPart.alternate</skos:altLabel>
		<skos:definition>This is a pointer to further sets of ‘Materials’ that represent alternative components of the packaging.</skos:definition>
		<skos:prefLabel>Alternate material component</skos:prefLabel>
		<idmp:isUMLAttributeOf rdf:resource="&idmp;packageItemPart"/>
	</owl:NamedIndividual>
	
	<owl:NamedIndividual rdf:about="&idmp;packageItemPart.componentPart">
		<rdf:type rdf:resource="&skos;Concept"/>
		<rdf:type rdf:resource="&upper;DataAttribute"/>
		<rdf:type rdf:resource="&upper;LogicalDataEntity"/>
		<skos:altLabel>IDMP.packageItemPart.componentPart</skos:altLabel>
		<skos:definition>This is a term and a term identifier as defined in ISO/DIS 11239 and its resulting controlled vocabulary. It is to be specified using a CD data type.EXAMPLE Pre-Filled Pen, Stopper.</skos:definition>
		<skos:prefLabel>Package item part component part</skos:prefLabel>
		<idmp:isUMLAttributeOf rdf:resource="&idmp;packageItemPart"/>
	</owl:NamedIndividual>
	
	<owl:NamedIndividual rdf:about="&idmp;packageItemPart.material">
		<rdf:type rdf:resource="&skos;Concept"/>
		<rdf:type rdf:resource="&upper;DataAttribute"/>
		<rdf:type rdf:resource="&upper;LogicalDataEntity"/>
		<skos:altLabel>IDMP.packageItemPart.material</skos:altLabel>
		<skos:definition>This is a term and a term identifier as defined in ISO/DIS 11238 and the resulting controlled vocabulary. It is to be specified using a CD data type.</skos:definition>
		<skos:prefLabel>Package item part material code</skos:prefLabel>
		<idmp:isUMLAttributeOf rdf:resource="&idmp;packageItemPart"/>
	</owl:NamedIndividual>
	
	<owl:NamedIndividual rdf:about="&idmp;pharmaceuticalProduct">
		<rdf:type rdf:resource="&owl;Class"/>
		<rdf:type rdf:resource="&skos;Concept"/>
		<rdf:type rdf:resource="&upper;DataObject"/>
		<rdf:type rdf:resource="&upper;LogicalDataEntity"/>
		<rdfs:subClassOf rdf:resource="&skos;Concept"/>
		<skos:altLabel>IDMP.pharmaceuticalProduct</skos:altLabel>
		<skos:definition>This is the medicine as reconstituted ready to be given to the patient</skos:definition>
		<skos:prefLabel>Pharmaceutical product</skos:prefLabel>
		<skos:related rdf:resource="&idmp;IPCIDAttributeSet"/>
		<skos:related rdf:resource="&idmp;PCIDAttributeSet"/>
		<skos:related rdf:resource="&idmp;packageItem"/>
		<idmp:hasUMLAttribute rdf:resource="&idmp;pharmaceuticalProduct.PhPID"/>
		<idmp:hasUMLAttribute rdf:resource="&idmp;pharmaceuticalProduct.administrableDoseForm"/>
		<idmp:hasUMLAttribute rdf:resource="&idmp;pharmaceuticalProduct.indication"/>
		<idmp:hasUMLAttribute rdf:resource="&idmp;pharmaceuticalProduct.ingredientSet"/>
		<idmp:hasUMLAttribute rdf:resource="&idmp;pharmaceuticalProduct.packSize"/>
		<idmp:hasUMLAttribute rdf:resource="&idmp;pharmaceuticalProduct.routeOfAdministration"/>
		<idmp:hasUMLAttribute rdf:resource="&idmp;pharmaceuticalProduct.unitOfPresentation"/>
	</owl:NamedIndividual>
	
	<owl:NamedIndividual rdf:about="&idmp;pharmaceuticalProduct.PhPID">
		<rdf:type rdf:resource="&skos;Concept"/>
		<rdf:type rdf:resource="&upper;DataAttribute"/>
		<rdf:type rdf:resource="&upper;LogicalDataEntity"/>
		<skos:altLabel>IDMP.pharmaceuticalProduct.PhPID</skos:altLabel>
		<skos:definition>Globally unique identifier assigned to the pharmaceutical product(s)</skos:definition>
		<skos:prefLabel>Phpid</skos:prefLabel>
		<idmp:isUMLAttributeOf rdf:resource="&idmp;pharmaceuticalProduct"/>
	</owl:NamedIndividual>
	
	<owl:NamedIndividual rdf:about="&idmp;pharmaceuticalProduct.administrableDoseForm">
		<rdf:type rdf:resource="&skos;Concept"/>
		<rdf:type rdf:resource="&upper;DataAttribute"/>
		<rdf:type rdf:resource="&upper;LogicalDataEntity"/>
		<skos:altLabel>IDMP.pharmaceuticalProduct.administrableDoseForm</skos:altLabel>
		<skos:definition>This shall describe the pharmaceutical dose form as to be administered to the patient in accordance with the terms laid down in the marketing authorization. It is after it has undergone any necessary reconstitution. Aterm and a term identifier as defined by ISO/DIS 11239 and its resulting controlled vocabulary shall be used. It is to be specified using a CD data type. EXAMPLE Values are: Tablet, Capsule, Oral Solution, Suspension.NOTE A medicinal product may have two manufactured items, one with a ‘Manufactured Dose Form’ of ‘powder forsolution for injection’ and the other with a ‘Manufactured Dose Form’ of ‘solvent for solution for injection’. These are thenreconstituted to an ‘Administrable Dose Form’ ‘solution for injection’ before administered to a patient.</skos:definition>
		<skos:prefLabel>Administrable dose form</skos:prefLabel>
		<idmp:isUMLAttributeOf rdf:resource="&idmp;pharmaceuticalProduct"/>
	</owl:NamedIndividual>
	
	<owl:NamedIndividual rdf:about="&idmp;pharmaceuticalProduct.indication">
		<rdf:type rdf:resource="&skos;Concept"/>
		<rdf:type rdf:resource="&upper;DataAttribute"/>
		<rdf:type rdf:resource="&upper;LogicalDataEntity"/>
		<skos:altLabel>IDMP.pharmaceuticalProduct.indication</skos:altLabel>
		<skos:definition>intended use of the medicinal product as authorized by the medicines regulatory authority in a jurisdiction NOTE For clinical trials, this refers to the intended use under investigation and as described in the clinical trial protocol.</skos:definition>
		<skos:prefLabel>Pharmaceutical product Indication</skos:prefLabel>
		<idmp:isUMLAttributeOf rdf:resource="&idmp;pharmaceuticalProduct"/>
	</owl:NamedIndividual>
	
	<owl:NamedIndividual rdf:about="&idmp;pharmaceuticalProduct.ingredientSet">
		<rdf:type rdf:resource="&skos;Concept"/>
		<rdf:type rdf:resource="&upper;DataAttribute"/>
		<rdf:type rdf:resource="&upper;LogicalDataEntity"/>
		<skos:altLabel>IDMP.pharmaceuticalProduct.ingredientSet</skos:altLabel>
		<skos:definition>Reference attribute from Ingredient class</skos:definition>
		<skos:prefLabel>Pharmaceutical product ingredient set</skos:prefLabel>
		<idmp:isUMLAttributeOf rdf:resource="&idmp;pharmaceuticalProduct"/>
	</owl:NamedIndividual>
	
	<owl:NamedIndividual rdf:about="&idmp;pharmaceuticalProduct.packSize">
		<rdf:type rdf:resource="&skos;Concept"/>
		<rdf:type rdf:resource="&upper;DataAttribute"/>
		<rdf:type rdf:resource="&upper;LogicalDataEntity"/>
		<skos:altLabel>IDMP.pharmaceuticalProduct.packSize</skos:altLabel>
		<skos:definition>This is the ‘Pack Size’ of the ‘Pharmaceutical Product’. It shall be specified using a PQ data type and the unit symbol and unit identifier as defined by ISO/DIS 11240 and its resulting controlled vocabulary. For many pharmaceutical dose forms with single ingredients, the value and units in ‘Pack Size’ will be a simple multiple of the value and units for the ‘Strength’ of the single ingredient. However, where there are multiple ingredients, or where the strength is expressed as a quantity per volume rather than a quantity per item, the values and units will be different.</skos:definition>
		<skos:prefLabel>Pharmaceutical product pack size</skos:prefLabel>
		<idmp:isUMLAttributeOf rdf:resource="&idmp;pharmaceuticalProduct"/>
	</owl:NamedIndividual>
	
	<owl:NamedIndividual rdf:about="&idmp;pharmaceuticalProduct.routeOfAdministration">
		<rdf:type rdf:resource="&skos;Concept"/>
		<rdf:type rdf:resource="&upper;DataAttribute"/>
		<rdf:type rdf:resource="&upper;LogicalDataEntity"/>
		<skos:altLabel>IDMP.pharmaceuticalProduct.routeOfAdministration</skos:altLabel>
		<skos:definition>The route(s) of administration as authorized in accordance with the terms outlined in the marketing authorizationshall be specified. ‘Route of Administration’ shall use the terms and term identifiers as defined in ISO/DIS 11239 and its resulting controlled vocabulary. A CD data type shall be used.</skos:definition>
		<skos:prefLabel>Route of administration</skos:prefLabel>
		<idmp:isUMLAttributeOf rdf:resource="&idmp;pharmaceuticalProduct"/>
	</owl:NamedIndividual>
	
	<owl:NamedIndividual rdf:about="&idmp;pharmaceuticalProduct.unitOfPresentation">
		<rdf:type rdf:resource="&skos;Concept"/>
		<rdf:type rdf:resource="&upper;DataAttribute"/>
		<rdf:type rdf:resource="&upper;LogicalDataEntity"/>
		<skos:altLabel>IDMP.pharmaceuticalProduct.unitOfPresentation</skos:altLabel>
		<skos:definition>This specifies the “real world” units in which the ‘Pack Size’ of the ‘Pharmaceutical Product’ is described. specified term and a term identifier as defined by ISO/DIS 11239 and its resulting controlled vocabulary shall be used. It is to be specified using a code data type. For items where their ‘Pack Size’ is a measured quantity of weight or volume the ‘Unit of Presentation’ shall not be given since it is the same as the units of ‘Pack Size’ (that is ml, mg or some multiple). For solid dose forms and other items that are measured by counting integer quantities the unit for ‘Pack Size’ shall be “Unit” and the ‘Presentation Unit’ shall be the item that is counted (e.g. Tablets, Capsules).</skos:definition>
		<skos:prefLabel>Pharmaceutical product unit of presentation</skos:prefLabel>
		<idmp:isUMLAttributeOf rdf:resource="&idmp;pharmaceuticalProduct"/>
	</owl:NamedIndividual>
	
	<owl:NamedIndividual rdf:about="&idmp;physicalCharacteristics.colour">
		<rdf:type rdf:resource="&skos;Concept"/>
		<rdf:type rdf:resource="&upper;DataAttribute"/>
		<rdf:type rdf:resource="&upper;LogicalDataEntity"/>
		<skos:altLabel>IDMP.physicalCharacteristics.colour</skos:altLabel>
		<skos:definition>The ‘Colour’ shall be described using a controlled vocabulary. The term and the term identifier shall be used. They are to be specified using code data types.</skos:definition>
		<skos:prefLabel>Colour</skos:prefLabel>
		<idmp:isUMLAttributeOf rdf:resource="&idmp;physicalCharacteristics"/>
	</owl:NamedIndividual>
	
	<owl:NamedIndividual rdf:about="&idmp;physicalCharacteristics.depth">
		<rdf:type rdf:resource="&skos;Concept"/>
		<rdf:type rdf:resource="&upper;DataAttribute"/>
		<rdf:type rdf:resource="&upper;LogicalDataEntity"/>
		<skos:altLabel>IDMP.physicalCharacteristics.depth</skos:altLabel>
		<skos:definition>The values for ‘Depth’ shall be described using the value set as specified in ISO/DIS 11240. The symbol and the symbol identifier shall be used. They are to be specified using a PQ data type.</skos:definition>
		<skos:prefLabel>Depth</skos:prefLabel>
		<idmp:isUMLAttributeOf rdf:resource="&idmp;physicalCharacteristics"/>
	</owl:NamedIndividual>
	
	<owl:NamedIndividual rdf:about="&idmp;physicalCharacteristics.height">
		<rdf:type rdf:resource="&skos;Concept"/>
		<rdf:type rdf:resource="&upper;DataAttribute"/>
		<rdf:type rdf:resource="&upper;LogicalDataEntity"/>
		<skos:altLabel>IDMP.physicalCharacteristics.height</skos:altLabel>
		<skos:definition>The values for ‘Height’ shall be described using the value set as specified in ISO/DIS 11240. The symbol and the symbol identifier shall be used. They are to be specified using a PQ data type.</skos:definition>
		<skos:prefLabel>Height</skos:prefLabel>
		<idmp:isUMLAttributeOf rdf:resource="&idmp;physicalCharacteristics"/>
	</owl:NamedIndividual>
	
	<owl:NamedIndividual rdf:about="&idmp;physicalCharacteristics.image">
		<rdf:type rdf:resource="&skos;Concept"/>
		<rdf:type rdf:resource="&upper;DataAttribute"/>
		<rdf:type rdf:resource="&upper;LogicalDataEntity"/>
		<skos:altLabel>IDMP.physicalCharacteristics.image</skos:altLabel>
		<skos:definition>One or more ‘Images’ and/or ‘Imprints’ of the packaged item shall be included as applicable. The format of the image shall follow ISO 12639:2004 and shall be held in an ED data type.</skos:definition>
		<skos:prefLabel>Image</skos:prefLabel>
		<idmp:isUMLAttributeOf rdf:resource="&idmp;physicalCharacteristics"/>
	</owl:NamedIndividual>
	
	<owl:NamedIndividual rdf:about="&idmp;physicalCharacteristics.imprint">
		<rdf:type rdf:resource="&skos;Concept"/>
		<rdf:type rdf:resource="&upper;DataAttribute"/>
		<rdf:type rdf:resource="&upper;LogicalDataEntity"/>
		<skos:altLabel>IDMP.physicalCharacteristics.imprint</skos:altLabel>
		<skos:definition>One or more ‘Images’ and/or ‘Imprints’ of the packaged item shall be included as applicable. The format of the image shall follow ISO 12639:2004 and shall be held in an ED data type.</skos:definition>
		<skos:prefLabel>Imprint</skos:prefLabel>
		<idmp:isUMLAttributeOf rdf:resource="&idmp;physicalCharacteristics"/>
	</owl:NamedIndividual>
	
	<owl:NamedIndividual rdf:about="&idmp;physicalCharacteristics.shape">
		<rdf:type rdf:resource="&skos;Concept"/>
		<rdf:type rdf:resource="&upper;DataAttribute"/>
		<rdf:type rdf:resource="&upper;LogicalDataEntity"/>
		<skos:altLabel>IDMP.physicalCharacteristics.shape</skos:altLabel>
		<skos:definition>Shape shall be described using a controlled vocabulary. The term and the term identifier shall be used. They are to be specified using code data types.</skos:definition>
		<skos:prefLabel>Shape</skos:prefLabel>
		<idmp:isUMLAttributeOf rdf:resource="&idmp;physicalCharacteristics"/>
	</owl:NamedIndividual>
	
	<owl:NamedIndividual rdf:about="&idmp;physicalCharacteristics.volume">
		<rdf:type rdf:resource="&skos;Concept"/>
		<rdf:type rdf:resource="&upper;DataAttribute"/>
		<rdf:type rdf:resource="&upper;LogicalDataEntity"/>
		<skos:altLabel>IDMP.physicalCharacteristics.volume</skos:altLabel>
		<skos:definition>The values for ‘Volume’ shall be described using the value set as specified in ISO/DIS 11240. The symbol and the symbol identifier shall be used. They are to be specified using a PQ data type.</skos:definition>
		<skos:prefLabel>Volume</skos:prefLabel>
		<idmp:isUMLAttributeOf rdf:resource="&idmp;physicalCharacteristics"/>
	</owl:NamedIndividual>
	
	<owl:NamedIndividual rdf:about="&idmp;physicalCharacteristics.weight">
		<rdf:type rdf:resource="&skos;Concept"/>
		<rdf:type rdf:resource="&upper;DataAttribute"/>
		<rdf:type rdf:resource="&upper;LogicalDataEntity"/>
		<skos:altLabel>IDMP.physicalCharacteristics.weight</skos:altLabel>
		<skos:definition>The values for ‘Weight’ shall be described using the value set as specified in ISO/DIS 11240. The symbol and the symbol identifier shall be used. They are to be specified using a PQ data type.</skos:definition>
		<skos:prefLabel>Weight</skos:prefLabel>
		<idmp:isUMLAttributeOf rdf:resource="&idmp;physicalCharacteristics"/>
	</owl:NamedIndividual>
	
	<owl:NamedIndividual rdf:about="&idmp;physicalCharacteristics.width">
		<rdf:type rdf:resource="&skos;Concept"/>
		<rdf:type rdf:resource="&upper;DataAttribute"/>
		<rdf:type rdf:resource="&upper;LogicalDataEntity"/>
		<skos:altLabel>IDMP.physicalCharacteristics.width</skos:altLabel>
		<skos:definition>The values for ‘Weight’ shall be described using the value set as specified in ISO/DIS 11240. The symbol and the symbol identifier shall be used. They are to be specified using a PQ data type.</skos:definition>
		<skos:prefLabel>Width</skos:prefLabel>
		<idmp:isUMLAttributeOf rdf:resource="&idmp;physicalCharacteristics"/>
	</owl:NamedIndividual>
	
	<owl:NamedIndividual rdf:about="&idmp;referenceStrength">
		<rdf:type rdf:resource="&owl;Class"/>
		<rdf:type rdf:resource="&skos;Concept"/>
		<rdf:type rdf:resource="&upper;DataObject"/>
		<rdf:type rdf:resource="&upper;LogicalDataEntity"/>
		<rdfs:subClassOf rdf:resource="&skos;Concept"/>
		<skos:altLabel>IDMP.referenceStrength</skos:altLabel>
		<skos:definition>The strength of the ‘Reference Substance’ shall be specified as a quantity of the substance as referred to in order to express a given quantity of the ‘Manufactured Item’ or ‘Pharmaceutical Product’. The symbol and the symbol identifier as defined in ISO/DIS 11240 and its resulting controlled vocabulary shall be specified. Where the strength is defined on the basis of a ‘Unit of Presentation’, the term and term identifier shall be used as defined in ISO/DIS 11239 and its resulting controlled vocabulary.</skos:definition>
		<skos:prefLabel>Reference strength</skos:prefLabel>
		<skos:related rdf:resource="&idmp;specifiedSubstance"/>
		<skos:related rdf:resource="&idmp;substance"/>
		<idmp:hasUMLAttribute rdf:resource="&idmp;referenceStrength.referenceSpecifiedSubstance"/>
		<idmp:hasUMLAttribute rdf:resource="&idmp;referenceStrength.referenceSpecifiedSubstanceStrength"/>
		<idmp:hasUMLAttribute rdf:resource="&idmp;referenceStrength.referenceSubstance"/>
		<idmp:hasUMLAttribute rdf:resource="&idmp;referenceStrength.referenceSubstanceStrength"/>
	</owl:NamedIndividual>
	
	<owl:NamedIndividual rdf:about="&idmp;referenceStrength.referenceSpecifiedSubstance">
		<rdf:type rdf:resource="&skos;Concept"/>
		<rdf:type rdf:resource="&upper;DataAttribute"/>
		<rdf:type rdf:resource="&upper;LogicalDataEntity"/>
		<skos:altLabel>IDMP.referenceStrength.referenceSpecifiedSubstance</skos:altLabel>
		<skos:definition>The value for the ‘Reference Specified Substance’ shall be described using a term and a term identifier as defined in ISO/DIS 11238 and its resulting controlled vocabulary. It shall be specified using a code data type.</skos:definition>
		<skos:prefLabel>Reference specified substance</skos:prefLabel>
		<idmp:isUMLAttributeOf rdf:resource="&idmp;referenceStrength"/>
	</owl:NamedIndividual>
	
	<owl:NamedIndividual rdf:about="&idmp;referenceStrength.referenceSpecifiedSubstanceStrength">
		<rdf:type rdf:resource="&skos;Concept"/>
		<rdf:type rdf:resource="&upper;DataAttribute"/>
		<rdf:type rdf:resource="&upper;LogicalDataEntity"/>
		<skos:altLabel>IDMP.referenceStrength.referenceSpecifiedSubstanceStrength</skos:altLabel>
		<skos:definition>The strength of the ‘Reference Specified Substance’ shall be specified as a quantity of the specified substance as referred to in order to express a given quantity of the ‘Manufactured Item’ or ‘Pharmaceutical Product’. The symbol and the symbol identifier as defined in ISO/DIS 11240 and its resulting controlled vocabulary shall be specified. Where the strength is defined on the basis of a ‘Unit of Presentation’, the term and term identifier shall be used as defined in ISO/DIS 11239 and its resulting controlled vocabulary.</skos:definition>
		<skos:prefLabel>Reference specified substance strength</skos:prefLabel>
		<idmp:isUMLAttributeOf rdf:resource="&idmp;referenceStrength"/>
	</owl:NamedIndividual>
	
	<owl:NamedIndividual rdf:about="&idmp;referenceStrength.referenceSubstance">
		<rdf:type rdf:resource="&skos;Concept"/>
		<rdf:type rdf:resource="&upper;DataAttribute"/>
		<rdf:type rdf:resource="&upper;LogicalDataEntity"/>
		<skos:altLabel>IDMP.referenceStrength.referenceSubstance</skos:altLabel>
		<skos:definition>The value for the ‘Reference Substance’ shall be described using a term and a term identifier as defined in ISO/DIS 11238 and its resulting controlled vocabulary. It shall be specified using a code data type.</skos:definition>
		<skos:prefLabel>Reference substance</skos:prefLabel>
		<idmp:isUMLAttributeOf rdf:resource="&idmp;referenceStrength"/>
	</owl:NamedIndividual>
	
	<owl:NamedIndividual rdf:about="&idmp;referenceStrength.referenceSubstanceStrength">
		<rdf:type rdf:resource="&skos;Concept"/>
		<rdf:type rdf:resource="&upper;DataAttribute"/>
		<rdf:type rdf:resource="&upper;LogicalDataEntity"/>
		<skos:altLabel>IDMP.referenceStrength.referenceSubstanceStrength</skos:altLabel>
		<skos:definition>The strength of the ‘Reference Substance’ shall be specified as a quantity of the substance as referred to in order to express a given quantity of the ‘Manufactured Item’ or ‘Pharmaceutical Product’. The symbol and the symbol identifier as defined in ISO/DIS 11240 and its resulting controlled vocabulary shall be specified. Where the strength is defined on the basis of a ‘Unit of Presentation’, the term and term identifier shall be used as defined in ISO/DIS 11239 and its resulting controlled vocabulary.</skos:definition>
		<skos:prefLabel>Reference substance strength</skos:prefLabel>
		<idmp:isUMLAttributeOf rdf:resource="&idmp;referenceStrength"/>
	</owl:NamedIndividual>
	
	<owl:NamedIndividual rdf:about="&idmp;routeOfAdministration">
		<rdf:type rdf:resource="&owl;Class"/>
		<rdf:type rdf:resource="&skos;Concept"/>
		<rdf:type rdf:resource="&upper;DataObject"/>
		<rdf:type rdf:resource="&upper;LogicalDataEntity"/>
		<rdfs:subClassOf rdf:resource="&skos;Concept"/>
		<skos:altLabel>IDMP.Route of Administration</skos:altLabel>
		<skos:definition>Source ISO IDMP 11615:2017Route of AdministrationThe route of administration is a concept that is used to describe the path by which the pharmaceutical product is taken into or makes contact with the body.The route of administration shall be specified using terms and a term identifier as defined in ISO 11239 and ISO/TS 20440 and its resulting terminology.</skos:definition>
		<skos:prefLabel>Route of administration</skos:prefLabel>
		<skos:related rdf:resource="&idmp;PhPIDSet"/>
		<idmp:hasUMLAttribute rdf:resource="&idmp;routeOfAdministration.maxDosePerRoute"/>
		<idmp:hasUMLAttribute rdf:resource="&idmp;routeOfAdministration.routeOfAdministration"/>
	</owl:NamedIndividual>
	
	<owl:NamedIndividual rdf:about="&idmp;routeOfAdministration.maxDosePerRoute">
		<rdf:type rdf:resource="&skos;Concept"/>
		<rdf:type rdf:resource="&upper;DataAttribute"/>
		<rdf:type rdf:resource="&upper;LogicalDataEntity"/>
		<skos:altLabel>IDMP.routeOfAdministration.maxDosePerRoute</skos:altLabel>
		<skos:definition>This shall specify the maximum single dose quantity that may be given for a first-in-human clinical trial in a single dose by the specified ‘Route of Administration’. This shall be specified using an RTO data type.</skos:definition>
		<skos:prefLabel>Max dose per route</skos:prefLabel>
		<idmp:isUMLAttributeOf rdf:resource="&idmp;routeOfAdministration"/>
	</owl:NamedIndividual>
	
	<owl:NamedIndividual rdf:about="&idmp;routeOfAdministration.routeOfAdministration">
		<rdf:type rdf:resource="&skos;Concept"/>
		<rdf:type rdf:resource="&upper;DataAttribute"/>
		<rdf:type rdf:resource="&upper;LogicalDataEntity"/>
		<skos:altLabel>IDMP.routeOfAdministration.routeOfAdministration</skos:altLabel>
		<skos:definition>‘Route of Administration’ shall use the terms and term identifiers as defined in ISO/DIS 11239 and its resulting controlled vocabulary. A CD data type shall be used.</skos:definition>
		<skos:prefLabel>Route Of administration</skos:prefLabel>
		<idmp:isUMLAttributeOf rdf:resource="&idmp;routeOfAdministration"/>
	</owl:NamedIndividual>
	
	<owl:NamedIndividual rdf:about="&idmp;specifiedSubstance">
		<rdf:type rdf:resource="&owl;Class"/>
		<rdf:type rdf:resource="&skos;Concept"/>
		<rdf:type rdf:resource="&upper;DataObject"/>
		<rdf:type rdf:resource="&upper;LogicalDataEntity"/>
		<rdfs:subClassOf rdf:resource="&skos;Concept"/>
		<skos:altLabel>IDMP.specifiedSubstance</skos:altLabel>
		<skos:definition>At the Substance level, substances are defined based on inherent attributes rather than use or method of manufacture. At the Specified Substance level, four separate groups of elements provide additional information. The four groups of Specified Substance elements allow for the explicit capture of information essential for the evaluation and tracking of material used in medicinal products. Each of the four groups of elements provides information essential for these regulatory needs in a manner that should facilitate compliance. The implementation of the Specified Substance Groups is conditional depending on the condition that one of the elements used to describe the Specified Substance is defining. Attributes specific to Specified Substance are: Constituent substances in a multi-substance material; Proportions of constituent substances in a multi-substance material; Physical state; Grade or purity of material;Manufacturing information; Analytical data, Specifications and Tests.</skos:definition>
		<skos:prefLabel>Specified substance</skos:prefLabel>
		<skos:related rdf:resource="&idmp;Ingredient"/>
		<skos:related rdf:resource="&idmp;PhPIDSpSubL1"/>
		<skos:related rdf:resource="&idmp;substance"/>
		<idmp:hasUMLAttribute rdf:resource="&idmp;specifiedSubstance.referenceStrength"/>
		<idmp:hasUMLAttribute rdf:resource="&idmp;specifiedSubstance.role"/>
		<idmp:hasUMLAttribute rdf:resource="&idmp;specifiedSubstance.specifiedSubstance"/>
		<idmp:hasUMLAttribute rdf:resource="&idmp;specifiedSubstance.specifiedSubstanceStrength"/>
	</owl:NamedIndividual>
	
	<owl:NamedIndividual rdf:about="&idmp;specifiedSubstance.referenceStrength">
		<rdf:type rdf:resource="&skos;Concept"/>
		<rdf:type rdf:resource="&upper;DataAttribute"/>
		<rdf:type rdf:resource="&upper;LogicalDataEntity"/>
		<skos:altLabel>IDMP.specifiedSubstance.referenceStrength</skos:altLabel>
		<skos:definition>The strength of the ‘Reference Specified Substance’ shall be specified as a quantity of the specified substance as referred to in order to express a given quantity of the ‘Manufactured Item’ or ‘Pharmaceutical Product’. The symbol and the symbol identifier as defined in ISO/DIS 11240 and its resulting controlled vocabulary shall be specified. Where the strength is defined on the basis of a ‘Unit of Presentation’, the term and term identifier shall be used as defined in ISO/DIS 11239 and its resulting controlled vocabulary. It shallbe specified using the ‘Strength’ class</skos:definition>
		<skos:prefLabel>Reference strength</skos:prefLabel>
		<idmp:isUMLAttributeOf rdf:resource="&idmp;specifiedSubstance"/>
	</owl:NamedIndividual>
	
	<owl:NamedIndividual rdf:about="&idmp;specifiedSubstance.role">
		<rdf:type rdf:resource="&skos;Concept"/>
		<rdf:type rdf:resource="&upper;DataAttribute"/>
		<rdf:type rdf:resource="&upper;LogicalDataEntity"/>
		<skos:altLabel>IDMP.specifiedSubstance.role</skos:altLabel>
		<skos:definition>The role of the ‘Specified Substance’ shall be described using a term and a term identifier of a controlled vocabulary. It shall be specified using a code data type.</skos:definition>
		<skos:prefLabel>Specified substance role</skos:prefLabel>
		<idmp:isUMLAttributeOf rdf:resource="&idmp;specifiedSubstance"/>
	</owl:NamedIndividual>
	
	<owl:NamedIndividual rdf:about="&idmp;specifiedSubstance.specifiedSubstance">
		<rdf:type rdf:resource="&skos;Concept"/>
		<rdf:type rdf:resource="&upper;DataAttribute"/>
		<rdf:type rdf:resource="&upper;LogicalDataEntity"/>
		<skos:altLabel>IDMP.specifiedSubstance.specifiedSubstance</skos:altLabel>
		<skos:definition>The attributes for the ‘Specified Substances’ class are the same as those described above for ‘Substances’ except that they refer to a specified substance as defined in ISO/DIS 11238.</skos:definition>
		<skos:prefLabel>Specified substance</skos:prefLabel>
		<idmp:isUMLAttributeOf rdf:resource="&idmp;specifiedSubstance"/>
	</owl:NamedIndividual>
	
	<owl:NamedIndividual rdf:about="&idmp;specifiedSubstance.specifiedSubstanceStrength">
		<rdf:type rdf:resource="&skos;Concept"/>
		<rdf:type rdf:resource="&upper;DataAttribute"/>
		<rdf:type rdf:resource="&upper;LogicalDataEntity"/>
		<skos:altLabel>IDMP.specifiedSubstance.specifiedSubstanceStrength</skos:altLabel>
		<skos:definition>The strength of the ‘Specified Substance’ shall be indicated as a quantity of the substance present in a given quantity of the ‘Manufactured Item’ or ‘Pharmaceutical Product’. The symbol and the symbol identifier as defined in ISO/DIS 11240 and its resulting controlled vocabulary shall be specified. Where the strength is defined on the basis of a ‘Unit of Presentation’, the term and term identifier shall be used as defined inISO/DIS 11239 and its resulting controlled vocabulary. This attribute is optional.</skos:definition>
		<skos:prefLabel>Specified substance strength</skos:prefLabel>
		<idmp:isUMLAttributeOf rdf:resource="&idmp;specifiedSubstance"/>
	</owl:NamedIndividual>
	
	<owl:NamedIndividual rdf:about="&idmp;specifiedSubstanceForm">
		<rdf:type rdf:resource="&owl;Class"/>
		<rdf:type rdf:resource="&skos;Concept"/>
		<rdf:type rdf:resource="&upper;DataObject"/>
		<rdf:type rdf:resource="&upper;LogicalDataEntity"/>
		<rdfs:subClassOf rdf:resource="&skos;Concept"/>
		<skos:altLabel>IDMP.specifiedSubstanceForm</skos:altLabel>
		<skos:definition>Pharmaceutical Product Specified Substance Form. Defined by special substance vocab, reference strength and administerable dose form</skos:definition>
		<skos:prefLabel>Specified substance form</skos:prefLabel>
		<skos:related rdf:resource="&idmp;PhPIDSpSubL3"/>
	</owl:NamedIndividual>
	
	<owl:NamedIndividual rdf:about="&idmp;specifiedSubstanceSet">
		<rdf:type rdf:resource="&owl;Class"/>
		<rdf:type rdf:resource="&skos;Concept"/>
		<rdf:type rdf:resource="&upper;DataObject"/>
		<rdf:type rdf:resource="&upper;LogicalDataEntity"/>
		<rdfs:subClassOf rdf:resource="&skos;Concept"/>
		<skos:altLabel>IDMP.specifiedSubstanceSet</skos:altLabel>
		<skos:definition>Pharmaceutical Product Specified Substance. Each pharmaceutical product shall have one or more active substances.</skos:definition>
		<skos:prefLabel>Specified substance set</skos:prefLabel>
		<skos:related rdf:resource="&idmp;PhPIDSpSub"/>
	</owl:NamedIndividual>
	
	<owl:NamedIndividual rdf:about="&idmp;specifiedSubstanceStrength">
		<rdf:type rdf:resource="&owl;Class"/>
		<rdf:type rdf:resource="&skos;Concept"/>
		<rdf:type rdf:resource="&upper;DataObject"/>
		<rdf:type rdf:resource="&upper;LogicalDataEntity"/>
		<rdfs:subClassOf rdf:resource="&skos;Concept"/>
		<skos:altLabel>IDMP.specifiedSubstanceStrength</skos:altLabel>
		<skos:definition>Pharmaceutical Product Specified Substance Strength. The strength of the Substance(s) or Specified Substance(s) shall be described as a quantity of the substance present in a given quantity of the Pharmaceutical Product.</skos:definition>
		<skos:prefLabel>Specified substance strength</skos:prefLabel>
		<skos:related rdf:resource="&idmp;PhPIDSpSubL2"/>
	</owl:NamedIndividual>
	
	<owl:NamedIndividual rdf:about="&idmp;sponsor.legalRepresentative">
		<rdf:type rdf:resource="&skos;Concept"/>
		<rdf:type rdf:resource="&upper;DataAttribute"/>
		<rdf:type rdf:resource="&upper;LogicalDataEntity"/>
		<skos:altLabel>IDMP.sponsor.legalRepresentative</skos:altLabel>
		<skos:definition>Legal representative of the sponsor</skos:definition>
		<skos:prefLabel>Legal representative</skos:prefLabel>
		<idmp:isUMLAttributeOf rdf:resource="&idmp;Sponsor"/>
	</owl:NamedIndividual>
	
	<owl:NamedIndividual rdf:about="&idmp;sponsor.organisation">
		<rdf:type rdf:resource="&skos;Concept"/>
		<rdf:type rdf:resource="&upper;DataAttribute"/>
		<rdf:type rdf:resource="&upper;LogicalDataEntity"/>
		<skos:altLabel>IDMP.sponsor.organisation</skos:altLabel>
		<skos:definition>Legal entity related to the sponsor</skos:definition>
		<skos:prefLabel>Sponsor organisation</skos:prefLabel>
		<idmp:isUMLAttributeOf rdf:resource="&idmp;Sponsor"/>
	</owl:NamedIndividual>
	
	<owl:NamedIndividual rdf:about="&idmp;sponsor.status">
		<rdf:type rdf:resource="&skos;Concept"/>
		<rdf:type rdf:resource="&upper;DataAttribute"/>
		<rdf:type rdf:resource="&upper;LogicalDataEntity"/>
		<skos:altLabel>IDMP.sponsor.status</skos:altLabel>
		<skos:definition>This shall specify the Sponsor to be either ‘Commercial’ or ‘Non-Commercial’. This is specified using an appropriate value set and a code data type.</skos:definition>
		<skos:prefLabel>Sponsor status</skos:prefLabel>
		<idmp:isUMLAttributeOf rdf:resource="&idmp;Sponsor"/>
	</owl:NamedIndividual>
	
	<owl:NamedIndividual rdf:about="&idmp;strength.country">
		<rdf:type rdf:resource="&skos;Concept"/>
		<rdf:type rdf:resource="&upper;DataAttribute"/>
		<rdf:type rdf:resource="&upper;LogicalDataEntity"/>
		<skos:altLabel>IDMP.strength.country</skos:altLabel>
		<skos:definition>The country or countries for which the Range and Measurement Point are valid may be specified. The values shall be specified using a code data type and using values from ISO 3166-1-alpha-2 code elements.</skos:definition>
		<skos:prefLabel>Strength country</skos:prefLabel>
		<idmp:isUMLAttributeOf rdf:resource="&idmp;Strength"/>
	</owl:NamedIndividual>
	
	<owl:NamedIndividual rdf:about="&idmp;strength.measurementPoint">
		<rdf:type rdf:resource="&skos;Concept"/>
		<rdf:type rdf:resource="&upper;DataAttribute"/>
		<rdf:type rdf:resource="&upper;LogicalDataEntity"/>
		<skos:altLabel>IDMP.strength.measurementPoint</skos:altLabel>
		<skos:definition>The point where a measurement is made shall be specified, as applicable. It shall be specified using a code data type.</skos:definition>
		<skos:prefLabel>Measurement point</skos:prefLabel>
		<idmp:isUMLAttributeOf rdf:resource="&idmp;Strength"/>
	</owl:NamedIndividual>
	
	<owl:NamedIndividual rdf:about="&idmp;strength.range">
		<rdf:type rdf:resource="&skos;Concept"/>
		<rdf:type rdf:resource="&upper;DataAttribute"/>
		<rdf:type rdf:resource="&upper;LogicalDataEntity"/>
		<skos:altLabel>IDMP.strength.range</skos:altLabel>
		<skos:definition>The actual value and units of the strength shall be specified using an RTO&lt;PQ,PQ&gt; data type, which requires data to be given as a numerator and a denominator, each with units, and for the numerator to be an interval. This allows both a low and a high value to be specified as well as upper and lower ranges. If both low and high values are the same, the interval is equivalent to a single value. If the low value is zero or not valued, the range is interpreted as not greater than the high value. Similarly if the high value is zero or not valued the range is interpreted as not less than the low value. The symbol and the symbol identifier as defined in ISO/DIS 11240 and its resulting controlled vocabulary shall be specified. Where the strength is defined on the basis of a ‘Unit of Presentation’, the term and term identifier shall be used as defined in ISO/DIS 11239 and its resulting controlled vocabulary.</skos:definition>
		<skos:prefLabel>Strength range</skos:prefLabel>
		<idmp:isUMLAttributeOf rdf:resource="&idmp;Strength"/>
	</owl:NamedIndividual>
	
	<owl:NamedIndividual rdf:about="&idmp;substance">
		<rdf:type rdf:resource="&owl;Class"/>
		<rdf:type rdf:resource="&skos;Concept"/>
		<rdf:type rdf:resource="&upper;DataObject"/>
		<rdf:type rdf:resource="&upper;LogicalDataEntity"/>
		<rdfs:subClassOf rdf:resource="&skos;Concept"/>
		<dct:source>Source ISO IDMP 11615:2017Substances</dct:source>
		<skos:altLabel>IDMP.substance</skos:altLabel>
		<skos:definition>Matter of defined composition that has discrete existence  whose origin may be biological  mineral or chemicalNote 1 to entry: A substance can be a moiety. A moiety is an entity within a substance that has a complete and continuous molecular structure. The strength of a pharmaceutical product  3.1.60  is often based on what is referred to as the active moiety of the molecule  responsible for the physiological or pharmacological action of the drug substance. Chemically  the active moiety of a stoichiometric or non-stoichoimetrical substance molecule is considered that part of the molecule that is the base  free acid or ion molecular part of a salt  solvate  chelate  clathrate  molecular complex or ester.</skos:definition>
		<skos:prefLabel>Substance</skos:prefLabel>
		<skos:related rdf:resource="&idmp;Ingredient"/>
		<skos:related rdf:resource="&idmp;Strength"/>
		<idmp:hasUMLAttribute rdf:resource="&idmp;substance.referenceStrength"/>
		<idmp:hasUMLAttribute rdf:resource="&idmp;substance.role"/>
		<idmp:hasUMLAttribute rdf:resource="&idmp;substance.substanceAttribute"/>
		<idmp:hasUMLAttribute rdf:resource="&idmp;substance.substanceStrength"/>
	</owl:NamedIndividual>
	
	<owl:NamedIndividual rdf:about="&idmp;substance.referenceStrength">
		<rdf:type rdf:resource="&skos;Concept"/>
		<rdf:type rdf:resource="&upper;DataAttribute"/>
		<rdf:type rdf:resource="&upper;LogicalDataEntity"/>
		<skos:altLabel>IDMP.substance.referenceStrength</skos:altLabel>
		<skos:definition>The strength of the ‘Reference Substance’ shall be specified as a quantity of the substance as referred to in order to express a given quantity of the ‘Manufactured Item’ or ‘Pharmaceutical Product’. The symbol and the symbol identifier as defined in ISO/DIS 11240 and its resulting controlled vocabulary shall be specified. Where the strength is defined on the basis of a ‘Unit of Presentation’, the term and term identifier shall be used asdefined in ISO/DIS 11239 and its resulting controlled vocabulary. It shall be specified using the ‘Strength’ class.</skos:definition>
		<skos:prefLabel>Reference strength</skos:prefLabel>
		<idmp:isUMLAttributeOf rdf:resource="&idmp;substance"/>
	</owl:NamedIndividual>
	
	<owl:NamedIndividual rdf:about="&idmp;substance.role">
		<rdf:type rdf:resource="&skos;Concept"/>
		<rdf:type rdf:resource="&upper;DataAttribute"/>
		<rdf:type rdf:resource="&upper;LogicalDataEntity"/>
		<skos:altLabel>IDMP.substance.role</skos:altLabel>
		<skos:definition>The role of the ‘Substance’ shall be described using a term and a term identifier of a controlled vocabulary. It shall be specified using a code data type.</skos:definition>
		<skos:prefLabel>Substance role</skos:prefLabel>
		<idmp:isUMLAttributeOf rdf:resource="&idmp;substance"/>
	</owl:NamedIndividual>
	
	<owl:NamedIndividual rdf:about="&idmp;substance.substanceAttribute">
		<rdf:type rdf:resource="&skos;Concept"/>
		<rdf:type rdf:resource="&upper;DataAttribute"/>
		<rdf:type rdf:resource="&upper;LogicalDataEntity"/>
		<skos:altLabel>IDMP.substance.substanceAttribute</skos:altLabel>
		<skos:definition>The ‘Substance’ shall be described using a term and a term identifier as defined in ISO/DIS 11238 and its resulting controlled vocabulary. It shall be specified using a code data type.</skos:definition>
		<skos:prefLabel>Substance attribute</skos:prefLabel>
		<idmp:isUMLAttributeOf rdf:resource="&idmp;substance"/>
	</owl:NamedIndividual>
	
	<owl:NamedIndividual rdf:about="&idmp;substance.substanceStrength">
		<rdf:type rdf:resource="&skos;Concept"/>
		<rdf:type rdf:resource="&upper;DataAttribute"/>
		<rdf:type rdf:resource="&upper;LogicalDataEntity"/>
		<skos:altLabel>IDMP.substance.substanceStrength</skos:altLabel>
		<skos:definition>The strength of the ‘Substance’ shall be specified as a quantity of the substance present in a given quantity of the ‘Manufactured Item’ or ‘Pharmaceutical Product’. It shall be specified using the Strength class see section 5.13.5. The symbol and the symbol identifier as defined in ISO/DIS 11240 and its resulting controlled vocabulary shall be specified. Where the strength is defined on the basis of a ‘Unit of Presentation’, the term and term identifier shall be used as defined in ISO/DIS 11239 and its resulting controlled vocabulary.</skos:definition>
		<skos:prefLabel>Substance strength</skos:prefLabel>
		<idmp:isUMLAttributeOf rdf:resource="&idmp;substance"/>
	</owl:NamedIndividual>
	
	<owl:NamedIndividual rdf:about="&idmp;substanceForm">
		<rdf:type rdf:resource="&owl;Class"/>
		<rdf:type rdf:resource="&skos;Concept"/>
		<rdf:type rdf:resource="&upper;DataObject"/>
		<rdf:type rdf:resource="&upper;LogicalDataEntity"/>
		<rdfs:subClassOf rdf:resource="&skos;Concept"/>
		<skos:altLabel>IDMP.substanceForm</skos:altLabel>
		<skos:definition>Pharmaceutical Product  Substance Form. Defined by substance vocab, reference strength and administerable dose form</skos:definition>
		<skos:prefLabel>Substance form</skos:prefLabel>
		<skos:related rdf:resource="&idmp;PhPIDSubL3"/>
	</owl:NamedIndividual>
	
	<owl:NamedIndividual rdf:about="&idmp;substanceItem">
		<rdf:type rdf:resource="&owl;Class"/>
		<rdf:type rdf:resource="&skos;Concept"/>
		<rdf:type rdf:resource="&upper;DataObject"/>
		<rdf:type rdf:resource="&upper;LogicalDataEntity"/>
		<rdfs:subClassOf rdf:resource="&skos;Concept"/>
		<skos:altLabel>IDMP.substanceItem</skos:altLabel>
		<skos:definition>Substance item</skos:definition>
		<skos:prefLabel>Substance item</skos:prefLabel>
		<skos:related rdf:resource="&idmp;PhPIDSubL1"/>
	</owl:NamedIndividual>
	
	<owl:NamedIndividual rdf:about="&idmp;substanceSet">
		<rdf:type rdf:resource="&owl;Class"/>
		<rdf:type rdf:resource="&skos;Concept"/>
		<rdf:type rdf:resource="&upper;DataObject"/>
		<rdf:type rdf:resource="&upper;LogicalDataEntity"/>
		<rdfs:subClassOf rdf:resource="&skos;Concept"/>
		<skos:altLabel>IDMP.substanceSet</skos:altLabel>
		<skos:definition>Set of attributes that define a substance</skos:definition>
		<skos:prefLabel>Substance set</skos:prefLabel>
		<skos:related rdf:resource="&idmp;PhPIDSub"/>
	</owl:NamedIndividual>
	
	<owl:NamedIndividual rdf:about="&idmp;substanceStrengthItem">
		<rdf:type rdf:resource="&owl;Class"/>
		<rdf:type rdf:resource="&skos;Concept"/>
		<rdf:type rdf:resource="&upper;DataObject"/>
		<rdf:type rdf:resource="&upper;LogicalDataEntity"/>
		<rdfs:subClassOf rdf:resource="&skos;Concept"/>
		<skos:altLabel>IDMP.substanceStrengthItem</skos:altLabel>
		<skos:definition>Substance strength item</skos:definition>
		<skos:prefLabel>Substance strength item</skos:prefLabel>
		<skos:related rdf:resource="&idmp;PhPIDSubL2"/>
	</owl:NamedIndividual>
	
	<owl:NamedIndividual rdf:about="&idmp;version">
		<rdf:type rdf:resource="&owl;Class"/>
		<rdf:type rdf:resource="&skos;Concept"/>
		<rdf:type rdf:resource="&upper;DataObject"/>
		<rdf:type rdf:resource="&upper;LogicalDataEntity"/>
		<rdfs:subClassOf rdf:resource="&skos;Concept"/>
		<skos:altLabel>IDMP.version</skos:altLabel>
		<skos:definition>The characteristics of authorized medicinal products as defined in this standard shall be versioned. This refers to the fact that at the given effective date, some characteristics of the medicinal product have changed. Thesecharacteristics are not different to a sufficient extent to warrant the assignment of a new Primary Identifier Attribute Set</skos:definition>
		<skos:prefLabel>Version</skos:prefLabel>
		<skos:related rdf:resource="&idmp;IMPIDAttributeSet"/>
		<skos:related rdf:resource="&idmp;MPIDAttributeSet"/>
		<skos:related rdf:resource="&idmp;PhPIDSet"/>
		<idmp:hasUMLAttribute rdf:resource="&idmp;version.effectiveDate"/>
		<idmp:hasUMLAttribute rdf:resource="&idmp;version.regulatedDocument"/>
	</owl:NamedIndividual>
	
	<owl:NamedIndividual rdf:about="&idmp;version.effectiveDate">
		<rdf:type rdf:resource="&skos;Concept"/>
		<rdf:type rdf:resource="&upper;DataAttribute"/>
		<rdf:type rdf:resource="&upper;LogicalDataEntity"/>
		<skos:altLabel>IDMP.version.effectiveDate</skos:altLabel>
		<skos:definition>Mechanism that takes into account that at the given effective date, some characteristics of the investigational or authorized medicinal product have changed and those changes may be traced during the entire life cycle of a product. Date from which that mechanism is applicable.</skos:definition>
		<skos:prefLabel>Effective date</skos:prefLabel>
		<idmp:isUMLAttributeOf rdf:resource="&idmp;version"/>
	</owl:NamedIndividual>
	
	<owl:NamedIndividual rdf:about="&idmp;version.regulatedDocument">
		<rdf:type rdf:resource="&skos;Concept"/>
		<rdf:type rdf:resource="&upper;DataAttribute"/>
		<rdf:type rdf:resource="&upper;LogicalDataEntity"/>
		<skos:altLabel>IDMP.version.regulatedDocument</skos:altLabel>
		<skos:definition>The reference to the regulatory decision document related to the granting of the authorization or the latest update of the regulated medicinal product information shall be specified. The reference document ID shall be specified using an integer data type.</skos:definition>
		<skos:prefLabel>Regulated document</skos:prefLabel>
		<idmp:isUMLAttributeOf rdf:resource="&idmp;version"/>
	</owl:NamedIndividual>

</rdf:RDF>