<?xml version="1.0" encoding="UTF-8"?>
<!DOCTYPE rdf:RDF [
	<!ENTITY cmns-cls "https://www.omg.org/spec/Commons/Classifiers/">
	<!ENTITY cmns-col "https://www.omg.org/spec/Commons/Collections/">
	<!ENTITY cmns-cxtdsg "https://www.omg.org/spec/Commons/ContextualDesignators/">
	<!ENTITY cmns-dsg "https://www.omg.org/spec/Commons/Designators/">
	<!ENTITY cmns-qtu "https://www.omg.org/spec/Commons/QuantitiesAndUnits/">
	<!ENTITY dct "http://purl.org/dc/terms/">
	<!ENTITY owl "http://www.w3.org/2002/07/owl#">
	<!ENTITY rdf "http://www.w3.org/1999/02/22-rdf-syntax-ns#">
	<!ENTITY rdfs "http://www.w3.org/2000/01/rdf-schema#">
	<!ENTITY skos "http://www.w3.org/2004/02/skos/core#">
	<!ENTITY sm "http://www.omg.org/techprocess/ab/SpecificationMetadata/">
	<!ENTITY xsd "http://www.w3.org/2001/XMLSchema#">
]>
<rdf:RDF xml:base="https://www.omg.org/spec/Commons/QuantitiesAndUnits/"
	xmlns:cmns-cls="https://www.omg.org/spec/Commons/Classifiers/"
	xmlns:cmns-col="https://www.omg.org/spec/Commons/Collections/"
	xmlns:cmns-cxtdsg="https://www.omg.org/spec/Commons/ContextualDesignators/"
	xmlns:cmns-dsg="https://www.omg.org/spec/Commons/Designators/"
	xmlns:cmns-qtu="https://www.omg.org/spec/Commons/QuantitiesAndUnits/"
	xmlns:dct="http://purl.org/dc/terms/"
	xmlns:owl="http://www.w3.org/2002/07/owl#"
	xmlns:rdf="http://www.w3.org/1999/02/22-rdf-syntax-ns#"
	xmlns:rdfs="http://www.w3.org/2000/01/rdf-schema#"
	xmlns:skos="http://www.w3.org/2004/02/skos/core#"
	xmlns:sm="http://www.omg.org/techprocess/ab/SpecificationMetadata/"
	xmlns:xsd="http://www.w3.org/2001/XMLSchema#">
	
	<owl:Ontology rdf:about="https://www.omg.org/spec/Commons/QuantitiesAndUnits/">
		<rdfs:label>Quantities and Units Ontology</rdfs:label>
		<dct:abstract>This ontology provides a core set of concepts for quantities, units, systems of quantities, and systems of units. The most widely accepted, scrutinized, and globally used system of quantities and system of units are the International System of Quantities (ISQ) and the International System of Units (SI). They are formally standardized through [ISO31] and [IEC60027]. The harmonization of these two sets of standards into one new set [ISO/IEC80000] has been published by ISO in 2009 and 2010. This ontology is derived from the QUDV (Quantities, Units, Dimensions and Values) model in SysML, which, in turn, is based on ISO/IEC 80000-1:2009, which refers normatively to the ISO/IEC Guide 99:2007. Originally developed for use in the Financial Industry Business Ontology (FIBO), it is compatible with and can be mapped directly to the OMG Date Time Vocabulary (DTV) Quantities Ontology, the de-facto QUDT ontology representing Units of Measure, Quantity Kinds, Dimensions and Data Types (see http://www.qudt.org/), the Units of Measurement Ontology (UO) ontology available from the BioPortal (https://bioportal.bioontology.org/ontologies/UO) and others, as well as the QUDV annex of the SysML specification.</dct:abstract>
		<dct:license rdf:datatype="&xsd;anyURI">http://opensource.org/licenses/MIT</dct:license>
		<sm:copyright>Copyright (c) 2015-2022 EDM Council, Inc.</sm:copyright>
		<sm:copyright>Copyright (c) 2015-2022 Object Management Group, Inc.</sm:copyright>
		<owl:imports rdf:resource="https://www.omg.org/spec/Commons/Classifiers/"/>
		<owl:imports rdf:resource="https://www.omg.org/spec/Commons/Collections/"/>
		<owl:imports rdf:resource="https://www.omg.org/spec/Commons/ContextualDesignators/"/>
		<owl:imports rdf:resource="https://www.omg.org/spec/Commons/Designators/"/>
		<owl:versionIRI rdf:resource="https://www.omg.org/spec/Commons/20220201/QuantitiesAndUnits/"/>
	</owl:Ontology>
	
	<owl:Class rdf:about="&cmns-qtu;BaseQuantityKind">
		<rdfs:subClassOf rdf:resource="&cmns-qtu;QuantityKind"/>
		<rdfs:subClassOf>
			<owl:Restriction>
				<owl:onProperty rdf:resource="&cmns-dsg;isDefinedIn"/>
				<owl:onClass rdf:resource="&cmns-qtu;SystemOfQuantities"/>
				<owl:qualifiedCardinality rdf:datatype="&xsd;nonNegativeInteger">1</owl:qualifiedCardinality>
			</owl:Restriction>
		</rdfs:subClassOf>
		<rdfs:label>base quantity kind</rdfs:label>
		<dct:source rdf:datatype="&xsd;anyURI">http://www.omg.org/spec/DTV/</dct:source>
		<dct:source rdf:datatype="&xsd;anyURI">https://www.omg.org/spec/SysML/</dct:source>
		<rdfs:altLabel>simple quantity kind</rdfs:altLabel>
		<skos:definition>quantity kind in a conventionally chosen subset of a given system of quantities, where no subset quantity can be expressed in terms of the others</skos:definition>
		<skos:example>The International System of Quantities (ISQ) comprises these base quantities (with their SI base measurement units): length (meter), mass (kilogram), duration (second), electric current (ampere), thermodynamic temperature (kelvin), amount of substance (mole), and luminous intensity (candela).  These base quantities are not mutually comparable.  All quantities of any one of these kinds are, however, mutually comparable.</skos:example>
	</owl:Class>
	
	<owl:Class rdf:about="&cmns-qtu;BaseUnit">
		<rdfs:subClassOf rdf:resource="&cmns-qtu;PhysicalUnit"/>
		<rdfs:label>base unit</rdfs:label>
		<dct:source rdf:datatype="&xsd;anyURI">http://www.omg.org/spec/DTV/</dct:source>
		<dct:source rdf:datatype="&xsd;anyURI">https://www.omg.org/spec/SysML/</dct:source>
		<rdfs:altLabel>simple unit</rdfs:altLabel>
		<skos:definition>measurement unit that is defined by a system of units to be the reference measurement unit for a base quantity</skos:definition>
		<skos:note>Quantity units that are not base units are derived units.</skos:note>
	</owl:Class>
	
	<owl:Class rdf:about="&cmns-qtu;CoherentDerivedUnit">
		<rdfs:subClassOf rdf:resource="&cmns-qtu;DerivedUnit"/>
		<rdfs:label>coherent derived unit</rdfs:label>
		<skos:definition>derived unit that, for a given system of quantities and for a chosen set of base units, is a product of powers of base units with no other proportionality factor than one</skos:definition>
	</owl:Class>
	
	<owl:Class rdf:about="&cmns-qtu;Constant">
		<rdfs:subClassOf rdf:resource="&cmns-qtu;QuantityValue"/>
		<rdfs:label>constant</rdfs:label>
		<skos:definition>symbol that represents a value that does not change (i.e., is fixed) with respect to a formula or expression</skos:definition>
	</owl:Class>
	
	<owl:Class rdf:about="&cmns-qtu;ConversionBasedUnit">
		<rdfs:subClassOf rdf:resource="&cmns-qtu;DerivedUnit"/>
		<rdfs:subClassOf>
			<owl:Restriction>
				<owl:onProperty rdf:resource="&cmns-qtu;hasExpression"/>
				<owl:someValuesFrom rdf:resource="&cmns-qtu;Expression"/>
			</owl:Restriction>
		</rdfs:subClassOf>
		<rdfs:label>conversion-based unit</rdfs:label>
		<dct:source rdf:datatype="&xsd;anyURI">https://www.omg.org/spec/SysML/</dct:source>
		<skos:definition>derived unit that is defined with respect to another reference unit through an explicit conversion relationship</skos:definition>
	</owl:Class>
	
	<owl:Class rdf:about="&cmns-qtu;DerivedQuantityKind">
		<rdfs:subClassOf rdf:resource="&cmns-qtu;QuantityKind"/>
		<rdfs:subClassOf>
			<owl:Restriction>
				<owl:onProperty rdf:resource="&cmns-qtu;hasFactor"/>
				<owl:someValuesFrom rdf:resource="&cmns-qtu;QuantityKindPowerFactor"/>
			</owl:Restriction>
		</rdfs:subClassOf>
		<rdfs:subClassOf>
			<owl:Restriction>
				<owl:onProperty rdf:resource="&cmns-qtu;isDerivedFrom"/>
				<owl:someValuesFrom rdf:resource="&cmns-qtu;QuantityKind"/>
			</owl:Restriction>
		</rdfs:subClassOf>
		<rdfs:label>derived quantity kind</rdfs:label>
		<dct:source rdf:datatype="&xsd;anyURI">http://www.omg.org/spec/DTV/</dct:source>
		<dct:source rdf:datatype="&xsd;anyURI">https://www.omg.org/spec/SysML/</dct:source>
		<owl:disjointWith rdf:resource="&cmns-qtu;BaseQuantityKind"/>
		<skos:definition>quantity kind that may be defined as a product of powers of one or more other kinds of quantity</skos:definition>
		<skos:example>velocity (length/time), mass density (mass/length3)</skos:example>
		<skos:note>A derived quantity may also be used to define a synonym kind of quantity for another kind of quantity.</skos:note>
	</owl:Class>
	
	<owl:Class rdf:about="&cmns-qtu;DerivedUnit">
		<rdfs:subClassOf rdf:resource="&cmns-qtu;PhysicalUnit"/>
		<rdfs:subClassOf>
			<owl:Restriction>
				<owl:onProperty rdf:resource="&cmns-qtu;hasFactor"/>
				<owl:someValuesFrom rdf:resource="&cmns-qtu;UnitPowerFactor"/>
			</owl:Restriction>
		</rdfs:subClassOf>
		<rdfs:subClassOf>
			<owl:Restriction>
				<owl:onProperty rdf:resource="&cmns-qtu;isDerivedFrom"/>
				<owl:someValuesFrom rdf:resource="&cmns-qtu;BaseUnit"/>
			</owl:Restriction>
		</rdfs:subClassOf>
		<rdfs:label>derived unit</rdfs:label>
		<dct:source rdf:datatype="&xsd;anyURI">http://www.omg.org/spec/DTV/</dct:source>
		<dct:source rdf:datatype="&xsd;anyURI">https://www.omg.org/spec/SysML/</dct:source>
		<skos:definition>measurement unit that is defined with respect to one or more base units, such as as a product of powers of one or more other measurement units</skos:definition>
		<skos:example>1 minute = 60 seconds</skos:example>
		<skos:example>For example velocity can be specified as the product of length to the power one times time to the power minus one, and subsequently speed can be specified as velocity to the power one.</skos:example>
		<skos:note>Every derived unit is defined in terms of base units.</skos:note>
	</owl:Class>
	
	<owl:Class rdf:about="&cmns-qtu;Dimensionality">
		<rdfs:subClassOf rdf:resource="&cmns-cls;Classifier"/>
		<rdfs:subClassOf>
			<owl:Restriction>
				<owl:onProperty rdf:resource="&cmns-qtu;hasFactor"/>
				<owl:onClass rdf:resource="&cmns-qtu;QuantityKindPowerFactor"/>
				<owl:minQualifiedCardinality rdf:datatype="&xsd;nonNegativeInteger">0</owl:minQualifiedCardinality>
			</owl:Restriction>
		</rdfs:subClassOf>
		<rdfs:label>dimensionality</rdfs:label>
		<dct:source>ISO 11179-3:2013 Information technology - Metadata registries (MDR)</dct:source>
		<dct:source rdf:datatype="&xsd;anyURI">https://www.omg.org/spec/SysML/</dct:source>
		<skos:definition>classifier that represents a set of equivalent units of measure</skos:definition>
		<skos:note>Note that this definition is broader than that provided in SysML, which is an expression of the dependence of a quantity on the base quantities of a system of quantities as a product of powers of factors corresponding to the base quantities.</skos:note>
	</owl:Class>
	
	<owl:Class rdf:about="&cmns-qtu;Expression">
		<rdfs:subClassOf>
			<owl:Restriction>
				<owl:onProperty rdf:resource="&cmns-qtu;hasArgument"/>
				<owl:onClass rdf:resource="&cmns-qtu;Constant"/>
				<owl:minQualifiedCardinality rdf:datatype="&xsd;nonNegativeInteger">0</owl:minQualifiedCardinality>
			</owl:Restriction>
		</rdfs:subClassOf>
		<rdfs:subClassOf>
			<owl:Restriction>
				<owl:onProperty rdf:resource="&cmns-qtu;hasArgument"/>
				<owl:onClass rdf:resource="&cmns-qtu;Variable"/>
				<owl:minQualifiedCardinality rdf:datatype="&xsd;nonNegativeInteger">0</owl:minQualifiedCardinality>
			</owl:Restriction>
		</rdfs:subClassOf>
		<rdfs:label>expression</rdfs:label>
		<skos:definition>finite combination of symbols that are well-formed according to applicable rules</skos:definition>
	</owl:Class>
	
	<owl:Class rdf:about="&cmns-qtu;Factor">
		<rdfs:label>factor</rdfs:label>
		<skos:definition>number or quantity that when multiplied with another produces a given number or expression</skos:definition>
	</owl:Class>
	
	<owl:Class rdf:about="&cmns-qtu;IntervalScale">
		<rdfs:subClassOf rdf:resource="&cmns-qtu;MeasurementScale"/>
		<rdfs:label>interval scale</rdfs:label>
		<dct:source rdf:datatype="&xsd;anyURI">https://plato.stanford.edu/entries/measurement-science/</dct:source>
		<dct:source rdf:datatype="&xsd;anyURI">https://www.omg.org/spec/SysML/</dct:source>
		<dct:source rdf:datatype="&xsd;anyURI">https://www.statista.com/statistics-glossary/definition/320/interval_scale/</dct:source>
		<skos:definition>measurement scale that represents quantitative values and for which mode, median and mean can be calculated</skos:definition>
		<skos:example>Celsius and Fahrenheit are examples of interval scales: they represent equality or inequality among intervals of temperature, but not ratios of temperature, because their zero points are arbitrary. Rating scales, where it is assumed that the distances between the single expressions of evaluation (score) are equal, are also interval scales with no natural zero point.</skos:example>
		<skos:note>Linear interval scales allow both multiplication by a positive number and a constant shift, e.g., the conversion from Celsius to Fahrenheit in accordance with the formula °C × 9/5 + 32 = °F.</skos:note>
	</owl:Class>
	
	<owl:Class rdf:about="&cmns-qtu;LogarithmicScale">
		<rdfs:subClassOf rdf:resource="&cmns-qtu;MeasurementScale"/>
		<rdfs:label>logarithmic scale</rdfs:label>
		<dct:source rdf:datatype="&xsd;anyURI">https://en.wikipedia.org/wiki/Logarithmic_scale/</dct:source>
		<dct:source rdf:datatype="&xsd;anyURI">https://plato.stanford.edu/entries/measurement-science/</dct:source>
		<dct:source rdf:datatype="&xsd;anyURI">https://www.omg.org/spec/SysML/</dct:source>
		<skos:definition>measurement scale on which the actual distance of a point from the scale&apos;s zero is proportional to the logarithm of the corresponding scale number rather than to the number itself</skos:definition>
		<skos:example>A logarithmic scale (or log scale) is a way of displaying numerical data over a very wide range of values in a compact way - typically the largest numbers in the data are hundreds or even thousands of times larger than the smallest numbers. Such a scale is nonlinear: the numbers 10 and 20, and 60 and 70, are not the same distance apart on a log scale. Rather, the numbers 10 and 100, and 60 and 600 are equally spaced. Thus moving a unit of distance along the scale means the number has been multiplied by 10 (or some other fixed factor).</skos:example>
	</owl:Class>
	
	<owl:Class rdf:about="&cmns-qtu;Measure">
		<rdfs:label>measure</rdfs:label>
		<dct:source rdf:datatype="&xsd;anyURI">https://stats.oecd.org/glossary/detail.asp?ID=7062</dct:source>
		<skos:definition>amount or degree of something; the dimensions, capacity, or amount of something ascertained by measuring</skos:definition>
		<skos:note>Measure refers to the phenomenon or phenomena to be measured in a data set. In a data set, the instance of a measure is often called an observation.</skos:note>
	</owl:Class>
	
	<owl:Class rdf:about="&cmns-qtu;MeasurementScale">
		<rdfs:subClassOf rdf:resource="&cmns-cls;ClassificationScheme"/>
		<rdfs:subClassOf>
			<owl:Restriction>
				<owl:onProperty rdf:resource="&cmns-qtu;hasMaximumPermissiveValue"/>
				<owl:onClass rdf:resource="&cmns-qtu;QuantityValue"/>
				<owl:minQualifiedCardinality rdf:datatype="&xsd;nonNegativeInteger">0</owl:minQualifiedCardinality>
			</owl:Restriction>
		</rdfs:subClassOf>
		<rdfs:subClassOf>
			<owl:Restriction>
				<owl:onProperty rdf:resource="&cmns-qtu;hasMinimumPermissiveValue"/>
				<owl:onClass rdf:resource="&cmns-qtu;QuantityValue"/>
				<owl:minQualifiedCardinality rdf:datatype="&xsd;nonNegativeInteger">0</owl:minQualifiedCardinality>
			</owl:Restriction>
		</rdfs:subClassOf>
		<rdfs:subClassOf>
			<owl:Restriction>
				<owl:onProperty rdf:resource="&cmns-qtu;isMaximumInclusive"/>
				<owl:minQualifiedCardinality rdf:datatype="&xsd;nonNegativeInteger">0</owl:minQualifiedCardinality>
				<owl:onDataRange rdf:resource="&xsd;boolean"/>
			</owl:Restriction>
		</rdfs:subClassOf>
		<rdfs:subClassOf>
			<owl:Restriction>
				<owl:onProperty rdf:resource="&cmns-qtu;isMinimumInclusive"/>
				<owl:minQualifiedCardinality rdf:datatype="&xsd;nonNegativeInteger">0</owl:minQualifiedCardinality>
				<owl:onDataRange rdf:resource="&xsd;boolean"/>
			</owl:Restriction>
		</rdfs:subClassOf>
		<rdfs:subClassOf>
			<owl:Restriction>
				<owl:onProperty rdf:resource="&cmns-cls;classifies"/>
				<owl:someValuesFrom rdf:resource="&cmns-qtu;MeasurementUnit"/>
			</owl:Restriction>
		</rdfs:subClassOf>
		<rdfs:label>measurement scale</rdfs:label>
		<dct:source rdf:datatype="&xsd;anyURI">https://plato.stanford.edu/entries/measurement-science/</dct:source>
		<dct:source rdf:datatype="&xsd;anyURI">https://www.omg.org/spec/SysML/</dct:source>
		<skos:definition>classification scheme that provides a many-to-one mapping from an empirical to a numerical relational structure, acting as a reference against which measurements can be compared</skos:definition>
	</owl:Class>
	
	<owl:Class rdf:about="&cmns-qtu;MeasurementUnit">
		<rdfs:subClassOf rdf:resource="&cmns-qtu;Quantity"/>
		<rdfs:subClassOf>
			<owl:Restriction>
				<owl:onProperty rdf:resource="&cmns-qtu;specializes"/>
				<owl:onClass rdf:resource="&cmns-qtu;MeasurementUnit"/>
				<owl:minQualifiedCardinality rdf:datatype="&xsd;nonNegativeInteger">0</owl:minQualifiedCardinality>
			</owl:Restriction>
		</rdfs:subClassOf>
		<rdfs:subClassOf>
			<owl:Restriction>
				<owl:onProperty rdf:resource="&cmns-dsg;isDefinedIn"/>
				<owl:onClass rdf:resource="&cmns-qtu;SystemOfUnits"/>
				<owl:minQualifiedCardinality rdf:datatype="&xsd;nonNegativeInteger">0</owl:minQualifiedCardinality>
			</owl:Restriction>
		</rdfs:subClassOf>
		<rdfs:subClassOf>
			<owl:Restriction>
				<owl:onProperty rdf:resource="&cmns-qtu;hasFactor"/>
				<owl:onClass rdf:resource="&cmns-qtu;UnitPowerFactor"/>
				<owl:minQualifiedCardinality rdf:datatype="&xsd;nonNegativeInteger">0</owl:minQualifiedCardinality>
			</owl:Restriction>
		</rdfs:subClassOf>
		<rdfs:subClassOf>
			<owl:Restriction>
				<owl:onProperty rdf:resource="&cmns-qtu;hasQuantityKind"/>
				<owl:onClass rdf:resource="&cmns-qtu;QuantityKind"/>
				<owl:qualifiedCardinality rdf:datatype="&xsd;nonNegativeInteger">1</owl:qualifiedCardinality>
			</owl:Restriction>
		</rdfs:subClassOf>
		<rdfs:label>measurement unit</rdfs:label>
		<dct:source rdf:datatype="&xsd;anyURI">http://www.omg.org/spec/DTV/</dct:source>
		<dct:source rdf:datatype="&xsd;anyURI">https://www.omg.org/spec/SysML/</dct:source>
		<skos:definition>quantity, defined and adopted by convention, with which any other quantity of the same kind can be compared to express the ratio of the two quantities as a number</skos:definition>
		<skos:example>week, day, hour, minute, second, kilogram, joule, meter</skos:example>
		<skos:note>A Unit is a quantity in terms of which the magnitudes of other quantities that have the same quantity kind can be stated. A unit often relies on precise and reproducible ways to measure the unit. For example, a unit of length such as meter may be specified as a multiple of a particular wavelength of light. A unit may also specify less stable or precise ways to express some value, such as a cost expressed in some currency, or a severity rating measured by a numerical scale.</skos:note>
	</owl:Class>
	
	<owl:Class rdf:about="&cmns-qtu;NominalScale">
		<rdfs:subClassOf rdf:resource="&cmns-qtu;MeasurementScale"/>
		<rdfs:label>nominal scale</rdfs:label>
		<dct:source rdf:datatype="&xsd;anyURI">https://plato.stanford.edu/entries/measurement-science/</dct:source>
		<dct:source rdf:datatype="&xsd;anyURI">https://www.ncbi.nlm.nih.gov/pmc/articles/PMC4589638/</dct:source>
		<skos:definition>measurement scale that represents objects as belonging to classes that have no particular order</skos:definition>
		<skos:example>Many nominal scales are qualitative in nature. A common example of a nominal scale is that of gender identity, which is a way of describing one&apos;s persistent inner concept of their gender. While the terminology from a psychological and medical perspective continues to evolve, the scale covers individuals who self identify as male or female as well as those that have an indeterminate perspective, such as transsexual or non-binary.</skos:example>
	</owl:Class>
	
	<owl:Class rdf:about="&cmns-qtu;OrdinalScale">
		<rdfs:subClassOf rdf:resource="&cmns-qtu;MeasurementScale"/>
		<rdfs:label>ordinal scale</rdfs:label>
		<dct:source rdf:datatype="&xsd;anyURI">https://plato.stanford.edu/entries/measurement-science/</dct:source>
		<dct:source rdf:datatype="&xsd;anyURI">https://www.omg.org/spec/SysML/</dct:source>
		<skos:definition>measurement scale that represents order but no further algebraic structure</skos:definition>
		<skos:example>For example, the Mohs scale of mineral hardness represents minerals with numbers ranging from 1 (softest) to 10 (hardest), but there is no empirical significance to equality among intervals or ratios of those numbers.</skos:example>
		<skos:note>Ordinal scales allow any transformation function as long as it is monotonic and increasing.</skos:note>
	</owl:Class>
	
	<owl:Class rdf:about="&cmns-qtu;Percentage">
		<rdfs:subClassOf rdf:resource="&cmns-qtu;Ratio"/>
		<rdfs:label>percentage</rdfs:label>
		<skos:definition>ratio value expressed as a fraction of 100, i.e., in which the denominator is fixed rather than variable and equal to 100</skos:definition>
		<skos:note>The percent value is computed by multiplying the numeric value of the ratio by 100.</skos:note>
		<skos:note>While many percentage values are between 0 and 100, there is no mathematical restriction and percentages may take on other values (positive or negative), particularly in the case of comparisons (percent change).</skos:note>
	</owl:Class>
	
	<owl:Class rdf:about="&cmns-qtu;PhysicalUnit">
		<rdfs:subClassOf rdf:resource="&cmns-qtu;MeasurementUnit"/>
		<rdfs:subClassOf>
			<owl:Restriction>
				<owl:onProperty rdf:resource="&cmns-dsg;isDefinedIn"/>
				<owl:someValuesFrom rdf:resource="&cmns-qtu;SystemOfUnits"/>
			</owl:Restriction>
		</rdfs:subClassOf>
		<rdfs:label>physical unit</rdfs:label>
		<dct:source>ISO 11240:2012, clause 3.1.1</dct:source>
		<skos:definition>unit of measurement that is defined using a physical quantity</skos:definition>
		<skos:note>Its definition relates measured quantities to the base quantities through a set of well-defined equations.</skos:note>
		<skos:note>Physical units and their related scales are defined independently of the measurement procedure and the measured components. They relate to an internationally standardized system of units and equations governing the mathematical relations between those units.</skos:note>
	</owl:Class>
	
	<owl:Class rdf:about="&cmns-qtu;Prefix">
		<rdfs:subClassOf rdf:resource="&cmns-qtu;Factor"/>
		<rdfs:subClassOf>
			<owl:Restriction>
				<owl:onProperty rdf:resource="&cmns-qtu;hasFactorValue"/>
				<owl:onDataRange rdf:resource="&owl;rational"/>
				<owl:qualifiedCardinality rdf:datatype="&xsd;nonNegativeInteger">1</owl:qualifiedCardinality>
			</owl:Restriction>
		</rdfs:subClassOf>
		<rdfs:label>prefix</rdfs:label>
		<skos:definition>named multiple or submultiple multiplication factor used in the specification of a derived unit</skos:definition>
		<skos:note>A system of units may specify a set of prefixes.</skos:note>
	</owl:Class>
	
	<owl:Class rdf:about="&cmns-qtu;PrefixedUnit">
		<rdfs:subClassOf rdf:resource="&cmns-qtu;ConversionBasedUnit"/>
		<rdfs:subClassOf>
			<owl:Restriction>
				<owl:onProperty rdf:resource="&cmns-qtu;hasFactor"/>
				<owl:someValuesFrom rdf:resource="&cmns-qtu;Prefix"/>
			</owl:Restriction>
		</rdfs:subClassOf>
		<rdfs:label>prefixed unit</rdfs:label>
		<dct:source rdf:datatype="&xsd;anyURI">https://www.omg.org/spec/SysML/</dct:source>
		<skos:definition>conversion-based unit that is defined with respect to another measurement reference unit through a linear conversion relationship with a named prefix that represents a multiple or submultiple of a unit</skos:definition>
	</owl:Class>
	
	<owl:Class rdf:about="&cmns-qtu;Quantity">
		<rdfs:subClassOf rdf:resource="&cmns-qtu;Measure"/>
		<rdfs:subClassOf>
			<owl:Restriction>
				<owl:onProperty rdf:resource="&cmns-dsg;hasName"/>
				<owl:someValuesFrom rdf:resource="&cmns-qtu;QuantityName"/>
			</owl:Restriction>
		</rdfs:subClassOf>
		<rdfs:subClassOf>
			<owl:Restriction>
				<owl:onProperty rdf:resource="&cmns-qtu;hasQuantityKind"/>
				<owl:someValuesFrom rdf:resource="&cmns-qtu;QuantityKind"/>
			</owl:Restriction>
		</rdfs:subClassOf>
		<rdfs:label>quantity</rdfs:label>
		<dct:source rdf:datatype="&xsd;anyURI">http://www.omg.org/spec/DTV/</dct:source>
		<dct:source rdf:datatype="&xsd;anyURI">https://www.omg.org/spec/SysML/</dct:source>
		<skos:definition>property of a phenomenon, body, or substance, to which a number can be assigned with respect to a reference</skos:definition>
		<skos:editorialNote>The term quantity is used here to refer to the abstraction of the properties - the amount of measurable stuff that can be compared between particular quantities. The height of the something refers to a particular quantity; 555 ft 5 inches refers to a quantity value.</skos:editorialNote>
		<skos:example>second, kilogram, joule, meter. These are quantities in a general sense, which is what is meant here by quantity.</skos:example>
		<skos:note>A quantity as defined here is said to be a &quot;scalar&quot; as distinct from a &quot;vector.&quot; However, a vector or a tensor whose components are quantities is also considered to be a quantity.</skos:note>
	</owl:Class>
	
	<owl:Class rdf:about="&cmns-qtu;QuantityKind">
		<rdfs:subClassOf rdf:resource="&cmns-cls;Classifier"/>
		<rdfs:subClassOf>
			<owl:Restriction>
				<owl:onProperty rdf:resource="&cmns-qtu;hasMeasurementUnit"/>
				<owl:onClass rdf:resource="&cmns-qtu;MeasurementUnit"/>
				<owl:minQualifiedCardinality rdf:datatype="&xsd;nonNegativeInteger">0</owl:minQualifiedCardinality>
			</owl:Restriction>
		</rdfs:subClassOf>
		<rdfs:subClassOf>
			<owl:Restriction>
				<owl:onProperty rdf:resource="&cmns-qtu;specializes"/>
				<owl:onClass rdf:resource="&cmns-qtu;QuantityKind"/>
				<owl:minQualifiedCardinality rdf:datatype="&xsd;nonNegativeInteger">0</owl:minQualifiedCardinality>
			</owl:Restriction>
		</rdfs:subClassOf>
		<rdfs:subClassOf>
			<owl:Restriction>
				<owl:onProperty rdf:resource="&cmns-dsg;isDefinedIn"/>
				<owl:onClass rdf:resource="&cmns-qtu;SystemOfQuantities"/>
				<owl:minQualifiedCardinality rdf:datatype="&xsd;nonNegativeInteger">0</owl:minQualifiedCardinality>
			</owl:Restriction>
		</rdfs:subClassOf>
		<rdfs:label>quantity kind</rdfs:label>
		<dct:source rdf:datatype="&xsd;anyURI">http://www.omg.org/spec/DTV/</dct:source>
		<dct:source rdf:datatype="&xsd;anyURI">https://www.omg.org/spec/SysML/</dct:source>
		<skos:definition>classifier that characterizes quantities as being mutually comparable</skos:definition>
		<skos:note>A QuantityKind is a kind of quantity that may be stated by means of defined units. For example, the quantity kind of length may be measured by units of meters, kilometers, or feet. Note that this definition allows for dimensionless quantity kinds, such as rates.</skos:note>
		<skos:note>Every instance of &apos;quantity kind&apos; is also a specialization of &apos;quantity&apos;. So the concept &apos;duration&apos; is an instance of &apos;quantity kind&apos; and it is a specialization of &apos;quantity&apos;, i.e., it is a classifier of actual quantities. But a given duration (i.e., the duration of something) is an instance of &apos;duration&apos; and thus a &apos;quantity value,&apos; not an instance of &apos;quantity kind&apos;. For example, a &apos;year&apos; is not an instance of quantity kind; it is an instance of quantity, but not a category of quantity.</skos:note>
	</owl:Class>
	
	<owl:Class rdf:about="&cmns-qtu;QuantityKindPowerFactor">
		<rdfs:subClassOf rdf:resource="&cmns-qtu;Factor"/>
		<rdfs:subClassOf>
			<owl:Restriction>
				<owl:onProperty rdf:resource="&cmns-qtu;hasExponent"/>
				<owl:onDataRange rdf:resource="&owl;rational"/>
				<owl:qualifiedCardinality rdf:datatype="&xsd;nonNegativeInteger">1</owl:qualifiedCardinality>
			</owl:Restriction>
		</rdfs:subClassOf>
		<rdfs:subClassOf>
			<owl:Restriction>
				<owl:onProperty rdf:resource="&cmns-qtu;hasQuantityKind"/>
				<owl:someValuesFrom rdf:resource="&cmns-qtu;QuantityKind"/>
			</owl:Restriction>
		</rdfs:subClassOf>
		<rdfs:label>quantity kind power factor</rdfs:label>
		<dct:source rdf:datatype="&xsd;anyURI">https://www.omg.org/spec/SysML/</dct:source>
		<skos:definition>factor in a product of powers that defines a derived quantity</skos:definition>
	</owl:Class>
	
	<owl:Class rdf:about="&cmns-qtu;QuantityName">
		<rdfs:subClassOf rdf:resource="&cmns-dsg;Name"/>
		<rdfs:subClassOf>
			<owl:Restriction>
				<owl:onProperty rdf:resource="&cmns-dsg;isNameOf"/>
				<owl:someValuesFrom rdf:resource="&cmns-qtu;Quantity"/>
			</owl:Restriction>
		</rdfs:subClassOf>
		<rdfs:label>quantity name</rdfs:label>
		<skos:definition>human-readable textual representation of the quantity</skos:definition>
		<skos:note>A number of systems of quantities and units encode a quantity, such as a unit of measure, via a generally accepted abbreviation. URIs representing such quantities are very useful in applications that require globally unique, machine readable names, but are less accessible to people. This concept is intended to provide the corresponding name for a given quantity in the context of a specific system of quantities and units for human consumption.</skos:note>
	</owl:Class>
	
	<owl:Class rdf:about="&cmns-qtu;QuantityValue">
		<rdfs:subClassOf>
			<owl:Restriction>
				<owl:onProperty rdf:resource="&cmns-qtu;hasMeasurementUnit"/>
				<owl:onClass rdf:resource="&cmns-qtu;MeasurementUnit"/>
				<owl:maxQualifiedCardinality rdf:datatype="&xsd;nonNegativeInteger">1</owl:maxQualifiedCardinality>
			</owl:Restriction>
		</rdfs:subClassOf>
		<rdfs:subClassOf>
			<owl:Restriction>
				<owl:onProperty rdf:resource="&cmns-qtu;expressesTheMagnitudeOf"/>
				<owl:onClass rdf:resource="&cmns-qtu;Quantity"/>
				<owl:minQualifiedCardinality rdf:datatype="&xsd;nonNegativeInteger">0</owl:minQualifiedCardinality>
			</owl:Restriction>
		</rdfs:subClassOf>
		<rdfs:subClassOf>
			<owl:Restriction>
				<owl:onProperty rdf:resource="&cmns-qtu;hasNumericValue"/>
				<owl:onDataRange rdf:resource="&xsd;decimal"/>
				<owl:qualifiedCardinality rdf:datatype="&xsd;nonNegativeInteger">1</owl:qualifiedCardinality>
			</owl:Restriction>
		</rdfs:subClassOf>
		<rdfs:label>quantity value</rdfs:label>
		<dct:source rdf:datatype="&xsd;anyURI">http://www.omg.org/spec/DTV/</dct:source>
		<dct:source rdf:datatype="&xsd;anyURI">https://www.omg.org/spec/SysML/</dct:source>
		<rdfs:altLabel>measurement</rdfs:altLabel>
		<skos:definition>number and measurement unit together giving magnitude of a quantity</skos:definition>
		<skos:example>2 days, 3.5 hours, 150 lb, 45.5 miles</skos:example>
		<skos:note>The quantity expressed by a quantity value is the quantity whose ratio to the measurement unit is the number.  Note that dimensionless quantities may not have a measurement unit associated with them.</skos:note>
	</owl:Class>
	
	<owl:Class rdf:about="&cmns-qtu;Ratio">
		<rdfs:subClassOf rdf:resource="&cmns-qtu;Expression"/>
		<rdfs:subClassOf>
			<owl:Restriction>
				<owl:onProperty rdf:resource="&cmns-qtu;hasDenominator"/>
				<owl:onClass rdf:resource="&cmns-qtu;QuantityValue"/>
				<owl:qualifiedCardinality rdf:datatype="&xsd;nonNegativeInteger">1</owl:qualifiedCardinality>
			</owl:Restriction>
		</rdfs:subClassOf>
		<rdfs:subClassOf>
			<owl:Restriction>
				<owl:onProperty rdf:resource="&cmns-qtu;hasNumerator"/>
				<owl:onClass rdf:resource="&cmns-qtu;QuantityValue"/>
				<owl:qualifiedCardinality rdf:datatype="&xsd;nonNegativeInteger">1</owl:qualifiedCardinality>
			</owl:Restriction>
		</rdfs:subClassOf>
		<rdfs:label>ratio</rdfs:label>
		<dct:source rdf:datatype="&xsd;anyURI">https://stats.oecd.org/glossary/detail.asp?ID=6688</dct:source>
		<dct:source rdf:datatype="&xsd;anyURI">https://www150.statcan.gc.ca/n1/edu/power-pouvoir/glossary-glossaire/5214842-eng.htm#r.</dct:source>
		<rdfs:altLabel>rate</rdfs:altLabel>
		<skos:definition>proportional relationship between two different quantity values that gives rise to a datum of a specific quantity kind</skos:definition>
		<skos:note>A ratio is a quantity measured with respect to some other quantity, or in mathematics a quotient of two numbers or expressions, arrived at by dividing one by the other.</skos:note>
	</owl:Class>
	
	<owl:Class rdf:about="&cmns-qtu;RatioScale">
		<rdfs:subClassOf rdf:resource="&cmns-qtu;MeasurementScale"/>
		<rdfs:label>ratio scale</rdfs:label>
		<dct:source rdf:datatype="&xsd;anyURI">https://plato.stanford.edu/entries/measurement-science/</dct:source>
		<dct:source rdf:datatype="&xsd;anyURI">https://www.omg.org/spec/SysML/</dct:source>
		<skos:definition>measurement scale that represents quantitative values, allows comparison of differences in values, has a fixed zero value and is invariant under multiplication by a positive number</skos:definition>
		<skos:example>The Kelvin scale is a ratio scale, as are the familiar scales representing mass in kilograms, length in meters and duration in seconds.</skos:example>
	</owl:Class>
	
	<owl:Class rdf:about="&cmns-qtu;SystemOfQuantities">
		<rdfs:subClassOf rdf:resource="&cmns-cls;ClassificationScheme"/>
		<rdfs:subClassOf>
			<owl:Restriction>
				<owl:onProperty rdf:resource="&cmns-col;comprises"/>
				<owl:onClass rdf:resource="&cmns-qtu;SystemOfQuantities"/>
				<owl:minQualifiedCardinality rdf:datatype="&xsd;nonNegativeInteger">0</owl:minQualifiedCardinality>
			</owl:Restriction>
		</rdfs:subClassOf>
		<rdfs:subClassOf>
			<owl:Restriction>
				<owl:onProperty rdf:resource="&cmns-cxtdsg;uses"/>
				<owl:onClass rdf:resource="&cmns-qtu;SystemOfQuantities"/>
				<owl:minQualifiedCardinality rdf:datatype="&xsd;nonNegativeInteger">0</owl:minQualifiedCardinality>
			</owl:Restriction>
		</rdfs:subClassOf>
		<rdfs:subClassOf>
			<owl:Restriction>
				<owl:onProperty rdf:resource="&cmns-dsg;defines"/>
				<owl:someValuesFrom rdf:resource="&cmns-qtu;QuantityKind"/>
			</owl:Restriction>
		</rdfs:subClassOf>
		<rdfs:label xml:lang="en">system of quantities</rdfs:label>
		<dct:source rdf:datatype="&xsd;anyURI">http://www.omg.org/spec/DTV/</dct:source>
		<dct:source rdf:datatype="&xsd;anyURI">https://www.omg.org/spec/SysML/</dct:source>
		<skos:definition>set of quantities together with a set of non-contradictory equations relating those quantities</skos:definition>
		<skos:example>The International System of Quantities (ISQ) is an example of a SystemOfQuantities, defined in ISO 31 and ISO/IEC 80000.</skos:example>
	</owl:Class>
	
	<owl:Class rdf:about="&cmns-qtu;SystemOfUnits">
		<rdfs:subClassOf rdf:resource="&cmns-cls;ClassificationScheme"/>
		<rdfs:subClassOf>
			<owl:Restriction>
				<owl:onProperty rdf:resource="&cmns-col;comprises"/>
				<owl:onClass rdf:resource="&cmns-qtu;SystemOfUnits"/>
				<owl:minQualifiedCardinality rdf:datatype="&xsd;nonNegativeInteger">0</owl:minQualifiedCardinality>
			</owl:Restriction>
		</rdfs:subClassOf>
		<rdfs:subClassOf>
			<owl:Restriction>
				<owl:onProperty rdf:resource="&cmns-cxtdsg;uses"/>
				<owl:onClass rdf:resource="&cmns-qtu;SystemOfUnits"/>
				<owl:minQualifiedCardinality rdf:datatype="&xsd;nonNegativeInteger">0</owl:minQualifiedCardinality>
			</owl:Restriction>
		</rdfs:subClassOf>
		<rdfs:subClassOf>
			<owl:Restriction>
				<owl:onProperty rdf:resource="&cmns-col;compliesWith"/>
				<owl:onClass rdf:resource="&cmns-qtu;SystemOfQuantities"/>
				<owl:qualifiedCardinality rdf:datatype="&xsd;nonNegativeInteger">1</owl:qualifiedCardinality>
			</owl:Restriction>
		</rdfs:subClassOf>
		<rdfs:subClassOf>
			<owl:Restriction>
				<owl:onProperty rdf:resource="&cmns-dsg;defines"/>
				<owl:someValuesFrom rdf:resource="&cmns-qtu;MeasurementUnit"/>
			</owl:Restriction>
		</rdfs:subClassOf>
		<rdfs:label>system of units</rdfs:label>
		<dct:source rdf:datatype="&xsd;anyURI">http://www.omg.org/spec/DTV/</dct:source>
		<dct:source rdf:datatype="&xsd;anyURI">https://www.omg.org/spec/SysML/</dct:source>
		<skos:definition>set of measurement units associated with a system of quantities, together with a set of rules that assign one measurement unit to be the base unit for each base quantity in the system of quantities and a set of rules for the derivation of other units from the base units</skos:definition>
		<skos:example>The International System of Units (SI) is a system of units.</skos:example>
	</owl:Class>
	
	<owl:Class rdf:about="&cmns-qtu;UnitPowerFactor">
		<rdfs:subClassOf rdf:resource="&cmns-qtu;Factor"/>
		<rdfs:subClassOf>
			<owl:Restriction>
				<owl:onProperty rdf:resource="&cmns-qtu;hasMeasurementUnit"/>
				<owl:onClass rdf:resource="&cmns-qtu;MeasurementUnit"/>
				<owl:qualifiedCardinality rdf:datatype="&xsd;nonNegativeInteger">1</owl:qualifiedCardinality>
			</owl:Restriction>
		</rdfs:subClassOf>
		<rdfs:subClassOf>
			<owl:Restriction>
				<owl:onProperty rdf:resource="&cmns-qtu;hasExponent"/>
				<owl:onDataRange rdf:resource="&owl;rational"/>
				<owl:qualifiedCardinality rdf:datatype="&xsd;nonNegativeInteger">1</owl:qualifiedCardinality>
			</owl:Restriction>
		</rdfs:subClassOf>
		<rdfs:label>unit power factor</rdfs:label>
		<dct:source rdf:datatype="&xsd;anyURI">https://www.omg.org/spec/SysML/</dct:source>
		<skos:definition>factor in a product of powers that defines a derived unit</skos:definition>
	</owl:Class>
	
	<owl:Class rdf:about="&cmns-qtu;Variable">
		<rdfs:subClassOf rdf:resource="&cmns-qtu;QuantityValue"/>
		<rdfs:label>variable</rdfs:label>
		<skos:definition>symbol that represents a parameter in a formula or expression</skos:definition>
	</owl:Class>
	
	<owl:AnnotationProperty rdf:about="&cmns-qtu;describesActualExpression">
		<rdfs:subPropertyOf rdf:resource="&cmns-dsg;hasDescription"/>
		<rdfs:label>describes actual expression</rdfs:label>
		<skos:definition>specifies the calculation or expression used to determine the value of something</skos:definition>
		<skos:note>In cases where some expression can only be calculated in SPARQL or via rules, this property is useful for stating what that calculation should be using the input arguments to the expression.</skos:note>
	</owl:AnnotationProperty>
	
	<owl:ObjectProperty rdf:about="&cmns-qtu;expressesTheMagnitudeOf">
		<rdfs:label>expresses the magnitude of</rdfs:label>
		<rdfs:range rdf:resource="&cmns-qtu;Quantity"/>
		<skos:definition>specifies the quantity that some quantity value reflects</skos:definition>
	</owl:ObjectProperty>
	
	<owl:ObjectProperty rdf:about="&cmns-qtu;hasArgument">
		<rdfs:label>has argument</rdfs:label>
		<rdfs:altLabel>has independent variable</rdfs:altLabel>
		<rdfs:range rdf:resource="&cmns-qtu;Variable"/>
		<skos:definition>indicates a specific input to a function, formula or expression, also known as an independent variable</skos:definition>
	</owl:ObjectProperty>
	
	<owl:ObjectProperty rdf:about="&cmns-qtu;hasDenominator">
		<rdfs:subPropertyOf rdf:resource="&cmns-qtu;hasArgument"/>
		<rdfs:label>has denominator</rdfs:label>
		<rdfs:range rdf:resource="&cmns-qtu;QuantityValue"/>
		<skos:definition>specifies the quantity value that is the part of a fraction &apos;below the line&apos; and signifies the value by which the numerator should be divided</skos:definition>
		<skos:note>If a fraction is considered as an ordered pair, the denominator is the second argument of the fraction.</skos:note>
	</owl:ObjectProperty>
	
	<owl:ObjectProperty rdf:about="&cmns-qtu;hasDimension">
		<rdfs:label>has dimension</rdfs:label>
		<rdfs:domain rdf:resource="&cmns-qtu;QuantityKind"/>
		<rdfs:range rdf:resource="&cmns-qtu;Dimensionality"/>
		<skos:definition>indicates a measurable extent associated with a given quantity kind in some system of quantities, which may be derived, depending on the choice of base quantity</skos:definition>
	</owl:ObjectProperty>
	
	<owl:DatatypeProperty rdf:about="&cmns-qtu;hasExponent">
		<rdfs:label>has exponent</rdfs:label>
		<rdfs:range rdf:resource="&owl;rational"/>
		<skos:definition>indicates the number of times a number should be multiplied by itself</skos:definition>
	</owl:DatatypeProperty>
	
	<owl:ObjectProperty rdf:about="&cmns-qtu;hasExpression">
		<rdfs:label>has expression</rdfs:label>
		<rdfs:range rdf:resource="&cmns-qtu;Expression"/>
		<skos:definition>specifies a finite combination of symbols, including constants, variables that may be ordered via one or more operators, that is well-formed according to rules that depend on the language and context</skos:definition>
	</owl:ObjectProperty>
	
	<owl:ObjectProperty rdf:about="&cmns-qtu;hasFactor">
		<rdfs:subPropertyOf rdf:resource="&cmns-qtu;hasArgument"/>
		<rdfs:label>has factor</rdfs:label>
		<skos:definition>indicates a number or quantity that when multiplied with another produces a given number or expression</skos:definition>
	</owl:ObjectProperty>
	
	<owl:DatatypeProperty rdf:about="&cmns-qtu;hasFactorValue">
		<rdfs:label>has factor value</rdfs:label>
		<rdfs:range rdf:resource="&owl;rational"/>
		<skos:definition>indicates the numeric multiple or submultiple multiplication factor</skos:definition>
	</owl:DatatypeProperty>
	
	<owl:ObjectProperty rdf:about="&cmns-qtu;hasMaximumPermissiveValue">
		<rdfs:label>has maximum permissive value</rdfs:label>
		<rdfs:domain rdf:resource="&cmns-qtu;MeasurementScale"/>
		<rdfs:range rdf:resource="&cmns-qtu;QuantityValue"/>
		<skos:definition>indicates the maximum allowed value for a measurement on the given scale</skos:definition>
	</owl:ObjectProperty>
	
	<owl:ObjectProperty rdf:about="&cmns-qtu;hasMeasurementUnit">
		<rdfs:label>has measurement unit</rdfs:label>
		<rdfs:range rdf:resource="&cmns-qtu;MeasurementUnit"/>
		<skos:definition>indicates the unit in which something is expressed</skos:definition>
	</owl:ObjectProperty>
	
	<owl:ObjectProperty rdf:about="&cmns-qtu;hasMinimumPermissiveValue">
		<rdfs:label>has minimum permissive value</rdfs:label>
		<rdfs:domain rdf:resource="&cmns-qtu;MeasurementScale"/>
		<rdfs:range rdf:resource="&cmns-qtu;QuantityValue"/>
		<skos:definition>indicates the minimum allowed value for a measurement on the given scale</skos:definition>
	</owl:ObjectProperty>
	
	<owl:ObjectProperty rdf:about="&cmns-qtu;hasNumerator">
		<rdfs:subPropertyOf rdf:resource="&cmns-qtu;hasArgument"/>
		<rdfs:label>has numerator</rdfs:label>
		<rdfs:range rdf:resource="&cmns-qtu;QuantityValue"/>
		<skos:definition>specifies the quantity value that is the part of a fraction &apos;above the line&apos; and signifies the value to be divided by the denominator</skos:definition>
		<skos:note>If a fraction is considered as an ordered pair, the numerator is the first argument of the fraction.</skos:note>
	</owl:ObjectProperty>
	
	<owl:DatatypeProperty rdf:about="&cmns-qtu;hasNumericValue">
		<rdfs:label>has numeric value</rdfs:label>
		<dct:source rdf:datatype="&xsd;anyURI">https://www.omg.org/spec/SysML/</dct:source>
		<rdfs:range rdf:resource="&xsd;decimal"/>
		<skos:definition>indicates a particular magnitude or designation for a given observable characteristic that is a number</skos:definition>
	</owl:DatatypeProperty>
	
	<owl:ObjectProperty rdf:about="&cmns-qtu;hasQuantityKind">
		<rdfs:subPropertyOf rdf:resource="&cmns-cls;isClassifiedBy"/>
		<rdfs:label>has quantity kind</rdfs:label>
		<rdfs:range rdf:resource="&cmns-qtu;QuantityKind"/>
		<skos:definition>indicates the class of mutually comparable quantities involved in the definition of an individual quantity or factor</skos:definition>
	</owl:ObjectProperty>
	
	<owl:ObjectProperty rdf:about="&cmns-qtu;hasQuantityValue">
		<rdfs:label>has quantity value</rdfs:label>
		<rdfs:range rdf:resource="&cmns-qtu;QuantityValue"/>
		<skos:definition>relates something (an expression, formula, etc.) to its magnitude expressed as a number together with its unit of measure (if applicable)</skos:definition>
	</owl:ObjectProperty>
	
	<owl:ObjectProperty rdf:about="&cmns-qtu;isDerivedFrom">
		<rdfs:label>is derived from</rdfs:label>
		<skos:definition>indicates something from which the subject is obtained or determined</skos:definition>
		<skos:example>a derived quantity is derived from a base quantity; a derived unit is derived from a base unit</skos:example>
	</owl:ObjectProperty>
	
	<owl:DatatypeProperty rdf:about="&cmns-qtu;isMaximumInclusive">
		<rdfs:label>is maximum inclusive</rdfs:label>
		<rdfs:domain rdf:resource="&cmns-qtu;MeasurementScale"/>
		<rdfs:range rdf:resource="&xsd;boolean"/>
		<skos:definition>indicates whether the scale includes the absolute maximum permissive value or not</skos:definition>
	</owl:DatatypeProperty>
	
	<owl:DatatypeProperty rdf:about="&cmns-qtu;isMinimumInclusive">
		<rdfs:label>is minimum inclusive</rdfs:label>
		<rdfs:domain rdf:resource="&cmns-qtu;MeasurementScale"/>
		<rdfs:range rdf:resource="&xsd;boolean"/>
		<skos:definition>indicates whether the scale includes the absolute minimum permissive value or not</skos:definition>
	</owl:DatatypeProperty>
	
	<owl:ObjectProperty rdf:about="&cmns-qtu;specializes">
		<rdfs:label>specializes</rdfs:label>
		<skos:definition>indicates something whose nature is more general (broader than) the subject</skos:definition>
	</owl:ObjectProperty>

</rdf:RDF>